@prefix clarify: <http://clarify2020.eu/vocab/> .
@prefix owl: <http://www.w3.org/2002/07/owl#> .
@prefix rdf: <http://www.w3.org/1999/02/22-rdf-syntax-ns#> .
@prefix rdfs: <http://www.w3.org/2000/01/rdf-schema#> .
@prefix xsd: <http://www.w3.org/2001/XMLSchema#> .
@prefix dcterms: <http://purl.org/dc/terms/> .
@prefix dc: <http://purl.org/dc/elements/1.1/> .

#################################################################################################################################################
#################################################################################################################################################

<https://github.com/tibonto/clarify> rdf:type owl:Ontology ;
                                   owl:versionIRI <https://github.com/tibonto/clarify/tree/v5.0> ;
                                   dc:contributor "Samaneh Jozashoori" ,
                                                  "Maria-Esther Vidal" ;
                                   dc:creator "CLARIFY project" ;
                                   dc:title "CLARIFY Unified Schema" ;
                                   owl:versionInfo "v5.0" .

#################################################################################################################################################
#################################################################################################################################################
#################################################################################################################################################
###############################################################   Classes   #####################################################################
#################################################################################################################################################
#################################################################################################################################################
#################################################################################################################################################


######################################################################################################################################
#########################################################    SLCG    #################################################################
######################################################################################################################################



clarify:Concept	rdf:type	owl:Class;
				rdfs:label	"Concept";
				rdfs:comment "Constituents of thoughts or real world entities.";
				dcterms:modified "2020-10-19"^^xsd:date;
				dcterms:creator <https://www.tib.eu/en/research-development/scientific-data-management/staff/samaneh-jozashoori/>.

clarify:Annotation	rdf:type	owl:Class;
					rdfs:label	"Annotation";
					rdfs:comment "Annotation of a concept including label, id and source of concept.";
					dcterms:modified "2020-10-19"^^xsd:date;
					dcterms:creator <https://www.tib.eu/en/research-development/scientific-data-management/staff/samaneh-jozashoori/>.

clarify:CancerPatient	rdf:type	owl:Class;
					rdfs:label	"CancerPatient";
					rdfs:comment "Cancer Patient independent of type of their cancer.";
					dcterms:modified "2020-10-19"^^xsd:date;
					dcterms:creator <https://www.tib.eu/en/research-development/scientific-data-management/staff/samaneh-jozashoori/>.

clarify:LCPatient	rdf:type	owl:Class;
				rdfs:label	"LungCancerPatient";
				rdfs:subClassOf	clarify:CancerPatient;
				rdfs:comment "A patient who is diagnosed with Lung Cancer.";
				dcterms:modified "2020-10-19"^^xsd:date;			
				dcterms:creator <https://www.tib.eu/en/research-development/scientific-data-management/staff/samaneh-jozashoori/>.

clarify:Observation	rdf:type	owl:Class;
				rdfs:label	"Observation";
				rdfs:subClassOf	clarify:Concept;
				rdfs:comment "Any record that relates to monitoring a process.";
				dcterms:modified "2021-01-25"^^xsd:date;			
				dcterms:creator <https://www.tib.eu/en/research-development/scientific-data-management/staff/samaneh-jozashoori/>.

clarify:Diagnosis  	rdf:type owl:Class;
					rdfs:label	"Diagnosis";
					rdfs:subClassOf	clarify:Observation;
					rdfs:comment "The identification of the nature of an illness or other problem by examination of the symptoms.";
					dcterms:modified "2020-09-15"^^xsd:date;
					dcterms:creator <https://www.tib.eu/en/research-development/scientific-data-management/staff/samaneh-jozashoori/>.	

clarify:Sex	rdf:type	owl:Class;
			rdfs:label	"Sex";
			rdfs:subClassOf	clarify:Concept;
			rdfs:comment "One of the main biological categories of female or male (independent of the gender identity).";
			dcterms:modified "2020-10-19"^^xsd:date;
			dcterms:creator <https://www.tib.eu/en/research-development/scientific-data-management/staff/samaneh-jozashoori/>.

clarify:Race	rdf:type	owl:Class;
				rdfs:label	"Race";
				rdfs:subClassOf	clarify:Concept;
				rdfs:comment "Categories of humankind that shares certain distinctive physical traits.";
				dcterms:modified "2020-10-19"^^xsd:date;
				dcterms:creator <https://www.tib.eu/en/research-development/scientific-data-management/staff/samaneh-jozashoori/>.						

clarify:Biomarker	 rdf:type	owl:Class;
					rdfs:label	"Biomarker";
					rdfs:subClassOf	clarify:Concept;
					rdfs:comment "A biomarker, or biological marker is a measurable indicator of some biological state or condition.";
					dcterms:modified "2020-10-19"^^xsd:date;
					dcterms:creator <https://www.tib.eu/en/research-development/scientific-data-management/staff/samaneh-jozashoori/>.

clarify:ProgressionRelapse	rdf:type	owl:Class;
							rdfs:label	"ProgressionRelapse";
							rdfs:subClassOf	clarify:Concept;
							rdfs:comment "Indicates the existance of progression OR relapse in the patient.";
							dcterms:modified "2021-02-25"^^xsd:date;
							dcterms:creator <https://www.tib.eu/en/research-development/scientific-data-management/staff/samaneh-jozashoori/>.	

clarify:PatientHistory	rdf:type	owl:Class;
						rdfs:label	"PatientHistory";
						rdfs:subClassOf	clarify:Concept;
						rdfs:comment "Represents the cancers from which the patient have suffered before.";
						dcterms:modified "2020-10-20"^^xsd:date;
						dcterms:creator <https://www.tib.eu/en/research-development/scientific-data-management/staff/samaneh-jozashoori/>.

clarify:FamilyHistory	rdf:type	owl:Class;
						rdfs:label	"FamilyHistory";
						rdfs:subClassOf	clarify:Concept;
						rdfs:comment "Represents the cancers from which the direct blood relatives of the patient have suffered.";
						dcterms:modified "2020-10-20"^^xsd:date;
						dcterms:creator <https://www.tib.eu/en/research-development/scientific-data-management/staff/samaneh-jozashoori/>.	

clarify:ClinicalTrial	rdf:type	owl:Class;
						rdfs:label	"ClinicalTrial";
						rdfs:subClassOf	clarify:Observation;
						rdfs:comment "Represents the clinical trial that the patient is involved in.";
						dcterms:modified "2020-10-20"^^xsd:date;
						dcterms:creator <https://www.tib.eu/en/research-development/scientific-data-management/staff/samaneh-jozashoori/>.

clarify:OccurrenceLocation	rdf:type	owl:Class;
							rdfs:label	"OccurrenceLocation";
							rdfs:subClassOf	clarify:Concept;
							rdfs:comment "Superclass of metastasis location proportion and radiotherapy location.";
							dcterms:modified "2021-02-25"^^xsd:date;
							dcterms:creator <https://www.tib.eu/en/research-development/scientific-data-management/staff/samaneh-jozashoori/>.

clarify:MetastasisLocation	rdf:type	owl:Class;
							rdfs:label	"MetastasisLocation";
							rdfs:subClassOf	clarify:OccurrenceLocation;
							rdfs:comment "Determines the area to which the cancer is metastasized.";
							dcterms:modified "2020-10-20"^^xsd:date;
							dcterms:creator <https://www.tib.eu/en/research-development/scientific-data-management/staff/samaneh-jozashoori/>.

clarify:OncologicalTreatmentLine	rdf:type	owl:Class;
								rdfs:label	"OncologicalTreatmentLine";
								rdfs:subClassOf clarify:Observation;
								rdfs:comment "Records of patients in clinical notes that are related to oncological treatment lines";
								dcterms:modified "2020-10-20"^^xsd:date;
								dcterms:creator <https://www.tib.eu/en/research-development/scientific-data-management/staff/samaneh-jozashoori/>.

clarify:RadiotherapyTreatmentLine	rdf:type	owl:Class;
								rdfs:label	"RadiotherapyTreatmentLine";
								rdfs:subClassOf clarify:OncologicalTreatmentLine;
								rdfs:comment "Records of patients in clinical notes that are related to radiotherapy treatment lines";
								dcterms:modified "2020-09-15"^^xsd:date;
								dcterms:creator <https://www.tib.eu/en/research-development/scientific-data-management/staff/samaneh-jozashoori/>.	

clarify:ClinicalTrialTreatmentLine	rdf:type	owl:Class;
									rdfs:label	"ClinicalTrialTreatmentLine";
									rdfs:subClassOf clarify:OncologicalTreatmentLine;
									rdfs:comment "Records of patients in clinical notes that are related to clinical trial treatment lines";
									dcterms:modified "2021-04-07"^^xsd:date;
									dcterms:creator <https://www.tib.eu/en/research-development/scientific-data-management/staff/samaneh-jozashoori/>.	

clarify:OncologicalSurgery	rdf:type	owl:Class;
							rdfs:label	"OncologicalSurgery";
							rdfs:subClassOf clarify:Concept;
							rdfs:comment "Is the branch of surgery applied to oncology; it focuses on the surgical management of tumors, especially cancerous tumors.";
							dcterms:modified "2020-10-20"^^xsd:date;
							dcterms:creator <https://www.tib.eu/en/research-development/scientific-data-management/staff/samaneh-jozashoori/>.																																	

clarify:Drug	rdf:type	owl:Class;
				rdfs:label	"Drug";
				rdfs:subClassOf	clarify:Concept;
				rdfs:comment "A substance used as a medication or in the preparation of medication.";
				dcterms:modified "2020-10-20"^^xsd:date;
				dcterms:creator <https://www.tib.eu/en/research-development/scientific-data-management/staff/samaneh-jozashoori/>.

clarify:StageClassification	rdf:type	owl:Class;
									rdfs:label	"StageClassification";
									rdfs:subClassOf	clarify:Concept;
									rdfs:comment "Techniques that are applied to indicate the TNM stage.";
									dcterms:modified "2020-10-21"^^xsd:date;
									dcterms:creator <https://www.tib.eu/en/research-development/scientific-data-management/staff/samaneh-jozashoori/>.

clarify:ClinicalStageClassification	rdf:type	owl:Class;
									rdfs:label	"ClinicalStageClassification";
									rdfs:subClassOf	clarify:StageClassification;
									rdfs:comment "The clinical technique that is applied to indicate the TNM stage.";
									dcterms:modified "2020-10-21"^^xsd:date;
									dcterms:creator <https://www.tib.eu/en/research-development/scientific-data-management/staff/samaneh-jozashoori/>.

clarify:PathologicalStageClassification	rdf:type	owl:Class;
										rdfs:label	"PathologicalStageClassification";
										rdfs:subClassOf	clarify:StageClassification;
										rdfs:comment "The pathological technique that is applied to indicate the TNM stage.";
										dcterms:modified "2020-10-21"^^xsd:date;
										dcterms:creator <https://www.tib.eu/en/research-development/scientific-data-management/staff/samaneh-jozashoori/>.

clarify:Disorder	rdf:type	owl:Class;
					rdfs:label	"Disorder";
					rdfs:subClassOf	clarify:Concept;
					rdfs:comment "A particular abnormal condition that negatively affects the structure or function of all or part of an organism, and that is not due to any immediate external injury.";
					dcterms:modified "2020-10-21"^^xsd:date;
					dcterms:creator <https://www.tib.eu/en/research-development/scientific-data-management/staff/samaneh-jozashoori/>.

clarify:ComorbidityStatus	rdf:type	owl:Class;
							rdfs:label	"ComorbidityStatus";
							rdfs:subClassOf	clarify:Concept;
							rdfs:comment "Represents the existence of comorbidity in patients.";
							dcterms:modified "2021-04-07"^^xsd:date;
							dcterms:creator <https://www.tib.eu/en/research-development/scientific-data-management/staff/samaneh-jozashoori/>.

clarify:ComorbidityTreatmentLine	rdf:type	owl:Class;
									rdfs:label	"ComorbidityTreatmentLine";
									rdfs:subClassOf	clarify:Concept;
									rdfs:comment "Represents the observation of comorbidities and symptoms in patients in each treatment line.";
									dcterms:modified "2021-06-22"^^xsd:date;
									dcterms:creator <https://www.tib.eu/en/research-development/scientific-data-management/staff/samaneh-jozashoori/>.

clarify:StatusEvolution	rdf:type	owl:Class;
							rdfs:label	"StatusEvolution";
							rdfs:subClassOf	clarify:Observation;
							rdfs:comment "Patient survival status through monitoring.";
							dcterms:modified "2020-10-21"^^xsd:date;
							dcterms:creator <https://www.tib.eu/en/research-development/scientific-data-management/staff/samaneh-jozashoori/>.

clarify:TumorType	rdf:type	owl:Class;
						rdfs:subClassOf clarify:Concept;
						rdfs:label	"TumorType";
						rdfs:comment "The histology kind of the lung cancer. The type of tumor.";
						dcterms:modified "2020-09-15"^^xsd:date;
						dcterms:creator <https://www.tib.eu/en/research-development/scientific-data-management/staff/samaneh-jozashoori/>.	

clarify:PerformanceStatus	rdf:type	owl:Class;
						rdfs:subClassOf clarify:Observation;
						rdfs:label	"PerformanceStatus";
						rdfs:comment "Represents the Performance Status of the patient.";
						dcterms:modified "2020-10-21"^^xsd:date;
						dcterms:creator <https://www.tib.eu/en/research-development/scientific-data-management/staff/samaneh-jozashoori/>.	

clarify:ReproductionHistory	rdf:type	owl:Class;
							rdfs:subClassOf clarify:Concept;
							rdfs:label	"ReproductionHistory";
							rdfs:comment "Represents the reproduction history of the patient.";
							dcterms:modified "2020-10-21"^^xsd:date;
							dcterms:creator <https://www.tib.eu/en/research-development/scientific-data-management/staff/samaneh-jozashoori/>.

clarify:Prediagnosis  	rdf:type owl:Class;
					rdfs:label	"Prediagnosis";
					rdfs:subClassOf	clarify:Observation;
					rdfs:comment "Represents any symptom that isobserved in the patient prior to be diagnosed with cancer.";
					dcterms:modified "2020-10-23"^^xsd:date;
					dcterms:creator <https://www.tib.eu/en/research-development/scientific-data-management/staff/samaneh-jozashoori/>.	

clarify:Hemogram  	rdf:type owl:Class;
					rdfs:label	"Hemogram";
					rdfs:subClassOf	clarify:Observation;
					rdfs:comment "Represents a group of tests on blood samples to provide information about general health. The tests include white blood cell count (WBC), red blood cell count (RBC), hemoglobin (HGB), hematocrit (HCT), mean cell volume (MCV), mean cell hemoglobin (MCH), mean cell hemoglobin concentration (MCHC) and platelet count.";
					dcterms:modified "2020-10-23"^^xsd:date;
					dcterms:creator <https://www.tib.eu/en/research-development/scientific-data-management/staff/samaneh-jozashoori/>.	

clarify:NonOncologicalConsultation  	rdf:type owl:Class;
										rdfs:label	"NonOncologicalConsultation";
										rdfs:subClassOf	clarify:Observation;
										rdfs:comment "Represents the first consultation with a non-oncology specialist prior to be diagnosed with cancer.";
										dcterms:modified "2020-10-23"^^xsd:date;
										dcterms:creator <https://www.tib.eu/en/research-development/scientific-data-management/staff/samaneh-jozashoori/>.	

clarify:TreatmentLineType  	rdf:type owl:Class;
							rdfs:label	"TreatmentLineType";
							rdfs:subClassOf	clarify:Concept;
							rdfs:comment "Specification of the treatment line type.";
							dcterms:modified "2021-02-25"^^xsd:date;
							dcterms:creator <https://www.tib.eu/en/research-development/scientific-data-management/staff/samaneh-jozashoori/>.	

clarify:TreatementLineBestResponse  	rdf:type owl:Class;
										rdfs:label	"TreatementLineBestResponse";
										rdfs:subClassOf	clarify:Concept;
										dcterms:modified "2021-02-18"^^xsd:date;
										rdfs:comment "Indicates the best response that a patient has in a treatment line.";
										dcterms:creator <https://www.tib.eu/en/research-development/scientific-data-management/staff/samaneh-jozashoori/>.	

clarify:CancerType  rdf:type owl:Class;
					rdfs:label	"CancerType";
					rdfs:subClassOf	clarify:Concept;
					rdfs:comment "Indicates the type of the cancer.";
					dcterms:modified "2021-02-18"^^xsd:date;
					dcterms:creator <https://www.tib.eu/en/research-development/scientific-data-management/staff/samaneh-jozashoori/>.	

clarify:BiomarkerTestResult rdf:type owl:Class;
						rdfs:label	"BiomarkerTestResult";
						rdfs:subClassOf	clarify:Concept;
						rdfs:comment "Represents the results of a Biomarket test.";
						dcterms:modified "2021-03-02"^^xsd:date;
						dcterms:creator <https://www.tib.eu/en/research-development/scientific-data-management/staff/samaneh-jozashoori/>.	

clarify:TreatmentLineCycle  rdf:type owl:Class;
							rdfs:label	"TreatmentLineCycle";
							rdfs:subClassOf	clarify:Concept;
							rdfs:comment "Represents the number of cycles through which the corresponding treatment have been applied.";
							dcterms:modified "2021-02-25"^^xsd:date;
							dcterms:creator <https://www.tib.eu/en/research-development/scientific-data-management/staff/samaneh-jozashoori/>.	

clarify:TreatmentLineNumber rdf:type owl:Class;
							rdfs:label	"TreatmentLineNumber";
							rdfs:subClassOf	clarify:Concept;
							rdfs:comment "The number representing the oncological line of treatment.";
							dcterms:modified "2021-02-25"^^xsd:date;
							dcterms:creator <https://www.tib.eu/en/research-development/scientific-data-management/staff/samaneh-jozashoori/>.	

clarify:Assessment 	rdf:type owl:Class;
					rdfs:label	"Assessment";
					rdfs:subClassOf	clarify:Concept;
					rdfs:comment "Represents any procedure or technique that is applied in the process of evaluation.";
					dcterms:modified "2021-02-25"^^xsd:date;
					dcterms:creator <https://www.tib.eu/en/research-development/scientific-data-management/staff/samaneh-jozashoori/>.	

clarify:Procedure 	rdf:type owl:Class;
					rdfs:label	"Procedure";
					rdfs:subClassOf	clarify:Assessment;
					rdfs:comment "Any clinical stadification techniques that is applied as part of the evaluation.";
					dcterms:modified "2021-02-25"^^xsd:date;
					dcterms:creator <https://www.tib.eu/en/research-development/scientific-data-management/staff/samaneh-jozashoori/>.	

clarify:TrialType 	rdf:type owl:Class;
					rdfs:label	"TrialType";
					rdfs:subClassOf	clarify:Concept;
					rdfs:comment "Represents the different trials, that can be directed, drug trial or observational trial."; 
					dcterms:modified "2021-02-25"^^xsd:date;
					dcterms:creator <https://www.tib.eu/en/research-development/scientific-data-management/staff/samaneh-jozashoori/>.	

clarify:TrialParticipation 	rdf:type owl:Class;
							rdfs:label	"TrialParticipation";
							rdfs:subClassOf	clarify:Concept;
							rdfs:comment "Provides information on trila participation."; 
							dcterms:modified "2021-04-07"^^xsd:date;
							dcterms:creator <https://www.tib.eu/en/research-development/scientific-data-management/staff/samaneh-jozashoori/>.	

clarify:TrialPhase 	rdf:type owl:Class;
					rdfs:label	"TrialPhase";
					rdfs:subClassOf	clarify:Concept;
					rdfs:comment "Indicates the phase of the clinical trial.";
					dcterms:modified "2021-02-25"^^xsd:date;
					dcterms:creator <https://www.tib.eu/en/research-development/scientific-data-management/staff/samaneh-jozashoori/>.	

clarify:TumorSize 	rdf:type owl:Class;
					rdfs:label	"TumorSize";
					rdfs:subClassOf	clarify:Concept;
					rdfs:comment "Indicates the size of the patient's tumor (T).";
					dcterms:modified "2021-02-25"^^xsd:date;
					dcterms:creator <https://www.tib.eu/en/research-development/scientific-data-management/staff/samaneh-jozashoori/>.	

clarify:PatientOccupation 	rdf:type owl:Class;
							rdfs:label	"PatientOccupation";
							rdfs:subClassOf	clarify:Concept;
							rdfs:comment "Patient occupation  (during longer number of years).";
							dcterms:modified "2021-02-25"^^xsd:date;
							dcterms:creator <https://www.tib.eu/en/research-development/scientific-data-management/staff/samaneh-jozashoori/>.	

clarify:FamilyWithCancer 	rdf:type owl:Class;
							rdfs:label	"FamilyWithCancer";
							rdfs:subClassOf	clarify:Concept;
							rdfs:comment "Represents if the patient has a relative with cancer.";
							dcterms:modified "2021-02-25"^^xsd:date;
							dcterms:creator <https://www.tib.eu/en/research-development/scientific-data-management/staff/samaneh-jozashoori/>.	

clarify:FamilyType 	rdf:type owl:Class;
					rdfs:label	"FamilyType";
					rdfs:subClassOf	clarify:Concept;
					rdfs:comment "Represents the type of family kinship with the patient.";
					dcterms:modified "2021-02-25"^^xsd:date;
					dcterms:creator <https://www.tib.eu/en/research-development/scientific-data-management/staff/samaneh-jozashoori/>.	

clarify:FamilyRelationDegree 	rdf:type owl:Class;
								rdfs:label	"FamilyRelationDegree";
								rdfs:subClassOf	clarify:Concept;
								rdfs:comment "Represents the relative degree of the family member with the patient.";
								dcterms:modified "2021-07-26"^^xsd:date;
								dcterms:creator <https://www.tib.eu/en/research-development/scientific-data-management/staff/samaneh-jozashoori/>.	

clarify:CauseOfDeath 	rdf:type owl:Class;
						rdfs:label	"CauseOfDeath";
						rdfs:subClassOf	clarify:Concept;
						rdfs:comment "Indicates the lung cancer patient's cause of death.";
						dcterms:modified "2021-02-25"^^xsd:date;
						dcterms:creator <https://www.tib.eu/en/research-development/scientific-data-management/staff/samaneh-jozashoori/>.	

clarify:ReasonOfDeath 	rdf:type owl:Class;
						rdfs:label	"ReasonOfDeath";
						rdfs:subClassOf	clarify:Concept;
						rdfs:comment "Indicates the lung cancer patient's reason of death.";
						dcterms:modified "2021-02-25"^^xsd:date;
						dcterms:creator <https://www.tib.eu/en/research-development/scientific-data-management/staff/samaneh-jozashoori/>.	

clarify:CurrentStatus 	rdf:type owl:Class;
						rdfs:label	"CurrentStatus";
						rdfs:subClassOf	clarify:Concept;
						rdfs:comment "Current status of Lung Cancer patient.";
						dcterms:modified "2021-02-25"^^xsd:date;
						dcterms:creator <https://www.tib.eu/en/research-development/scientific-data-management/staff/samaneh-jozashoori/>.	

clarify:PatientCancerHistory 	rdf:type owl:Class;
								rdfs:label	"PatientCancerHistory";
								rdfs:subClassOf	clarify:Concept;
								rdfs:comment "Connection between patient and her/his family history.";
								dcterms:modified "2021-02-25"^^xsd:date;
								dcterms:creator <https://www.tib.eu/en/research-development/scientific-data-management/staff/samaneh-jozashoori/>.	

clarify:Hospital 	rdf:type owl:Class;
					rdfs:label	"Hospital";
					rdfs:subClassOf	clarify:Concept;
					rdfs:comment "Represents in which hospital the patient is hospitalized.";
					dcterms:modified "2021-02-25"^^xsd:date;
					dcterms:creator <https://www.tib.eu/en/research-development/scientific-data-management/staff/samaneh-jozashoori/>.	

clarify:City 	rdf:type owl:Class;
				rdfs:label	"City";
				rdfs:subClassOf	clarify:Concept;
				rdfs:comment  "Represents the city of residence of the patient (structured information provided by HUPHM).";
				dcterms:modified "2021-02-25"^^xsd:date;
				dcterms:creator <https://www.tib.eu/en/research-development/scientific-data-management/staff/samaneh-jozashoori/>.	

clarify:Scale 	rdf:type owl:Class;
				rdfs:label	"Scale";
				rdfs:subClassOf	clarify:Assessment;
				rdfs:comment "Represents the scale that is applied in the evaluation of the patient's performance status.";
				dcterms:modified "2021-02-25"^^xsd:date;
				dcterms:creator <https://www.tib.eu/en/research-development/scientific-data-management/staff/samaneh-jozashoori/>.	

clarify:PerformanceStatusObservation 	rdf:type owl:Class;
										rdfs:label	"PerformanceStatusObservation";
										rdfs:subClassOf	clarify:Observation;
										rdfs:comment "Indicates if the person has previous cancer.";
										dcterms:modified "2021-02-25"^^xsd:date;
										dcterms:creator <https://www.tib.eu/en/research-development/scientific-data-management/staff/samaneh-jozashoori/>.	

clarify:PerformedStudyStatus 	rdf:type owl:Class;
								rdfs:label	"PerformedStudyStatus";
								rdfs:subClassOf	clarify:Observation;
								rdfs:comment "Indicates if a study is performed on the biomarker.";
								dcterms:modified "2021-04-07"^^xsd:date;
								dcterms:creator <https://www.tib.eu/en/research-development/scientific-data-management/staff/samaneh-jozashoori/>.	

clarify:ProgressionLocation	rdf:type	owl:Class;
							rdfs:label	"ProgressionLocation";
							rdfs:subClassOf	clarify:OccurrenceLocation;
							rdfs:comment "Represents the location of occurrence of the progression/ relapse.";
							dcterms:modified "2021-02-25"^^xsd:date;
							dcterms:creator <https://www.tib.eu/en/research-development/scientific-data-management/staff/samaneh-jozashoori/>.

clarify:RadiotherapyIntention	rdf:type	owl:Class;
								rdfs:label	"RadiotherapyIntention";
								rdfs:subClassOf	clarify:Concept;
								rdfs:comment "Represents the purpose(!) of performing radiotherapy.";
								dcterms:modified "2021-02-25"^^xsd:date;
								dcterms:creator <https://www.tib.eu/en/research-development/scientific-data-management/staff/samaneh-jozashoori/>.

clarify:RadiotherapyTreatmentLineType	rdf:type	owl:Class;
										rdfs:label	"RadiotherapyTreatmentLineType";
										rdfs:subClassOf	clarify:TreatmentLineType;
										rdfs:comment "Indicates the type of radiation.";
										dcterms:modified "2021-02-25"^^xsd:date;
										dcterms:creator <https://www.tib.eu/en/research-development/scientific-data-management/staff/samaneh-jozashoori/>.

clarify:RadiotherapyLocation	rdf:type	owl:Class;
								rdfs:label	"RadiotherapyLocation";
								rdfs:subClassOf	clarify:OccurrenceLocation;
								rdfs:comment "Indicates the location of the radiotherapy: bone, holocraneal bone, lung and others.";
								dcterms:modified "2021-02-25"^^xsd:date;
								dcterms:creator <https://www.tib.eu/en/research-development/scientific-data-management/staff/samaneh-jozashoori/>.

clarify:ProgressionType	rdf:type	owl:Class;
						rdfs:label	"ProgressionType";
						rdfs:subClassOf	clarify:Concept;
						rdfs:comment "Represents type of progression that patient has experienced.";
						dcterms:modified "2021-02-25"^^xsd:date;
						dcterms:creator <https://www.tib.eu/en/research-development/scientific-data-management/staff/samaneh-jozashoori/>.

clarify:TherapyType	rdf:type	owl:Class;
					rdfs:label	"TherapyType";
					rdfs:subClassOf	clarify:Concept;
					rdfs:comment "Represents the type of therapy that is prescribed to the patient (active or palliative care -pain relieving-).";
					dcterms:modified "2021-02-25"^^xsd:date;
					dcterms:creator <https://www.tib.eu/en/research-development/scientific-data-management/staff/samaneh-jozashoori/>.

clarify:SmokerFamily	rdf:type	owl:Class;
						rdfs:label	"SmokerFamily";
						rdfs:subClassOf	clarify:Concept;
						rdfs:comment "Represents if the patient lives with smokers.";
						dcterms:modified "2021-02-25"^^xsd:date;
						dcterms:creator <https://www.tib.eu/en/research-development/scientific-data-management/staff/samaneh-jozashoori/>.

clarify:SmokingHabit	rdf:type	owl:Class;
						rdfs:label	"SmokingHabit";
						rdfs:subClassOf	clarify:Concept;
						rdfs:comment "Represents the smoking habit of the patient.";
						dcterms:modified "2021-06-04"^^xsd:date;
						dcterms:creator <https://www.tib.eu/en/research-development/scientific-data-management/staff/samaneh-jozashoori/>.

clarify:LymphNodesInvolvement	rdf:type	owl:Class;
								rdfs:label	"LymphNodesInvolvement";
								rdfs:subClassOf	clarify:Concept;
								rdfs:comment "Indicates if the lymph nodes are involved (N).";
								dcterms:modified "2021-02-25"^^xsd:date;
								dcterms:creator <https://www.tib.eu/en/research-development/scientific-data-management/staff/samaneh-jozashoori/>.

clarify:PerioperativeDeath	rdf:type	owl:Class;
							rdfs:label	"PerioperativeDeath";
							rdfs:subClassOf	clarify:CauseOfDeath;
							rdfs:comment "Represents if the perioperative death was the cause of death (30 days after surgery)."; 
							dcterms:modified "2021-02-25"^^xsd:date;
							dcterms:creator <https://www.tib.eu/en/research-development/scientific-data-management/staff/samaneh-jozashoori/>.

clarify:SurgeryResectionDegree	rdf:type	owl:Class;
								rdfs:label	"SurgeryResectionDegree";
								rdfs:subClassOf	clarify:Concept;
								rdfs:comment "Indicates the degree of the resection that is applied during the surgery.";							dcterms:modified "2021-02-25"^^xsd:date;
								dcterms:creator <https://www.tib.eu/en/research-development/scientific-data-management/staff/samaneh-jozashoori/>.

clarify:SurgeryClass	rdf:type	owl:Class;
						rdfs:label	"SurgeryClass";
						rdfs:subClassOf	clarify:Concept;
						rdfs:comment "Represents the type of the surgery.";
						dcterms:modified "2021-02-25"^^xsd:date;
						dcterms:creator <https://www.tib.eu/en/research-development/scientific-data-management/staff/samaneh-jozashoori/>.

clarify:SurgerySubType	rdf:type	owl:Class;
						rdfs:label	"SurgerySubType";
						rdfs:subClassOf	clarify:Concept;
						rdfs:comment "Represents the subtype of the surgery.";
						dcterms:modified "2021-02-25"^^xsd:date;
						dcterms:creator <https://www.tib.eu/en/research-development/scientific-data-management/staff/samaneh-jozashoori/>.

clarify:SurgeryType	rdf:type	owl:Class;
					rdfs:label	"SurgeryType";
					rdfs:subClassOf	clarify:Concept;
					rdfs:comment "Represents the type of the surgery.";
					dcterms:modified "2021-04-26"^^xsd:date;
					dcterms:creator <https://www.tib.eu/en/research-development/scientific-data-management/staff/samaneh-jozashoori/>.


clarify:MetastatisStage	rdf:type	owl:Class;
						rdfs:label	"MetastatisStage";
						rdfs:subClassOf	clarify:Concept;
						rdfs:comment "Indicates that to what extend the cancer is metastasized (M).";
						dcterms:modified "2021-02-25"^^xsd:date;
						dcterms:creator <https://www.tib.eu/en/research-development/scientific-data-management/staff/samaneh-jozashoori/>.

clarify:SurgeryPathologicalResponse	rdf:type	owl:Class;
									rdfs:label	"SurgeryPathologicalResponse";
									rdfs:subClassOf	clarify:Concept;
									rdfs:comment "Represents the type of pathological response to the surgery that the patient experienced.";
									dcterms:modified "2021-02-25"^^xsd:date;
									dcterms:creator <https://www.tib.eu/en/research-development/scientific-data-management/staff/samaneh-jozashoori/>.

clarify:SynchronousTumor	rdf:type	owl:Class;
							rdfs:label	"SynchronousTumor";
							rdfs:subClassOf	clarify:Concept;
							rdfs:comment "Represents if a synchronous tumor (a second primary cancer diagnosed within 6 months of the primary cancer) is also discovered.";
							dcterms:modified "2021-02-25"^^xsd:date;
							dcterms:creator <https://www.tib.eu/en/research-development/scientific-data-management/staff/samaneh-jozashoori/>.

clarify:TrialTarget	rdf:type	owl:Class;
					rdfs:label	"TrialTarget";
					rdfs:subClassOf	clarify:Concept;
					rdfs:comment "Indicates the name of the target of the clinical trial.";
					dcterms:modified "2021-02-25"^^xsd:date;
					dcterms:creator <https://www.tib.eu/en/research-development/scientific-data-management/staff/samaneh-jozashoori/>.

clarify:HistologyDegree	rdf:type	owl:Class;
						rdfs:label	"HistologyDegree";
						rdfs:subClassOf	clarify:Concept;
						rdfs:comment "Represents the histology degree.";
						dcterms:modified "2021-02-25"^^xsd:date;
						dcterms:creator <https://www.tib.eu/en/research-development/scientific-data-management/staff/samaneh-jozashoori/>.

clarify:AdenocarcinomaHistology	rdf:type	owl:Class;
								rdfs:label	"AdenocarcinomaHistology";
								rdfs:subClassOf	clarify:Concept;
								rdfs:comment "Represents type of adenocarcinoma (originally developement of the cancer in an organ or gland) experienced by the patient (if any).";
								dcterms:modified "2021-02-25"^^xsd:date;
								dcterms:creator <https://www.tib.eu/en/research-development/scientific-data-management/staff/samaneh-jozashoori/>.

clarify:MesotheliomaType	rdf:type	owl:Class;
							rdfs:label	"MesotheliomaType";
							rdfs:subClassOf	clarify:Concept;
							rdfs:comment "Represents the type of small cell mesothelioma (a malignant tumor that is caused by inhaled asbestos fibers and forms in the lining of the lungs, abdomen or heart) that patient is experienced (if any).";
							dcterms:modified "2021-02-25"^^xsd:date;
							dcterms:creator <https://www.tib.eu/en/research-development/scientific-data-management/staff/samaneh-jozashoori/>.

clarify:CarcinomaType	rdf:type	owl:Class;
						rdfs:label	"CarcinomaType";
						rdfs:subClassOf	clarify:Concept;
						rdfs:comment "Represents the type of carcinoma that the patient is experienced.";
						dcterms:modified "2021-02-25"^^xsd:date;
						dcterms:creator <https://www.tib.eu/en/research-development/scientific-data-management/staff/samaneh-jozashoori/>.

clarify:SmallCellCarcinomaType	rdf:type	owl:Class;
								rdfs:label	"SmallCellCarcinomaType";
								rdfs:subClassOf	clarify:Concept;
								rdfs:comment "Represents the type of small cell carcinoma that patient is experienced (if any).";
								dcterms:modified "2021-02-25"^^xsd:date;
								dcterms:creator <https://www.tib.eu/en/research-development/scientific-data-management/staff/samaneh-jozashoori/>.

clarify:SecondNeoplasm	rdf:type        owl:Class;	
						rdfs:label	"SecondNeoplasm";
						rdfs:subClassOf	clarify:Concept;
						rdfs:comment "Secondary malignant neoplasm is a malignant tumor whose cause is the treatment (usually radiation or chemotherapy) which was used for a prior tumor.";
						dcterms:modified "2021-03-18"^^xsd:date;
						dcterms:creator <https://www.tib.eu/en/research-development/scientific-data-management/staff/samaneh-jozashoori/>.

clarify:Version	rdf:type        owl:Class;	
				rdfs:label	"Version";
				rdfs:subClassOf	clarify:Concept;
				rdfs:comment "Indicates the versioning of a concept.";
				dcterms:modified "2021-04-26"^^xsd:date;
				dcterms:creator <https://www.tib.eu/en/research-development/scientific-data-management/staff/samaneh-jozashoori/>.

clarify:PerformedMonitoring	rdf:type        owl:Class;	
							rdfs:label	"PerformedMonitoring";
							rdfs:subClassOf	clarify:Concept;
							rdfs:comment "Indicates performed monitoring.";
							dcterms:modified "2021-04-29"^^xsd:date;
							dcterms:creator <https://www.tib.eu/en/research-development/scientific-data-management/staff/samaneh-jozashoori/>.

clarify:SurgeryIteration	rdf:type        owl:Class;	
							rdfs:label	"SurgeryIteration";
							rdfs:subClassOf	clarify:Concept;
							rdfs:comment "Indicates surgery iteration.";
							dcterms:modified "2021-05-17"^^xsd:date;
							dcterms:creator <https://www.tib.eu/en/research-development/scientific-data-management/staff/samaneh-jozashoori/>.

######################################################################################################################################
#####################################################    Publication    ##############################################################
######################################################################################################################################

clarify:Publication	rdf:type	owl:Class;
					rdfs:label	"Publication";
					rdfs:subClassOf	clarify:Concept;
					rdfs:comment "Scientific publications.";
					dcterms:modified "2020-12-15"^^xsd:date;
					dcterms:creator <https://www.tib.eu/en/research-development/scientific-data-management/staff/samaneh-jozashoori/>.

clarify:Author	rdf:type	owl:Class;
				rdfs:label	"Author";
				rdfs:subClassOf	clarify:Concept;
				rdfs:comment "Author of Scientific publications.";
				dcterms:modified "2021-05-17"^^xsd:date;
				dcterms:creator <https://www.tib.eu/en/research-development/scientific-data-management/staff/samaneh-jozashoori/>.

clarify:Relation	rdf:type	owl:Class;
					rdfs:label	"Relation";
					rdfs:subClassOf	clarify:Concept;
					rdfs:comment "Defines relationship between UMLS concepts.";
					dcterms:modified "2021-01-26"^^xsd:date;
					dcterms:creator <https://www.tib.eu/en/research-development/scientific-data-management/staff/samaneh-jozashoori/>.

clarify:PublicationType	rdf:type	owl:Class;
						rdfs:label	"PublicationType";
						rdfs:subClassOf	clarify:Concept;
						rdfs:comment "Defines the type of publication.";
						dcterms:modified "2021-06-08"^^xsd:date;
						dcterms:creator <https://www.tib.eu/en/research-development/scientific-data-management/staff/samaneh-jozashoori/>.

clarify:AFFECTS	rdf:type	owl:Class;
					rdfs:label	"AFFECTS";
					rdfs:subClassOf	clarify:Relation;
					rdfs:comment "Relation between two UMLS CUIs to represent pharmacogenomics; it implies a direct effect on.";
					dcterms:modified "2021-01-26"^^xsd:date;
					dcterms:creator <https://www.tib.eu/en/research-development/scientific-data-management/staff/samaneh-jozashoori/>.

clarify:ASSOCIATED_WITH	rdf:type	owl:Class;
					rdfs:label	"ASSOCIATED_WITH";
					rdfs:subClassOf	clarify:Relation;
					rdfs:comment "Relation between UMLS CUIs to represent the genetic etiology of disease; the relation is of type association between two terms.";
					dcterms:modified "2021-01-26"^^xsd:date;
					dcterms:creator <https://www.tib.eu/en/research-development/scientific-data-management/staff/samaneh-jozashoori/>.

clarify:AUGMENTS	rdf:type	owl:Class;
					rdfs:label	"AUGMENTS";
					rdfs:subClassOf	clarify:Relation;
					rdfs:comment "Relation between two UMLS CUIs to represent pharmacogenomics. It implies expanding or stimulating a process.";
					dcterms:modified "2021-01-26"^^xsd:date;
					dcterms:creator <https://www.tib.eu/en/research-development/scientific-data-management/staff/samaneh-jozashoori/>.

clarify:CAUSES	rdf:type	owl:Class;
					rdfs:label	"CAUSES";
					rdfs:subClassOf	clarify:Relation;
					rdfs:comment "Relation between two UMLS CUIs to represent the genetic etiology of disease; it implies bringing about a condition or an effect.";
					dcterms:modified "2021-01-26"^^xsd:date;
					dcterms:creator <https://www.tib.eu/en/research-development/scientific-data-management/staff/samaneh-jozashoori/>.

clarify:COEXISTS_WITH	rdf:type	owl:Class;
					rdfs:label	"COEXISTS_WITH";
					rdfs:subClassOf	clarify:Relation;
					rdfs:comment "Relation between two UMLS CUIs to represent the genetic etiology of disease; it implies occurring together with, or jointly.";
					dcterms:modified "2021-01-26"^^xsd:date;
					dcterms:creator <https://www.tib.eu/en/research-development/scientific-data-management/staff/samaneh-jozashoori/>.

clarify:COMPLICATES	rdf:type	owl:Class;
					rdfs:label	"COMPLICATES";
					rdfs:subClassOf	clarify:Relation;
					rdfs:comment "Relation between two UMLS CUIs to represent the genetic etiology of disease; it represents causes to become more severe or complex, or results in adverse effects.";
					dcterms:modified "2021-01-26"^^xsd:date;
					dcterms:creator <https://www.tib.eu/en/research-development/scientific-data-management/staff/samaneh-jozashoori/>.

clarify:CONVERTS_TO	rdf:type	owl:Class;
					rdfs:label	"CONVERTS_TO";
					rdfs:subClassOf	clarify:Relation;
					rdfs:comment "Relation between two UMLS CUIs to represent the genetic etiology of disease; it implies changing from one form to another.";
					dcterms:modified "2021-01-26"^^xsd:date;
					dcterms:creator <https://www.tib.eu/en/research-development/scientific-data-management/staff/samaneh-jozashoori/>.

clarify:DIAGNOSES	rdf:type	owl:Class;
					rdfs:label	"DIAGNOSES";
					rdfs:subClassOf	clarify:Relation;
					rdfs:comment "Relation between two UMLS CUIs that represents the relation of type distinguishing or identifying the nature or characteristics of two clinical medicine terms.";
					dcterms:modified "2021-01-26"^^xsd:date;
					dcterms:creator <https://www.tib.eu/en/research-development/scientific-data-management/staff/samaneh-jozashoori/>.

clarify:DISRUPTS	rdf:type	owl:Class;
					rdfs:label	"DISRUPTS";
					rdfs:subClassOf	clarify:Relation;
					rdfs:comment "Relation between UMLS CUIs to represent pharmacogenomics; the relation is of type altering or influencing an already existing condition, state, or situation and producing a negative effect on between two terms.";
					dcterms:modified "2021-01-26"^^xsd:date;
					dcterms:creator <https://www.tib.eu/en/research-development/scientific-data-management/staff/samaneh-jozashoori/>.

clarify:INHIBITS	rdf:type	owl:Class;
					rdfs:label	"INHIBITS";
					rdfs:subClassOf	clarify:Relation;
					rdfs:comment "Relation between two UMLS CUIs that describes substance interactions in terms of decreasing, limiting, or blocks the action or function.";
					dcterms:modified "2021-01-26"^^xsd:date;
					dcterms:creator <https://www.tib.eu/en/research-development/scientific-data-management/staff/samaneh-jozashoori/>.

clarify:INTERACTS_WITH	rdf:type	owl:Class;
					rdfs:label	"INTERACTS_WITH";
					rdfs:subClassOf	clarify:Relation;
					rdfs:comment "Relation between UMLS CUIs that describes interactions between two terms representing substances.";
					dcterms:modified "2021-01-26"^^xsd:date;
					dcterms:creator <https://www.tib.eu/en/research-development/scientific-data-management/staff/samaneh-jozashoori/>.

clarify:ISA	rdf:type	owl:Class;
					rdfs:label	"ISA";
					rdfs:subClassOf	clarify:Relation;
					rdfs:comment "Relation between two UMLS CUIs that represents that if one item has this relation to another item then the first item is more specific in meaning than the second item.";
					dcterms:modified "2021-01-26"^^xsd:date;
					dcterms:creator <https://www.tib.eu/en/research-development/scientific-data-management/staff/samaneh-jozashoori/>.

clarify:LOCATION_OF	rdf:type	owl:Class;
					rdfs:label	"LOCATION_OF";
					rdfs:subClassOf	clarify:Relation;
					rdfs:comment "The position, site, or region of an entity or the site of a process.";
					dcterms:modified "2021-01-26"^^xsd:date;
					dcterms:creator <https://www.tib.eu/en/research-development/scientific-data-management/staff/samaneh-jozashoori/>.

clarify:MANIFESTATION_OF	rdf:type	owl:Class;
					rdfs:label	"MANIFESTATION_OF";
					rdfs:subClassOf	clarify:Relation;
					rdfs:comment "Relation between two UMLS CUIs that represents that part of a phenomenon which is directly observable or concretely or visibly expressed, or which gives evidence to the underlying process.";
					dcterms:modified "2021-01-26"^^xsd:date;
					dcterms:creator <https://www.tib.eu/en/research-development/scientific-data-management/staff/samaneh-jozashoori/>.

clarify:MEASUREMENT_OF	rdf:type	owl:Class;
					rdfs:label	"MEASUREMENT_OF";
					rdfs:subClassOf	clarify:Relation;
					rdfs:comment "Relation between UMLS CUIs that represents the relation of type measurement between two terms.";
					dcterms:modified "2021-01-26"^^xsd:date;
					dcterms:creator <https://www.tib.eu/en/research-development/scientific-data-management/staff/samaneh-jozashoori/>.										

clarify:MEASURES	rdf:type	owl:Class;
					rdfs:label	"MEASURES";
					rdfs:subClassOf	clarify:Relation;
					rdfs:comment "Relation between UMLS CUIs that represents the relation of type measurement  between two terms.";
					dcterms:modified "2021-01-26"^^xsd:date;
					dcterms:creator <https://www.tib.eu/en/research-development/scientific-data-management/staff/samaneh-jozashoori/>.

clarify:METHOD_OF	rdf:type	owl:Class;
					rdfs:label	"METHOD_OF";
					rdfs:subClassOf	clarify:Relation;
					rdfs:comment "Relation between two UMLS CUIs that represents the manner and sequence of events in performing an act or procedure.";
					dcterms:modified "2021-01-26"^^xsd:date;
					dcterms:creator <https://www.tib.eu/en/research-development/scientific-data-management/staff/samaneh-jozashoori/>.					

clarify:NEG_ADMINISTERED_TO	rdf:type	owl:Class;
					rdfs:label	"NEG_ADMINISTERED_TO";
					rdfs:subClassOf	clarify:Relation;
					rdfs:comment "Relation between two UMLS CUIs that represents the negation of ADMINISTERED_TO relation.";
					dcterms:modified "2021-01-26"^^xsd:date;
					dcterms:creator <https://www.tib.eu/en/research-development/scientific-data-management/staff/samaneh-jozashoori/>.

clarify:NEG_AFFECTS	rdf:type	owl:Class;
					rdfs:label	"NEG_AFFECTS";
					rdfs:subClassOf	clarify:Relation;
					rdfs:comment "Relation between two UMLS CUIs to represent pharmacogenomics; it implies a direct effect on.";
					dcterms:modified "2021-01-26"^^xsd:date;
					dcterms:creator <https://www.tib.eu/en/research-development/scientific-data-management/staff/samaneh-jozashoori/>.

clarify:NEG_ASSOCIATED_WITH	rdf:type	owl:Class;
					rdfs:label	"NEG_ASSOCIATED_WITH";
					rdfs:subClassOf	clarify:Relation;
					rdfs:comment "Relation between UMLS CUIs to represent the genetic etiology of disease; the relation is of type association between two terms.";
					dcterms:modified "2021-01-26"^^xsd:date;
					dcterms:creator <https://www.tib.eu/en/research-development/scientific-data-management/staff/samaneh-jozashoori/>.

clarify:NEG_AUGMENTS	rdf:type	owl:Class;
					rdfs:label	"NEG_AUGMENTS";
					rdfs:subClassOf	clarify:Relation;
					rdfs:comment "Relation between two UMLS CUIs that represents the negation of AUGMENTS relation.";
					dcterms:modified "2021-01-26"^^xsd:date;
					dcterms:creator <https://www.tib.eu/en/research-development/scientific-data-management/staff/samaneh-jozashoori/>.

clarify:NEG_CAUSES	rdf:type	owl:Class;
					rdfs:label	"NEG_CAUSES";
					rdfs:subClassOf	clarify:Relation;
					rdfs:comment "Relation between two UMLS CUIs that represents the negation of CAUSES relation.";
					dcterms:modified "2021-01-26"^^xsd:date;
					dcterms:creator <https://www.tib.eu/en/research-development/scientific-data-management/staff/samaneh-jozashoori/>.

clarify:NEG_COEXISTS_WITH	rdf:type	owl:Class;
					rdfs:label	"NEG_COEXISTS_WITH";
					rdfs:subClassOf	clarify:Relation;
					rdfs:comment "Relation between two UMLS CUIs that represents the negation of COEXISTS_WITH relation.";
					dcterms:modified "2021-01-26"^^xsd:date;
					dcterms:creator <https://www.tib.eu/en/research-development/scientific-data-management/staff/samaneh-jozashoori/>.

clarify:NEG_COMPLICATES	rdf:type	owl:Class;
					rdfs:label	"NEG_COMPLICATES";
					rdfs:subClassOf	clarify:Relation;
					rdfs:comment "Relation between two UMLS CUIs that represents the negation of COMPLICATES relation.";
					dcterms:modified "2021-01-26"^^xsd:date;
					dcterms:creator <https://www.tib.eu/en/research-development/scientific-data-management/staff/samaneh-jozashoori/>.

clarify:NEG_CONVERTS_TO	rdf:type	owl:Class;
					rdfs:label	"NEG_CONVERTS_TO";
					rdfs:subClassOf	clarify:Relation;
					rdfs:comment "Relation between two UMLS CUIs that represents the negation of CONVERTS_TO relation.";
					dcterms:modified "2021-01-26"^^xsd:date;
					dcterms:creator <https://www.tib.eu/en/research-development/scientific-data-management/staff/samaneh-jozashoori/>.

clarify:NEG_DIAGNOSES	rdf:type	owl:Class;
					rdfs:label	"NEG_DIAGNOSES";
					rdfs:subClassOf	clarify:Relation;
					rdfs:comment "Relation between two UMLS CUIs that represents the negation of DIAGNOSES relation.";
					dcterms:modified "2021-01-26"^^xsd:date;
					dcterms:creator <https://www.tib.eu/en/research-development/scientific-data-management/staff/samaneh-jozashoori/>.

clarify:NEG_DISRUPTS	rdf:type	owl:Class;
					rdfs:label	"NEG_DISRUPTS";
					rdfs:subClassOf	clarify:Relation;
					rdfs:comment "Relation between two UMLS CUIs that represents the negation of DISRUPTS relation.";
					dcterms:modified "2021-01-26"^^xsd:date;
					dcterms:creator <https://www.tib.eu/en/research-development/scientific-data-management/staff/samaneh-jozashoori/>.

clarify:NEG_INHIBITS	rdf:type	owl:Class;
					rdfs:label	"NEG_INHIBITS";
					rdfs:subClassOf	clarify:Relation;
					rdfs:comment "Relation between two UMLS CUIs that represents the negation of INHIBITS relation.";
					dcterms:modified "2021-01-26"^^xsd:date;
					dcterms:creator <https://www.tib.eu/en/research-development/scientific-data-management/staff/samaneh-jozashoori/>.

clarify:NEG_INTERACTS_WITH	rdf:type	owl:Class;
					rdfs:label	"NEG_INTERACTS_WITH";
					rdfs:subClassOf	clarify:Relation;
					rdfs:comment "Relation between two UMLS CUIs that represents the negation of INTERACTS_WITH relation.";
					dcterms:modified "2021-01-26"^^xsd:date;
					dcterms:creator <https://www.tib.eu/en/research-development/scientific-data-management/staff/samaneh-jozashoori/>.

clarify:NEG_ISA	rdf:type	owl:Class;
					rdfs:label	"NEG_ISA";
					rdfs:subClassOf	clarify:Relation;
					rdfs:comment "Relation between two UMLS CUIs that represents the negation of ISA relation.";
					dcterms:modified "2021-01-26"^^xsd:date;
					dcterms:creator <https://www.tib.eu/en/research-development/scientific-data-management/staff/samaneh-jozashoori/>.

clarify:NEG_LOCATION_OF	rdf:type	owl:Class;
					rdfs:label	"NEG_LOCATION_OF";
					rdfs:subClassOf	clarify:Relation;
					rdfs:comment "Relation between two UMLS CUIs that represents the negation of LOCATION_OF relation.";
					dcterms:modified "2021-01-26"^^xsd:date;
					dcterms:creator <https://www.tib.eu/en/research-development/scientific-data-management/staff/samaneh-jozashoori/>.

clarify:NEG_MANIFESTATION_OF	rdf:type	owl:Class;
					rdfs:label	"NEG_MANIFESTATION_OF";
					rdfs:subClassOf	clarify:Relation;
					rdfs:comment "Relation between two UMLS CUIs that represents the negation of MANIFESTATION_OF relation.";
					dcterms:modified "2021-01-26"^^xsd:date;
					dcterms:creator <https://www.tib.eu/en/research-development/scientific-data-management/staff/samaneh-jozashoori/>.

clarify:NEG_MEASURES	rdf:type	owl:Class;
					rdfs:label	"NEG_MEASURES";
					rdfs:subClassOf	clarify:Relation;
					rdfs:comment "Relation between two UMLS CUIs that represents the negation of MEASURES relation.";
					dcterms:modified "2021-01-26"^^xsd:date;
					dcterms:creator <https://www.tib.eu/en/research-development/scientific-data-management/staff/samaneh-jozashoori/>.

clarify:NEG_METHOD_OF	rdf:type	owl:Class;
					rdfs:label	"NEG_METHOD_OF";
					rdfs:subClassOf	clarify:Relation;
					rdfs:comment "Relation between two UMLS CUIs that represents the negation of METHOD_OF relation.";
					dcterms:modified "2021-01-26"^^xsd:date;
					dcterms:creator <https://www.tib.eu/en/research-development/scientific-data-management/staff/samaneh-jozashoori/>.

clarify:NEG_OCCURS_IN	rdf:type	owl:Class;
					rdfs:label	"NEG_OCCURS_IN";
					rdfs:subClassOf	clarify:Relation;
					rdfs:comment "Relation between two UMLS CUIs that represents the negation of OCCURS_IN relation.";
					dcterms:modified "2021-01-26"^^xsd:date;
					dcterms:creator <https://www.tib.eu/en/research-development/scientific-data-management/staff/samaneh-jozashoori/>.

clarify:NEG_PART_OF	rdf:type	owl:Class;
					rdfs:label	"NEG_PART_OF";
					rdfs:subClassOf	clarify:Relation;
					rdfs:comment "Relation between two UMLS CUIs that represents the negation of PART_OF relation.";
					dcterms:modified "2021-01-26"^^xsd:date;
					dcterms:creator <https://www.tib.eu/en/research-development/scientific-data-management/staff/samaneh-jozashoori/>.

clarify:NEG_PRECEDES	rdf:type	owl:Class;
					rdfs:label	"NEG_PRECEDES";
					rdfs:subClassOf	clarify:Relation;
					rdfs:comment "Relation between two UMLS CUIs that represents the negation of PRECEDES relation.";
					dcterms:modified "2021-01-26"^^xsd:date;
					dcterms:creator <https://www.tib.eu/en/research-development/scientific-data-management/staff/samaneh-jozashoori/>.

clarify:NEG_PREDISPOSES	rdf:type	owl:Class;
					rdfs:label	"NEG_PREDISPOSES";
					rdfs:subClassOf	clarify:Relation;
					rdfs:comment "Relation between two UMLS CUIs that represents the negation of PREDISPOSES relation.";
					dcterms:modified "2021-01-26"^^xsd:date;
					dcterms:creator <https://www.tib.eu/en/research-development/scientific-data-management/staff/samaneh-jozashoori/>.

clarify:NEG_PREVENTS	rdf:type	owl:Class;
					rdfs:label	"NEG_PREVENTS";
					rdfs:subClassOf	clarify:Relation;
					rdfs:comment "Relation between two UMLS CUIs that represents the negation of PREVENTS relation.";
					dcterms:modified "2021-01-26"^^xsd:date;
					dcterms:creator <https://www.tib.eu/en/research-development/scientific-data-management/staff/samaneh-jozashoori/>.

clarify:NEG_PROCESS_OF	rdf:type	owl:Class;
					rdfs:label	"NEG_PROCESS_OF";
					rdfs:subClassOf	clarify:Relation;
					rdfs:comment "Relation between two UMLS CUIs that represents the negation of PROCESS_OF relation.";
					dcterms:modified "2021-01-26"^^xsd:date;
					dcterms:creator <https://www.tib.eu/en/research-development/scientific-data-management/staff/samaneh-jozashoori/>.

clarify:NEG_PRODUCES	rdf:type	owl:Class;
					rdfs:label	"NEG_PRODUCES";
					rdfs:subClassOf	clarify:Relation;
					rdfs:comment "Relation between two UMLS CUIs that represents the negation of PRODUCES relation.";
					dcterms:modified "2021-01-26"^^xsd:date;
					dcterms:creator <https://www.tib.eu/en/research-development/scientific-data-management/staff/samaneh-jozashoori/>.

clarify:NEG_STIMULATES	rdf:type	owl:Class;
					rdfs:label	"NEG_STIMULATES";
					rdfs:subClassOf	clarify:Relation;
					rdfs:comment "Relation between two UMLS CUIs that represents the negation of STIMULATES relation.";
					dcterms:modified "2021-01-26"^^xsd:date;
					dcterms:creator <https://www.tib.eu/en/research-development/scientific-data-management/staff/samaneh-jozashoori/>.

clarify:NEG_TREATS	rdf:type	owl:Class;
					rdfs:label	"NEG_TREATS";
					rdfs:subClassOf	clarify:Relation;
					rdfs:comment "Relation between two UMLS CUIs that represents the negation of TREATS relation.";
					dcterms:modified "2021-01-26"^^xsd:date;
					dcterms:creator <https://www.tib.eu/en/research-development/scientific-data-management/staff/samaneh-jozashoori/>.

clarify:NEG_USES	rdf:type	owl:Class;
					rdfs:label	"NEG_USES";
					rdfs:subClassOf	clarify:Relation;
					rdfs:comment "Relation between two UMLS CUIs that represents the negation of USES relation.";
					dcterms:modified "2021-01-26"^^xsd:date;
					dcterms:creator <https://www.tib.eu/en/research-development/scientific-data-management/staff/samaneh-jozashoori/>.

clarify:NEG_higher_than	rdf:type	owl:Class;
					rdfs:label	"NEG_higher_than";
					rdfs:subClassOf	clarify:Relation;
					rdfs:comment "Relation between two UMLS CUIs that represents the negation of higher_than relation.";
					dcterms:modified "2021-01-26"^^xsd:date;
					dcterms:creator <https://www.tib.eu/en/research-development/scientific-data-management/staff/samaneh-jozashoori/>.

clarify:NEG_lower_than	rdf:type	owl:Class;
					rdfs:label	"NEG_lower_than";
					rdfs:subClassOf	clarify:Relation;
					rdfs:comment "Relation between two UMLS CUIs that represents the negation of lower_than relation.";
					dcterms:modified "2021-01-26"^^xsd:date;
					dcterms:creator <https://www.tib.eu/en/research-development/scientific-data-management/staff/samaneh-jozashoori/>.

clarify:NEG_same_as	rdf:type	owl:Class;
					rdfs:label	"NEG_same_as";
					rdfs:subClassOf	clarify:Relation;
					rdfs:comment "Relation between two UMLS CUIs that represents the negation of same_as relation.";
					dcterms:modified "2021-01-26"^^xsd:date;
					dcterms:creator <https://www.tib.eu/en/research-development/scientific-data-management/staff/samaneh-jozashoori/>.

clarify:OCCURS_IN	rdf:type	owl:Class;
					rdfs:label	"OCCURS_IN";
					rdfs:subClassOf	clarify:Relation;
					rdfs:comment "Relation between two UMLS CUIs that represents having incidence in a group or population.";
					dcterms:modified "2021-01-26"^^xsd:date;
					dcterms:creator <https://www.tib.eu/en/research-development/scientific-data-management/staff/samaneh-jozashoori/>.

clarify:PART_OF	rdf:type	owl:Class;
					rdfs:label	"PART_OF";
					rdfs:subClassOf	clarify:Relation;
					rdfs:comment "Relation between two UMLS CUIs that represents composing, with one or more other physical units, some larger whole.";
					dcterms:modified "2021-01-26"^^xsd:date;
					dcterms:creator <https://www.tib.eu/en/research-development/scientific-data-management/staff/samaneh-jozashoori/>.

clarify:PRECEDES	rdf:type	owl:Class;
					rdfs:label	"PRECEDES";
					rdfs:subClassOf	clarify:Relation;
					rdfs:comment "Relation between two UMLS CUIs that represents occurring earlier in time.";
					dcterms:modified "2021-01-26"^^xsd:date;
					dcterms:creator <https://www.tib.eu/en/research-development/scientific-data-management/staff/samaneh-jozashoori/>.

clarify:PREDISPOSES	rdf:type	owl:Class;
					rdfs:label	"PREDISPOSES";
					rdfs:subClassOf	clarify:Relation;
					rdfs:comment "Relation between UMLS CUIs to represent the genetic etiology of disease; the relation is of type predisposal between two terms.";
					dcterms:modified "2021-01-26"^^xsd:date;
					dcterms:creator <https://www.tib.eu/en/research-development/scientific-data-management/staff/samaneh-jozashoori/>.

clarify:PREVENTS	rdf:type	owl:Class;
					rdfs:label	"PREVENTS";
					rdfs:subClassOf	clarify:Relation;
					rdfs:comment "Relation between UMLS CUIs to represent stopping, hindering or eliminating an action or condition.";
					dcterms:modified "2021-01-26"^^xsd:date;
					dcterms:creator <https://www.tib.eu/en/research-development/scientific-data-management/staff/samaneh-jozashoori/>.

clarify:PROCESS_OF	rdf:type	owl:Class;
					rdfs:label	"PROCESS_OF";
					rdfs:subClassOf	clarify:Relation;
					rdfs:comment "Relation between two UMLS CUIs that represents the disorder occurs in (higher) organisms.";
					dcterms:modified "2021-01-26"^^xsd:date;
					dcterms:creator <https://www.tib.eu/en/research-development/scientific-data-management/staff/samaneh-jozashoori/>.

clarify:PRODUCES	rdf:type	owl:Class;
					rdfs:label	"PRODUCES";
					rdfs:subClassOf	clarify:Relation;
					rdfs:comment "Relation between UMLS CUIs that represents bringing forth, generating or creating.";
					dcterms:modified "2021-01-26"^^xsd:date;
					dcterms:creator <https://www.tib.eu/en/research-development/scientific-data-management/staff/samaneh-jozashoori/>.

clarify:STIMULATES	rdf:type	owl:Class;
					rdfs:label	"STIMULATES";
					rdfs:subClassOf	clarify:Relation;
					rdfs:comment "Relation between UMLS CUIs that describes substance interactions in terms of increasing or facilitating the action or function.";
					dcterms:modified "2021-01-26"^^xsd:date;
					dcterms:creator <https://www.tib.eu/en/research-development/scientific-data-management/staff/samaneh-jozashoori/>.

clarify:TREATS	rdf:type	owl:Class;
					rdfs:label	"TREATS";
					rdfs:subClassOf	clarify:Relation;
					rdfs:comment "Relation between UMLS CUIs that represents the relation of type treating between two clinical medicine terms.";
					dcterms:modified "2021-01-26"^^xsd:date;
					dcterms:creator <https://www.tib.eu/en/research-development/scientific-data-management/staff/samaneh-jozashoori/>.

clarify:USES	rdf:type	owl:Class;
					rdfs:label	"USES";
					rdfs:subClassOf	clarify:Relation;
					rdfs:comment "Relation between two UMLS CUIs that represents employing in the carrying out of some activity.";
					dcterms:modified "2021-01-26"^^xsd:date;
					dcterms:creator <https://www.tib.eu/en/research-development/scientific-data-management/staff/samaneh-jozashoori/>.

clarify:compared_with	rdf:type	owl:Class;
					rdfs:label	"compared_with";
					rdfs:subClassOf	clarify:Relation;
					rdfs:comment "Relation between UMLS CUIs that represents the relation of type comparative between two terms.";
					dcterms:modified "2021-01-26"^^xsd:date;
					dcterms:creator <https://www.tib.eu/en/research-development/scientific-data-management/staff/samaneh-jozashoori/>.

clarify:higher_than	rdf:type	owl:Class;
					rdfs:label	"higher_than";
					rdfs:subClassOf	clarify:Relation;
					rdfs:comment "Relation between UMLS CUIs that represents the relation of type comparative between two terms";
					dcterms:modified "2021-01-26"^^xsd:date;
					dcterms:creator <https://www.tib.eu/en/research-development/scientific-data-management/staff/samaneh-jozashoori/>.

clarify:lower_than	rdf:type	owl:Class;
					rdfs:label	"lower_than";
					rdfs:subClassOf	clarify:Relation;
					rdfs:comment "Relation between UMLS CUIs that represents the relation of type comparative between two terms.";
					dcterms:modified "2021-01-26"^^xsd:date;
					dcterms:creator <https://www.tib.eu/en/research-development/scientific-data-management/staff/samaneh-jozashoori/>.

clarify:same_as	rdf:type	owl:Class;
					rdfs:label	"same_as";
					rdfs:subClassOf	clarify:Relation;
					rdfs:comment "Relation between UMLS CUIs that represents the relation of type comparative between two terms.";
					dcterms:modified "2021-01-26"^^xsd:date;
					dcterms:creator <https://www.tib.eu/en/research-development/scientific-data-management/staff/samaneh-jozashoori/>.



######################################################################################################################################
#########################################################    Drug    #################################################################
######################################################################################################################################


clarify:Drug	rdf:type	owl:Class;
			rdfs:label	"Drug";
			rdfs:subClassOf	clarify:Concept;
			rdfs:comment "A substance used as a medication or in the preparation of medication.";
			dcterms:modified "2020-09-14"^^xsd:date;
			dcterms:creator <https://www.tib.eu/en/research-development/scientific-data-management/staff/samaneh-jozashoori/>.

clarify:NonOncologicalDrug	rdf:type	owl:Class;
							rdfs:label	"NonOncologicalDrug";
							rdfs:subClassOf	clarify:Drug;
							rdfs:comment "A Drug which is prescribed to treat disorders other than cancer.";
							dcterms:modified "2021-06-29"^^xsd:date;
							dcterms:creator <https://www.tib.eu/en/research-development/scientific-data-management/staff/samaneh-jozashoori/>.

clarify:OncologicalDrug	rdf:type	owl:Class;
							rdfs:label	"OncologicalDrug";
							rdfs:subClassOf	clarify:Drug;
							rdfs:comment "A Drug category which is prescribed to treat cancer.";
							dcterms:modified "2021-06-29"^^xsd:date;
							dcterms:creator <https://www.tib.eu/en/research-development/scientific-data-management/staff/samaneh-jozashoori/>.

clarify:ChemotherapyDrug	rdf:type	owl:Class;
							rdfs:label	"ChemotherapyDrug";
							rdfs:subClassOf	clarify:OncologicalDrug;
							rdfs:comment "A subcategory of oncological drugs.";
							dcterms:modified "2021-06-29"^^xsd:date;
							dcterms:creator <https://www.tib.eu/en/research-development/scientific-data-management/staff/samaneh-jozashoori/>.

clarify:TKIDrug	rdf:type	owl:Class;
				rdfs:label	"TKIDrug";
				rdfs:subClassOf	clarify:OncologicalDrug;
				rdfs:comment "A subcategory of oncological drugs.";
				dcterms:modified "2021-06-29"^^xsd:date;
				dcterms:creator <https://www.tib.eu/en/research-development/scientific-data-management/staff/samaneh-jozashoori/>.

clarify:ImmunotherapyDrug	rdf:type	owl:Class;
							rdfs:label	"ImmunotherapyDrug";
							rdfs:subClassOf	clarify:OncologicalDrug;
							rdfs:comment "A subcategory of oncological drugs.";
							dcterms:modified "2021-06-29"^^xsd:date;
							dcterms:creator <https://www.tib.eu/en/research-development/scientific-data-management/staff/samaneh-jozashoori/>.

clarify:AngiogenesisInhibitorDrug	rdf:type	owl:Class;
									rdfs:label	"AngiogenesisInhibitorDrug";
									rdfs:subClassOf	clarify:OncologicalDrug;
									rdfs:comment "A subcategory of oncological drugs.";
									dcterms:modified "2021-06-29"^^xsd:date;
									dcterms:creator <https://www.tib.eu/en/research-development/scientific-data-management/staff/samaneh-jozashoori/>.

clarify:Biomarker	 rdf:type	owl:Class;
					rdfs:label	"Biomarker";
					rdfs:subClassOf	clarify:Concept;
					rdfs:comment "A biomarker, or biological marker is a measurable indicator of some biological state or condition.";
					dcterms:modified "2020-09-14"^^xsd:date;
					dcterms:creator <https://www.tib.eu/en/research-development/scientific-data-management/staff/samaneh-jozashoori/>.

clarify:Phenotype	rdf:type	owl:Class;
					rdfs:label	"Phenotype";
					rdfs:subClassOf	clarify:Concept;
					rdfs:comment "The set of observable characteristics of an individual resulting from the interaction of its genotype with the environment. This class include side effects that result from different drugs.";
					dcterms:modified "2020-12-15"^^xsd:date;
					dcterms:creator <https://www.tib.eu/en/research-development/scientific-data-management/staff/samaneh-jozashoori/>.

clarify:Target	rdf:type	owl:Class;
				rdfs:label	"Target";
				rdfs:subClassOf	clarify:Concept;
				rdfs:comment "A drug target is a molecule in the body, usually a protein, that is intrinsically associated with a particular disease process and that could be addressed by a drug to produce a desired therapeutic effect.";
				dcterms:modified "2020-12-15"^^xsd:date;
				dcterms:creator <https://www.tib.eu/en/research-development/scientific-data-management/staff/samaneh-jozashoori/>.

clarify:Protein	rdf:type	owl:Class;
				rdfs:label	"Protein";
				rdfs:subClassOf	clarify:Concept;
				rdfs:comment "Large and complex molecules that play many critical roles in the body. They are required for the structure, function and regulation of the body's tissues and organs.";
				dcterms:modified "2020-12-15"^^xsd:date;
				dcterms:creator <https://www.tib.eu/en/research-development/scientific-data-management/staff/samaneh-jozashoori/>.

clarify:Enzyme	rdf:type	owl:Class;
				rdfs:label	"Enzyme";
				rdfs:subClassOf	clarify:Concept;
				rdfs:comment "Macromolecular biological catalyst that accelerate chemical reactions. Most enzymes are proteins.";
				dcterms:modified "2020-12-15"^^xsd:date;
				dcterms:creator <https://www.tib.eu/en/research-development/scientific-data-management/staff/samaneh-jozashoori/>.

clarify:DrugDrugInteraction	rdf:type	owl:Class;
				rdfs:label	"DrugDrugInteraction";
				rdfs:subClassOf	clarify:Interaction;
				rdfs:comment "The relation between two drugs that interact.";
				dcterms:modified "2020-12-15"^^xsd:date;
				dcterms:creator <https://www.tib.eu/en/research-development/scientific-data-management/staff/samaneh-jozashoori/>.

clarify:Interaction	rdf:type owl:Class;
			rdfs:label	"Interaction";
			rdfs:subClassOf	clarify:INTERACTS_WITH;
			rdfs:comment "Interaction between drugs and disorder, enzyme, target.";
			dcterms:modified "2021-01-07"^^xsd:date;
			dcterms:creator <https://www.tib.eu/en/research-development/scientific-data-management/staff/samaneh-jozashoori/>.

clarify:DrugDisorderInteraction	rdf:type	owl:Class;
				rdfs:label	"DrugDisorderInteraction";
				rdfs:subClassOf	clarify:Interaction;
				rdfs:comment "A drug-induced disorder.";
				dcterms:modified "2020-12-15"^^xsd:date;
				dcterms:creator <https://www.tib.eu/en/research-development/scientific-data-management/staff/maria-isabel-castellanos/>.

clarify:DrugEnzymeInteraction	rdf:type	owl:Class;
				rdfs:label	"DrugEnzymeInteraction";
				rdfs:subClassOf	clarify:Interaction;
				rdfs:comment "Interactions similar to drug receptor interactions where drugs resemble the natural substrates and bind enzymes.";
				dcterms:modified "2020-12-15"^^xsd:date;
				dcterms:creator <https://www.tib.eu/en/research-development/scientific-data-management/staff/samaneh-jozashoori/>.

clarify:DrugSideEffectInteraction	rdf:type	owl:Class;
						rdfs:label	"DrugSideEffectInteraction";
						rdfs:subClassOf	clarify:Interaction;
						rdfs:comment "Effects of drugs, whether therapeutic or adverse, that are secondary to the one intended.";
						dcterms:modified "2020-12-15"^^xsd:date;
						dcterms:creator <https://www.tib.eu/en/research-development/scientific-data-management/staff/samaneh-jozashoori/>.

clarify:DrugTargetInteraction	rdf:type	owl:Class;
				rdfs:label	"DrugTargetInteraction";
				rdfs:subClassOf	clarify:Interaction;
				rdfs:comment "Interactions between chemical compounds and the protein targets in the human body.";
				dcterms:modified "2020-12-15"^^xsd:date;
				dcterms:creator <https://www.tib.eu/en/research-development/scientific-data-management/staff/samaneh-jozashoori/>.

clarify:SymmetricDrugDrugInteraction	rdf:type	owl:Class;
				rdfs:label	"SymmetricDrugDrugInteraction";
				rdfs:subClassOf	clarify:DrugDrugInteraction;
				rdfs:comment "The interactions between two drugs that do not change the effectiveness of the drugs.";
				dcterms:modified "2020-12-15"^^xsd:date;
				dcterms:creator <https://www.tib.eu/en/research-development/scientific-data-management/staff/samaneh-jozashoori/>.

clarify:NonSymmetricDrugDrugInteraction	rdf:type	owl:Class;
				rdfs:label	"NonSymmetricDrugDrugInteraction";
				rdfs:subClassOf	clarify:DrugDrugInteraction;
				rdfs:comment "The interactions between two drugs that change the effectiveness of the drugs.";
				dcterms:modified "2021-07-01"^^xsd:date;
				dcterms:creator <https://www.tib.eu/en/research-development/scientific-data-management/staff/samaneh-jozashoori/>.


clarify:AdverseEvent	rdf:type	owl:Class;
				rdfs:label	"AdverseEvent";
				rdfs:subClassOf	clarify:Concept;
				rdfs:comment "The concept that explains the consequence of the drug drug interaction resulting in their effectiveness.";
				dcterms:modified "2020-12-15"^^xsd:date;
				dcterms:creator <https://www.tib.eu/en/research-development/scientific-data-management/staff/samaneh-jozashoori/>.

clarify:Impact	rdf:type	owl:Class;
				rdfs:label	"Impact";
				rdfs:subClassOf	clarify:Concept;
				rdfs:comment "The concept that explains the impact of the drug drug interaction resulting in the effectiveness of the object drug.";
				dcterms:modified "2020-12-15"^^xsd:date;
				dcterms:creator <https://www.tib.eu/en/research-development/scientific-data-management/staff/samaneh-jozashoori/>.

clarify:CancerStage	rdf:type	owl:Class;
					rdfs:label	"CancerStage";
					rdfs:comment "Represents the assessment of the stage of tumor in a particular date.";
					dcterms:modified "2020-09-14"^^xsd:date;
					dcterms:creator <https://www.tib.eu/en/research-development/scientific-data-management/staff/samaneh-jozashoori/>.

clarify:SemanticType	rdf:type	owl:Class;
						rdfs:label	"SemanticType";
						rdfs:subClassOf	clarify:Concept;
						rdfs:comment "Represents the Semantic Type provided by UMLS.";
						dcterms:modified "2021-07-21"^^xsd:date;
						dcterms:creator <https://www.tib.eu/en/research-development/scientific-data-management/staff/samaneh-jozashoori/>.

clarify:SemanticTypeGroup	rdf:type	owl:Class;
							rdfs:label	"SemanticTypeGroup";
							rdfs:subClassOf	clarify:Concept;
							rdfs:comment "Represents the Semantic Type Group provided by UMLS.";
							dcterms:modified "2021-07-21"^^xsd:date;
							dcterms:creator <https://www.tib.eu/en/research-development/scientific-data-management/staff/samaneh-jozashoori/>.

######################################################################################################################################
#################################################    Drug Predictions   ##############################################################
######################################################################################################################################

clarify:DrugDrugPrediction	rdf:type owl:Class;
						rdfs:label	"DrugDrugPrediction";
						rdfs:subClassOf	clarify:Interaction;
						rdfs:comment "Represents the predicted relation between drugs.";
						dcterms:modified "2021-01-07"^^xsd:date;
						dcterms:creator <https://www.tib.eu/en/research-development/scientific-data-management/staff/samaneh-jozashoori/>.

clarify:DrugEnzymePrediction	rdf:type owl:Class;
							rdfs:label	"DrugEnzymePrediction";
							rdfs:subClassOf	clarify:Interaction;
							rdfs:comment "Represents the predicted relation between drug and enzyme.";
							dcterms:modified "2021-01-07"^^xsd:date;
							dcterms:creator <https://www.tib.eu/en/research-development/scientific-data-management/staff/samaneh-jozashoori/>.

clarify:DrugSideEffectPrediction	rdf:type owl:Class;
								rdfs:label	"DrugSideEffectPrediction";
								rdfs:subClassOf	clarify:Interaction;
								rdfs:comment "Represents the predicted relation between drug and side effects.";
								dcterms:modified "2021-01-07"^^xsd:date;
								dcterms:creator <https://www.tib.eu/en/research-development/scientific-data-management/staff/samaneh-jozashoori/>.

clarify:DrugTargetPrediction	rdf:type owl:Class;
							rdfs:label	"DrugTargetPrediction";
							rdfs:subClassOf	clarify:Interaction;
							rdfs:comment "Represents the predicted relation between drug and target.";
							dcterms:modified "2021-01-07"^^xsd:date;
							dcterms:creator <https://www.tib.eu/en/research-development/scientific-data-management/staff/samaneh-jozashoori/>.

#################################################################################################################################################
#################################################################################################################################################
#################################################################################################################################################
######################################################## Properties - attributes ################################################################
#################################################################################################################################################
#################################################################################################################################################
#################################################################################################################################################


######################################################################################################################################
#########################################################    SLCG    #################################################################
######################################################################################################################################

clarify:annID	rdf:type	owl:DatatypeProperty;
				rdfs:label	"annID";
				rdfs:domain clarify:Annotation;
				rdfs:range	rdfs:Literal;
				rdfs:comment	"Identification of instances of Annotation class";	
				dcterms:modified "2020-11-19"^^xsd:date;
				dcterms:creator <https://www.tib.eu/en/research-development/scientific-data-management/staff/samaneh-jozashoori/>.

clarify:date	rdf:type	owl:DatatypeProperty;
								rdfs:label	"date";
								rdfs:domain	clarify:Concept;
								rdfs:range	rdfs:Literal;
								rdfs:comment "Represents the date of occurrence.";
								dcterms:modified "2020-10-20"^^xsd:date;							
								dcterms:creator <https://www.tib.eu/en/research-development/scientific-data-management/staff/samaneh-jozashoori/>.

clarify:previousCancerTypeDescription	rdf:type	owl:DatatypeProperty;
										rdfs:label	"previousCancerTypeDescription";
										rdfs:domain	clarify:Concept;
										rdfs:range	rdfs:Literal;
										rdfs:comment "Provides extra texual descriptions about the concept.";
										dcterms:modified "2020-10-21"^^xsd:date;							
										dcterms:creator <https://www.tib.eu/en/research-development/scientific-data-management/staff/samaneh-jozashoori/>.

clarify:birthDate	rdf:type	owl:DatatypeProperty;
						rdfs:label	"birthDate";
						rdfs:domain	clarify:LCPatient;
						rdfs:range	rdfs:Literal;
						rdfs:comment "Represents the birth date of the patient.";
						dcterms:modified "2020-10-19"^^xsd:date;
						dcterms:creator <https://www.tib.eu/en/research-development/scientific-data-management/staff/samaneh-jozashoori/>.		

clarify:biomarkerSpecification	rdf:type	owl:DatatypeProperty;
								rdfs:label	"biomarkerSpecification";
								rdfs:domain	clarify:Biomarker;
								rdfs:range	rdfs:Literal;
								rdfs:comment "Textual description of a molecular marker.";
								dcterms:modified "2020-10-19"^^xsd:date;
								dcterms:creator <https://www.tib.eu/en/research-development/scientific-data-management/staff/samaneh-jozashoori/>.

clarify:numberOfFamilyWithLC	rdf:type	owl:DatatypeProperty;
									rdfs:label	"numberOfFamilyWithLC";
									rdfs:domain	clarify:FamilyHistory;
									rdfs:range	rdfs:Literal;
									rdfs:comment "Represents the number of family members with lung cancer.";
									dcterms:modified "2020-10-20"^^xsd:date;							
									dcterms:creator <https://www.tib.eu/en/research-development/scientific-data-management/staff/samaneh-jozashoori/>.

clarify:numberOfFamilyWithOtherCancers	rdf:type	owl:DatatypeProperty;
										rdfs:label	"numberOfFamilyWithOtherCancers";
										rdfs:domain	clarify:FamilyHistory;
										rdfs:range	rdfs:Literal;
										rdfs:comment "Represents the number of family members with cancers other than lung.";
										dcterms:modified "2020-10-20"^^xsd:date;							
										dcterms:creator <https://www.tib.eu/en/research-development/scientific-data-management/staff/samaneh-jozashoori/>.

clarify:treatmentLineDosage	rdf:type	owl:DatatypeProperty;
							rdfs:label	"treatmentLineDosage";
							rdfs:domain	clarify:OncologicalTreatmentLine;
							rdfs:range	rdfs:Literal;
							rdfs:comment "Represents the dosage that is prescribed to the patient.";
							dcterms:modified "2020-10-20"^^xsd:date;														
							dcterms:creator <https://www.tib.eu/en/research-development/scientific-data-management/staff/samaneh-jozashoori/>.

clarify:treatmentLineFractioning	rdf:type	owl:DatatypeProperty;
									rdfs:label	"treatmentLineFractioning";
									rdfs:domain	clarify:OncologicalTreatmentLine;
									rdfs:range	rdfs:Literal;
									rdfs:comment "Represents the radiotherapy fraction that is prescribed to the patient.";
									dcterms:modified "2020-11-19"^^xsd:date;														
									dcterms:creator <https://www.tib.eu/en/research-development/scientific-data-management/staff/samaneh-jozashoori/>.

clarify:disorderLabel	rdf:type owl:DatatypeProperty;
							rdfs:label "disorderLabel";
							rdfs:domain clarify:Disorder;
						  	rdfs:range rdfs:Literal;
							rdfs:comment "Disorder label.";
							dcterms:modified "2020-10-21"^^xsd:date;
							dcterms:creator <https://www.tib.eu/en/research-development/scientific-data-management/staff/samaneh-jozashoori/>.

clarify:lastMonitoringDate	rdf:type owl:DatatypeProperty;
							rdfs:label "lastMonitoringDate";
							rdfs:domain clarify:StatusEvolution;
						  	rdfs:range rdfs:Literal;
							rdfs:comment "Represents the date on which the patient was monitored for the last time.";
							dcterms:modified "2020-10-21"^^xsd:date;
							dcterms:creator <https://www.tib.eu/en/research-development/scientific-data-management/staff/samaneh-jozashoori/>.

clarify:deathDate	rdf:type	owl:DatatypeProperty;
					rdfs:label	"deathDate";
					rdfs:domain	clarify:StatusEvolution;
					rdfs:range	rdfs:Literal;
					rdfs:comment "Represents the lung cancer patient's date of death (structured information provided by HUPHM).";
					dcterms:modified "2020-10-21"^^xsd:date;
					dcterms:creator <https://www.tib.eu/en/research-development/scientific-data-management/staff/samaneh-jozashoori/>.

clarify:numberOfCigarettesPerDay	rdf:type	owl:DatatypeProperty;	
									rdfs:label	"numberOfCigarettesPerDay";
									rdfs:domain	clarify:CancerPatient;
									rdfs:range	rdfs:Literal;
									rdfs:comment	"The number of cigarettes per day that the patient smokes.";
									dcterms:modified "2020-10-21"^^xsd:date;
									dcterms:creator <https://www.tib.eu/en/research-development/scientific-data-management/staff/samaneh-jozashoori/>.

clarify:numberOfCigarettesPerYear	rdf:type	owl:DatatypeProperty;	
									rdfs:label	"numberOfCigarettesPerYear";
									rdfs:domain	clarify:CancerPatient;
									rdfs:range	rdfs:Literal;
									rdfs:comment	"The number of cigarettes per year that the patient smokes.";
									dcterms:modified "2020-11-19"^^xsd:date;
									dcterms:creator <https://www.tib.eu/en/research-development/scientific-data-management/staff/samaneh-jozashoori/>.

clarify:numberOfYearsOfSmoking	rdf:type        owl:DatatypeProperty;	
								rdfs:label	"numberOfYearsOfSmoking";
								rdfs:domain	clarify:CancerPatient;
								rdfs:range	rdfs:Literal;
								rdfs:comment "Represents for how many years the patient used to be an active smoker.";
								dcterms:modified "2020-10-21"^^xsd:date;
								dcterms:creator <https://www.tib.eu/en/research-development/scientific-data-management/staff/samaneh-jozashoori/>.

clarify:treatementLineEndingDate	rdf:type owl:DatatypeProperty;	
									rdfs:label	"treatementLineEndingDate";
									rdfs:domain	clarify:OncologicalTreatmentLine;
									rdfs:range	rdfs:Literal;
									rdfs:comment "Represents the ending date of the treatment line.";
									dcterms:modified "2021-02-25"^^xsd:date;
									dcterms:creator <https://www.tib.eu/en/research-development/scientific-data-management/staff/samaneh-jozashoori/>.

clarify:treatementLineStartDate	rdf:type owl:DatatypeProperty;	
								rdfs:label	"treatementLineStartDate";
								rdfs:domain	clarify:OncologicalTreatmentLine;
								rdfs:range	rdfs:Literal;
								rdfs:comment "Represents the starting date of the treatment line.";
								dcterms:modified "2021-02-25"^^xsd:date;
								dcterms:creator <https://www.tib.eu/en/research-development/scientific-data-management/staff/samaneh-jozashoori/>.

clarify:hasOriginalValue	rdf:type owl:DatatypeProperty;	
							rdfs:label	"hasOriginalValue";
							rdfs:domain	clarify:Concept;
							rdfs:range	rdfs:Literal;
							rdfs:comment "The original value of the instance in the RDB provided by UPM.";
							dcterms:modified "2021-05-17"^^xsd:date;
							dcterms:creator <https://www.tib.eu/en/research-development/scientific-data-management/staff/samaneh-jozashoori/>.

clarify:biomarkerAnalysisDate	rdf:type owl:DatatypeProperty;	
								rdfs:label	"biomarkerAnalysisDate";
								rdfs:domain	clarify:CancerPatient;
								rdfs:range	rdfs:Literal;
								rdfs:comment "The date on which a biomarker test of the patient is analysed.";
								dcterms:modified "2021-05-17"^^xsd:date;
								dcterms:creator <https://www.tib.eu/en/research-development/scientific-data-management/staff/samaneh-jozashoori/>.

clarify:surgerySubTypeSpecification	rdf:type owl:DatatypeProperty;	
									rdfs:label	"surgerySubTypeSpecification";
									rdfs:domain	clarify:SurgerySubType;
									rdfs:range	rdfs:Literal;
									rdfs:comment "Further specification of the surgery subtype.";
									dcterms:modified "2021-05-17"^^xsd:date;
									dcterms:creator <https://www.tib.eu/en/research-development/scientific-data-management/staff/samaneh-jozashoori/>.

clarify:age	rdf:type owl:DatatypeProperty;	
				rdfs:label	"age";
				rdfs:domain	clarify:CancerPatient;
				rdfs:range	rdfs:Literal;
				rdfs:comment "Indicates the calculated age of the patient.";
				dcterms:modified "2021-06-02"^^xsd:date;
				dcterms:creator <https://www.tib.eu/en/research-development/scientific-data-management/staff/samaneh-jozashoori/>.

######################################################################################################################################
#####################################################    Publication    ##############################################################
######################################################################################################################################

clarify:pubmedID	rdf:type owl:DatatypeProperty;
					rdfs:label "PubMed ID";
					rdfs:domain clarify:Publication;
				  	rdfs:range rdfs:Literal;
					rdfs:comment "PubMed ID.";
					dcterms:modified "2020-12-15"^^xsd:date;
					dcterms:creator <https://www.tib.eu/en/research-development/scientific-data-management/staff/samaneh-jozashoori/>.

clarify:confidence    rdf:type     owl:DatatypeProperty;
					rdfs:label	"confidence";
					rdfs:domain	clarify:Concept;
					rdfs:range	rdfs:Literal;
					rdfs:comment "Confidence score of the concept";
					dcterms:modified "2020-12-15"^^xsd:date;
					dcterms:creator <https://www.tib.eu/en/research-development/scientific-data-management/staff/samaneh-jozashoori/>.

clarify:semanticType	rdf:type	owl:DatatypeProperty;
					rdfs:label	"semanticType";
					rdfs:domain	clarify:Annotation;
					rdfs:range	rdfs:Literal;
					rdfs:comment	"A list with the allowed semantic_types for this Annotation in the UMLS.";
					dcterms:modified "2020-12-15"^^xsd:date;
					dcterms:creator <https://www.tib.eu/en/research-development/scientific-data-management/staff/samaneh-jozashoori/>.

clarify:year	rdf:type owl:DatatypeProperty;
				rdfs:label "year";
				rdfs:domain clarify:Publication;
			  	rdfs:range rdfs:Literal;
				rdfs:comment "Year of Publication.";
				dcterms:modified "2021-05-17"^^xsd:date;
				dcterms:creator <https://www.tib.eu/en/research-development/scientific-data-management/staff/samaneh-jozashoori/>.

clarify:authorName	rdf:type owl:DatatypeProperty;
					rdfs:label "authorName";
					rdfs:domain clarify:Author;
				  	rdfs:range rdfs:Literal;
					rdfs:comment "Name of author.";
					dcterms:modified "2021-05-17"^^xsd:date;
					dcterms:creator <https://www.tib.eu/en/research-development/scientific-data-management/staff/samaneh-jozashoori/>.

clarify:rankingScore_SJR	rdf:type owl:DatatypeProperty;
							rdfs:label "rankingScore_SJR";
							rdfs:domain clarify:Publication;
						  	rdfs:range rdfs:Literal;
							rdfs:comment "ranking Score_SJR Journal of publication.";
							dcterms:modified "2021-05-17"^^xsd:date;
							dcterms:creator <https://www.tib.eu/en/research-development/scientific-data-management/staff/samaneh-jozashoori/>.

clarify:rankingScore_hIndex	rdf:type owl:DatatypeProperty;
							rdfs:label "rankingScore_hIndex";
							rdfs:domain clarify:Publication;
						  	rdfs:range rdfs:Literal;
							rdfs:comment "ranking Score_hIndex of Journal of publication.";
							dcterms:modified "2021-05-17"^^xsd:date;
							dcterms:creator <https://www.tib.eu/en/research-development/scientific-data-management/staff/samaneh-jozashoori/>.
clarify:authorAffiliation	rdf:type owl:DatatypeProperty;
							rdfs:label "authorAffiliation";
							rdfs:domain clarify:Publication;
						  	rdfs:range rdfs:Literal;
							rdfs:comment "Type of publication.";
							dcterms:modified "2021-05-17"^^xsd:date;
							dcterms:creator <https://www.tib.eu/en/research-development/scientific-data-management/staff/samaneh-jozashoori/>.

######################################################################################################################################
#########################################################    Drug    #################################################################
######################################################################################################################################

clarify:annLabel	rdf:type	owl:DatatypeProperty;
					rdfs:label	"annLabel";
					rdfs:domain	clarify:Annotation;
					rdfs:range	rdfs:Literal;
					rdfs:comment	"Label of instances of Annotation class";
					dcterms:modified "2020-12-15"^^xsd:date;
					dcterms:creator <https://www.tib.eu/en/research-development/scientific-data-management/staff/samaneh-jozashoori/>.

clarify:drugLabel	rdf:type owl:DatatypeProperty;
					rdfs:label "DrugLabel";
					rdfs:domain clarify:Drug;
				  	rdfs:range rdfs:Literal;
					rdfs:comment "Drug label.";
					dcterms:modified "2020-12-15"^^xsd:date;
					dcterms:creator <https://www.tib.eu/en/research-development/scientific-data-management/staff/samaneh-jozashoori/>.

clarify:drugBankID	rdf:type	owl:DatatypeProperty;
					rdfs:label "DrugBankID";
					rdfs:domain clarify:Drug;
				  	rdfs:range rdfs:Literal;
					rdfs:comment "Drug Bank ID.";
					dcterms:modified "2020-12-15"^^xsd:date;
					dcterms:creator <https://www.tib.eu/en/research-development/scientific-data-management/staff/samaneh-jozashoori/>.

clarify:semanticTypeLabel	rdf:type	owl:DatatypeProperty;
							rdfs:label	"semanticTypeLabel";
							rdfs:domain	clarify:SemanticType;
							rdfs:range	rdfs:Literal;
			                rdfs:comment "The semantic type label provided by UMLS.";
							dcterms:modified "2021-07-21"^^xsd:date;				
							dcterms:creator <https://www.tib.eu/en/research-development/scientific-data-management/staff/samaneh-jozashoori/>.

clarify:semanticTypeGroupLabel	rdf:type	owl:DatatypeProperty;
								rdfs:label	"semanticTypeGroupLabel";
								rdfs:domain	clarify:SemanticTypeGroup;
								rdfs:range	rdfs:Literal;
				                rdfs:comment "The semantic type group label provided by UMLS.";
								dcterms:modified "2021-07-21"^^xsd:date;				
								dcterms:creator <https://www.tib.eu/en/research-development/scientific-data-management/staff/samaneh-jozashoori/>.

clarify:semanticTypeDefition	rdf:type	owl:DatatypeProperty;
								rdfs:label	"semanticTypeDefition";
								rdfs:domain	clarify:SemanticType;
								rdfs:range	rdfs:Literal;
				                rdfs:comment "The semantic type definition provided by UMLS.";
								dcterms:modified "2021-07-21"^^xsd:date;				
								dcterms:creator <https://www.tib.eu/en/research-development/scientific-data-management/staff/samaneh-jozashoori/>.

clarify:biomarkerLabel	rdf:type	owl:DatatypeProperty;
				rdfs:label	"biomarkerLabel";
				rdfs:domain	clarify:Biomarker;
				rdfs:range	rdfs:Literal;
				rdfs:comment	"The name of biomarker.";
				dcterms:modified "2020-12-15"^^xsd:date;
				dcterms:creator <https://www.tib.eu/en/research-development/scientific-data-management/staff/samaneh-jozashoori/>.

clarify:targetID	rdf:type	owl:DatatypeProperty;
					rdfs:label "targetID";
					rdfs:domain clarify:Target;
				  	rdfs:range rdfs:Literal;
					rdfs:comment "Target ID.";
					dcterms:modified "2020-12-15"^^xsd:date;
					dcterms:creator <https://www.tib.eu/en/research-development/scientific-data-management/staff/samaneh-jozashoori/>.

clarify:targetLabel	rdf:type	owl:DatatypeProperty;
				rdfs:label	"targetLabel";
				rdfs:domain	clarify:Target;
				rdfs:range	rdfs:Literal;
				rdfs:comment	"Target Label";
				dcterms:modified "2020-12-15"^^xsd:date;
				dcterms:creator <https://www.tib.eu/en/research-development/scientific-data-management/staff/samaneh-jozashoori/>.

clarify:proteinID	rdf:type owl:DatatypeProperty;
					rdfs:label	"proteinID";
					rdfs:domain clarify:Protein;
					rdfs:range rdfs:Literal;
					rdfs:comment	"Uniprot Accession key for protein.";
					dcterms:modified "2020-12-15"^^xsd:date;
					dcterms:creator <https://www.tib.eu/en/research-development/scientific-data-management/staff/samaneh-jozashoori/>.

clarify:proteinLabel	rdf:type owl:DatatypeProperty;
					rdfs:label	"proteinLabel";
					rdfs:domain clarify:Protein;
					rdfs:range rdfs:Literal;
					rdfs:comment "Represents the name of protein.";
					dcterms:modified "2020-12-15"^^xsd:date;
					dcterms:creator <https://www.tib.eu/en/research-development/scientific-data-management/staff/samaneh-jozashoori/>.

clarify:enzymeID	rdf:type owl:DatatypeProperty;
					rdfs:label "EnzymeID";
					rdfs:domain clarify:Enzyme;
				  	rdfs:range rdfs:Literal;
					rdfs:comment "Enzyme ID.";
					dcterms:modified "2020-12-15"^^xsd:date;
					dcterms:creator <https://www.tib.eu/en/research-development/scientific-data-management/staff/samaneh-jozashoori/>.

clarify:enzymeLabel	rdf:type owl:DatatypeProperty;
					rdfs:label "EnzymeLabel";
					rdfs:domain clarify:Enzyme;
				  	rdfs:range rdfs:Literal;
					rdfs:comment "Enzyme Label.";
					dcterms:modified "2020-12-15"^^xsd:date;
					dcterms:creator <https://www.tib.eu/en/research-development/scientific-data-management/staff/samaneh-jozashoori/>.

clarify:disorderLabel	rdf:type	owl:DatatypeProperty;
					rdfs:label "DisorderLabel";
					rdfs:domain clarify:Disorder;
				  	rdfs:range rdfs:Literal;
					rdfs:comment "Disorder Label.";
					dcterms:modified "2020-09-14"^^xsd:date;
					dcterms:creator <https://www.tib.eu/en/research-development/scientific-data-management/staff/samaneh-jozashoori/>.

clarify:targetID	rdf:type	owl:DatatypeProperty;
					rdfs:label "targetID";
					rdfs:domain clarify:Target;
				  	rdfs:range rdfs:Literal;
					rdfs:comment "Target ID.";
					dcterms:modified "2020-09-14"^^xsd:date;
					dcterms:creator <https://www.tib.eu/en/research-development/scientific-data-management/staff/samaneh-jozashoori/>.
					
clarify:targetLabel	rdf:type	owl:DatatypeProperty;
				rdfs:label	"targetLabel";
				rdfs:domain	clarify:Target;
				rdfs:range	rdfs:Literal;
				rdfs:comment	"Target Label";
				dcterms:modified "2020-09-14"^^xsd:date;
				dcterms:creator <https://www.tib.eu/en/research-development/scientific-data-management/staff/samaneh-jozashoori/>.

clarify:phenotypeLabel	rdf:type owl:DatatypeProperty;
					rdfs:label "PhenotypeLabel";
					rdfs:domain clarify:Phenotype;
				  	rdfs:range rdfs:Literal;
					rdfs:comment "Phenotype Label.";
					dcterms:modified "2020-12-15"^^xsd:date;
					dcterms:creator <https://www.tib.eu/en/research-development/scientific-data-management/staff/samaneh-jozashoori/>.

clarify:toxicityType	rdf:type owl:DatatypeProperty;
					rdfs:label "toxicityType";
					rdfs:domain clarify:Phenotype;
				  	rdfs:range rdfs:Literal;
					rdfs:comment "Toxicity Label.";
					dcterms:modified "2020-12-15"^^xsd:date;
					dcterms:creator <https://www.tib.eu/en/research-development/scientific-data-management/staff/samaneh-jozashoori/>.

clarify:externalLink	rdf:type owl:DatatypeProperty;
					rdfs:label "externalLink";
					rdfs:domain clarify:Concept;
				  	rdfs:range xsd:anyURI;
					rdfs:comment "Link to external resources.";
					dcterms:modified "2020-12-15"^^xsd:date;
					dcterms:creator <https://www.tib.eu/en/research-development/scientific-data-management/staff/samaneh-jozashoori/>.

clarify:uniprotID	rdf:type	owl:DatatypeProperty;
					rdfs:label "uniprotID";
					rdfs:domain clarify:Concept;
				  	rdfs:range rdfs:Literal;
					rdfs:comment "External relationship to accession ID in uniprot.";
					dcterms:modified "2020-12-15"^^xsd:date;
					dcterms:creator <https://www.tib.eu/en/research-development/scientific-data-management/staff/samaneh-jozashoori/>.

clarify:dse_AvgFrequency	rdf:type	owl:DatatypeProperty;
							rdfs:label	"dse_AvgFrequency";
							rdfs:domain	clarify:DrugSideEffectInteraction;
							rdfs:range	rdfs:Literal;
							rdfs:comment	"Represents the average frequecy of particular drug having specific side effect.";
							dcterms:modified "2020-12-15"^^xsd:date;
							dcterms:creator <https://www.tib.eu/en/research-development/scientific-data-management/staff/samaneh-jozashoori/>.

clarify:ddi_description	rdf:type	owl:DatatypeProperty;
						rdfs:label	"ddi_description";
						rdfs:domain	clarify:DrugDrugInteraction;
						rdfs:range	rdfs:Literal;
						rdfs:comment "The texual description of the drug drug interacion.";
						dcterms:modified "2021-06-29"^^xsd:date;
						dcterms:creator <https://www.tib.eu/en/research-development/scientific-data-management/staff/samaneh-jozashoori/>.	

clarify:drugAbsorption	rdf:type	owl:DatatypeProperty;
						rdfs:label	"drugAbsorption";
						rdfs:domain	clarify:Drug;
						rdfs:range	rdfs:Literal;
						rdfs:comment "The texual explanation about the drug absorption.";
						dcterms:modified "2021-06-29"^^xsd:date;
						dcterms:creator <https://www.tib.eu/en/research-development/scientific-data-management/staff/samaneh-jozashoori/>.	

clarify:drugsMechanismOfAction	rdf:type	owl:DatatypeProperty;
								rdfs:label	"drugsMechanismOfAction";
								rdfs:domain	clarify:Drug;
								rdfs:range	rdfs:Literal;
								rdfs:comment "The texual explanation about the mechanism of action of the drug.";
								dcterms:modified "2021-06-29"^^xsd:date;
								dcterms:creator <https://www.tib.eu/en/research-development/scientific-data-management/staff/samaneh-jozashoori/>.	

######################################################################################################################################
#################################################    Drug Predictions   ##############################################################
######################################################################################################################################

clarify:interactor2	rdf:type	owl:ObjectProperty;
							rdfs:label	"interactor2";
							rdfs:domain	clarify:Interaction;
							rdfs:range	clarify:Concept;
							rdfs:comment	"Relation which connects an interacion to the second involved concept (e.g. disorder, enzyme,...).";
							dcterms:modified "2021-01-07"^^xsd:date;
							dcterms:creator <https://www.tib.eu/en/research-development/scientific-data-management/staff/samaneh-jozashoori/>.							

clarify:predictionMethod	rdf:type	owl:DatatypeProperty;
							rdfs:label	"predictionMethod";
							rdfs:domain	clarify:Interaction;
							rdfs:range	rdfs:Literal;
							rdfs:comment "Represents the prediction method that is used in order to extract DDI predictions from literature or databases.";
							dcterms:modified "2021-01-07"^^xsd:date;
							dcterms:creator <https://www.tib.eu/en/research-development/scientific-data-management/staff/samaneh-jozashoori/>.	

clarify:methodAbbreviation	rdf:type	owl:DatatypeProperty;
							rdfs:label	"methodAbbreviation";
							rdfs:domain	clarify:Interaction;
							rdfs:range	rdfs:Literal;
							rdfs:comment "Represents the abbreviation of the prediction method that is used.";
							dcterms:modified "2021-01-07"^^xsd:date;
							dcterms:creator <https://www.tib.eu/en/research-development/scientific-data-management/staff/samaneh-jozashoori/>.

clarify:total_number_of_metastasis	rdf:type	owl:DatatypeProperty;
									rdfs:label	"total_number_of_metastasis";
									rdfs:domain	clarify:LCPatient;
									rdfs:range	rdfs:Literal;
									rdfs:comment "Indicates the total number of metastasis of the patient.";
									dcterms:modified "2021-04-29"^^xsd:date;
									dcterms:creator <https://www.tib.eu/en/research-development/scientific-data-management/staff/samaneh-jozashoori/>.


#################################################################################################################################################																																			
#################################################################################################################################################
#################################################################################################################################################
#################################################### Properties - relationships #################################################################
#################################################################################################################################################
#################################################################################################################################################
#################################################################################################################################################


######################################################################################################################################
##########################################################    SLCG    ################################################################
######################################################################################################################################

clarify:hasCUIAnnotation	rdf:type owl:ObjectProperty;
							rdfs:label	"hasCUIAnnotation";
							rdfs:domain clarify:Concept;
			  				rdfs:range clarify:Annotation;
							rdfs:comment	"CUI annotation of the concept.";
							dcterms:modified "2020-10-19"^^xsd:date;
							dcterms:creator <https://www.tib.eu/en/research-development/scientific-data-management/staff/samaneh-jozashoori/>.

clarify:sex	rdf:type	owl:ObjectProperty;
			rdfs:label	"sex";
			rdfs:domain	clarify:CancerPatient;
			rdfs:range	clarify:Sex;
			rdfs:comment	"Association of the patient to one of the two main biological categories of female or male.";
			dcterms:modified "2020-10-19"^^xsd:date;
			dcterms:creator <https://www.tib.eu/en/research-development/scientific-data-management/staff/samaneh-jozashoori/>.	

clarify:hasRace	rdf:type	owl:ObjectProperty;
				rdfs:label	"hasRace";
				rdfs:domain	clarify:CancerPatient;
				rdfs:range	clarify:Race;
				rdfs:comment	"Association of the patient with one of the categories of humankind that shares certain distinctive physical traits.";
				dcterms:modified "2020-11-16"^^xsd:date;
				dcterms:creator <https://www.tib.eu/en/research-development/scientific-data-management/staff/samaneh-jozashoori/>.		

clarify:hasBiomarker	rdf:type	owl:ObjectProperty;
						rdfs:label	"hasBiomarker";
						rdfs:domain	clarify:Concept;
						rdfs:range	clarify:Biomarker;
						rdfs:comment "Associates a cancer patient with an observed biomarker.";
						dcterms:modified "2020-10-19"^^xsd:date;						
						dcterms:creator <https://www.tib.eu/en/research-development/scientific-data-management/staff/samaneh-jozashoori/>.						

clarify:involved_in	rdf:type	owl:ObjectProperty;
								rdfs:label	"involved_in";
								rdfs:domain	clarify:CancerPatient;
								rdfs:range	clarify:ClinicalTrial;
								rdfs:comment "Relation between the cancer patient and the clinical trial.";
								dcterms:modified "2020-10-20"^^xsd:date;								
								dcterms:creator <https://www.tib.eu/en/research-development/scientific-data-management/staff/samaneh-jozashoori/>.	

clarify:hasDiagnosisStage	rdf:type	owl:ObjectProperty;
								rdfs:label	"hasDiagnosisStage";
								rdfs:domain	clarify:Diagnosis;
								rdfs:range	clarify:CancerStage;
								rdfs:comment "Relation between the diagnosis observation and the coded cancer stage (at the diagnosis time).";
								dcterms:modified "2020-12-10"^^xsd:date;							
								dcterms:creator <https://www.tib.eu/en/research-development/scientific-data-management/staff/samaneh-jozashoori/>.

clarify:hasDiagnosis	rdf:type     owl:ObjectProperty;
						rdfs:label	"hasDiagnosis";
						rdfs:domain	clarify:CancerPatient;
						rdfs:range	clarify:Diagnosis;
						rdfs:comment "Patient's initial diagnosis.";
						dcterms:modified "2020-10-20"^^xsd:date;
						dcterms:creator <https://www.tib.eu/en/research-development/scientific-data-management/staff/samaneh-jozashoori/>.			

clarify:hasOncologicalTreatmentLine       rdf:type     owl:ObjectProperty;
										rdfs:label	"hasOncologicalTreatmentLine";
										rdfs:domain	clarify:LCPatient;
										rdfs:range	clarify:OncologicalTreatmentLine;
										rdfs:comment "Relation between the patient and the oncological treatment line that is received by the patient.";
										dcterms:modified "2020-10-20"^^xsd:date;
										dcterms:creator <https://www.tib.eu/en/research-development/scientific-data-management/staff/samaneh-jozashoori/>.

clarify:hasRadiotherapyTreatmentLine    rdf:type     owl:ObjectProperty;
										rdfs:label	"hasRadiotherapyTreatmentLine";
										rdfs:domain	clarify:LCPatient;
										rdfs:range	clarify:RadiotherapyTreatmentLine;
										rdfs:comment "Relation between the patient and the radiotherapy treatment line that is received by the patient.";
										dcterms:modified "2020-10-20"^^xsd:date;
										dcterms:creator <https://www.tib.eu/en/research-development/scientific-data-management/staff/samaneh-jozashoori/>.

clarify:hasOncologicalSurgery	rdf:type        owl:ObjectProperty;	
											rdfs:label	"hasOncologicalSurgery";
											rdfs:domain	clarify:LCPatient;
											rdfs:range	clarify:OncologicalSurgery;
											rdfs:comment "A relation between each oncological surgery observation and related data.";
											dcterms:modified "2020-10-20"^^xsd:date;
											dcterms:creator <https://www.tib.eu/en/research-development/scientific-data-management/staff/samaneh-jozashoori/>.	

clarify:hasFamilyHistory	rdf:type        owl:ObjectProperty;	
							rdfs:label	"hasFamilyHistory";
							rdfs:domain	clarify:CancerPatient;
							rdfs:range	clarify:FamilyHistory;
							rdfs:comment "Connection between patient and her/his family history.";
							dcterms:modified "2020-11-16"^^xsd:date;
							dcterms:creator <https://www.tib.eu/en/research-development/scientific-data-management/staff/samaneh-jozashoori/>.

clarify:hasDrug	rdf:type        owl:ObjectProperty;	
				rdfs:label	"hasDrug";
				rdfs:domain	clarify:OncologicalTreatmentLine;
				rdfs:range	clarify:Drug;
				rdfs:comment "A relation between the oncological treatment line and the prescribed drug.";
				dcterms:modified "2020-10-20"^^xsd:date;
				dcterms:creator <https://www.tib.eu/en/research-development/scientific-data-management/staff/samaneh-jozashoori/>.													

clarify:hasComorbidity	rdf:type        owl:ObjectProperty;	
						rdfs:label	"hasComorbidity";
						rdfs:domain	clarify:CancerPatient;
						rdfs:range	clarify:Disorder;
						rdfs:comment	"Connection between patient and her/his Comorbidities.";
						dcterms:modified "2020-10-21"^^xsd:date;
						dcterms:creator <https://www.tib.eu/en/research-development/scientific-data-management/staff/samaneh-jozashoori/>.

clarify:hasTreatmentLineSymptom	rdf:type        owl:ObjectProperty;	
								rdfs:label	"hasTreatmentLineSymptom";
								rdfs:domain	clarify:ComorbidityTreatmentLine;
								rdfs:range	clarify:Disorder;
								rdfs:comment	"Connection between the ComorbidityTreatmentLine and the observed Comorbidities.";
								dcterms:modified "2021-06-22"^^xsd:date;
								dcterms:creator <https://www.tib.eu/en/research-development/scientific-data-management/staff/samaneh-jozashoori/>.

clarify:hasNonOncologicalConsultation	rdf:type        owl:ObjectProperty;	
						rdfs:label	"hasNonOncologicalConsultation";
						rdfs:domain	clarify:CancerPatient;
						rdfs:range	clarify:NonOncologicalConsultation;
						rdfs:comment	"Connection between patient and her/his non-oncological consultation that have had.";
						dcterms:modified "2020-11-17"^^xsd:date;
						dcterms:creator <https://www.tib.eu/en/research-development/scientific-data-management/staff/samaneh-jozashoori/>.

clarify:hasPrediagnosis	rdf:type        owl:ObjectProperty;	
						rdfs:label	"hasPrediagnosis";
						rdfs:domain	clarify:CancerPatient;
						rdfs:range	clarify:Prediagnosis;
						rdfs:comment	"Connection between patient and her/his prediagnosis observation.";
						dcterms:modified "2020-11-17"^^xsd:date;
						dcterms:creator <https://www.tib.eu/en/research-development/scientific-data-management/staff/samaneh-jozashoori/>.

clarify:hasMontoring	rdf:type        owl:ObjectProperty;	
						rdfs:label	"hasMontoring";
						rdfs:domain	clarify:CancerPatient;
						rdfs:range	clarify:StatusEvolution;
						rdfs:comment	"Connection between patient and srvival observation.";
						dcterms:modified "2020-10-21"^^xsd:date;
						dcterms:creator <https://www.tib.eu/en/research-development/scientific-data-management/staff/samaneh-jozashoori/>.		

clarify:hasTumorHistology	rdf:type        owl:ObjectProperty;	
						rdfs:label	"hasTumorHistology";
						rdfs:domain	clarify:CancerPatient;
						rdfs:range	clarify:TumorType;
						rdfs:comment	"Connection between patient and the tumor histology (type).";
						dcterms:modified "2020-10-21"^^xsd:date;
						dcterms:creator <https://www.tib.eu/en/research-development/scientific-data-management/staff/samaneh-jozashoori/>.										

clarify:hasTreatmentLineMaintenance	rdf:type	owl:ObjectProperty;
									rdfs:label	"hasTreatmentLineMaintenance";
									rdfs:domain	clarify:OncologicalTreatmentLine;
									rdfs:range	clarify:Drug;
									rdfs:comment "Represents the type of drugs that are prescribed for the maintenance.";
									dcterms:modified "2021-02-18"^^xsd:date;														
									dcterms:creator <https://www.tib.eu/en/research-development/scientific-data-management/staff/samaneh-jozashoori/>.



clarify:treatmentLineCycle	rdf:type	owl:ObjectProperty;
							rdfs:label	"treatmentLineCycle";
							rdfs:domain	clarify:OncologicalTreatmentLine;
							rdfs:range	clarify:TreatmentLineCycle;
							rdfs:comment "Represents the number of cycles through which the corresponding drugs have been applied.";
							dcterms:modified "2021-02-25"^^xsd:date;														
							dcterms:creator <https://www.tib.eu/en/research-development/scientific-data-management/staff/samaneh-jozashoori/>.

clarify:familyType	rdf:type	owl:ObjectProperty;
					rdfs:label	"familyType";
					rdfs:domain	clarify:FamilyHistory;
					rdfs:range	clarify:FamilyType;
					rdfs:comment "Represents the type of family kinship with the patient.";
					dcterms:modified "2021-02-25"^^xsd:date;							
					dcterms:creator <https://www.tib.eu/en/research-development/scientific-data-management/staff/samaneh-jozashoori/>.

clarify:familyRelationDegree	rdf:type	owl:ObjectProperty;
								rdfs:label	"familyRelationDegree";
								rdfs:domain	clarify:FamilyHistory;
								rdfs:range	clarify:FamilyRelationDegree;
								rdfs:comment "Represents the relative degree of the family member with the patient.";
								dcterms:modified "2021-07-26"^^xsd:date;							
								dcterms:creator <https://www.tib.eu/en/research-development/scientific-data-management/staff/samaneh-jozashoori/>.

clarify:placeOfDeath	rdf:type owl:ObjectProperty;	
						rdfs:label	"placeOfDeath";
						rdfs:domain	clarify:StatusEvolution;
						rdfs:range	clarify:PlaceOfDeath;
						rdfs:comment "The place where the patient died.";
						dcterms:modified "2021-02-25"^^xsd:date;
						dcterms:creator <https://www.tib.eu/en/research-development/scientific-data-management/staff/samaneh-jozashoori/>.

clarify:hasTestResult	rdf:type owl:ObjectProperty;	
							rdfs:label	"hasTestResult";
							rdfs:domain	clarify:Concept;
							rdfs:range	clarify:BiomarkerTestResult;
							rdfs:comment "Indicates a positive test result.";
							dcterms:modified "2021-02-25"^^xsd:date;
							dcterms:creator <https://www.tib.eu/en/research-development/scientific-data-management/staff/samaneh-jozashoori/>.

clarify:hasTestIHQResult	rdf:type owl:ObjectProperty;	
							rdfs:label	"hasTestIHQResult";
							rdfs:domain	clarify:Biomarker;
							rdfs:range	clarify:BiomarkerTestResult;
							rdfs:comment	"Indicates a positive results of the Test IHQ.";
							dcterms:modified "2021-03-02"^^xsd:date;
							dcterms:creator <https://www.tib.eu/en/research-development/scientific-data-management/staff/samaneh-jozashoori/>.

clarify:hasTestFISHResult	rdf:type owl:ObjectProperty;	
							rdfs:label	"hasTestFISHResult";
							rdfs:domain	clarify:Biomarker;
							rdfs:range	clarify:BiomarkerTestResult;
							rdfs:comment	"Indicates a positive results of the Test FISH.";
							dcterms:modified "2021-03-02"^^xsd:date;
							dcterms:creator <https://www.tib.eu/en/research-development/scientific-data-management/staff/samaneh-jozashoori/>.

clarify:hasTestRNAResult	rdf:type owl:ObjectProperty;	
							rdfs:label	"hasTestRNAResult";
							rdfs:domain	clarify:Biomarker;
							rdfs:range	clarify:BiomarkerTestResult;
							rdfs:comment	"Indicates a positive results of the Test RNA.";
							dcterms:modified "2021-03-02"^^xsd:date;
							dcterms:creator <https://www.tib.eu/en/research-development/scientific-data-management/staff/samaneh-jozashoori/>.

clarify:hasBestResponse	rdf:type owl:ObjectProperty;	
						rdfs:label	"hasBestResponse";
						rdfs:domain	clarify:OncologicalTreatmentLine;
						rdfs:range	clarify:TreatementLineBestResponse;
						rdfs:comment	"Indicates the best response in the treatment line of a oncological.";
						dcterms:modified "2021-02-25"^^xsd:date;
						dcterms:creator <https://www.tib.eu/en/research-development/scientific-data-management/staff/samaneh-jozashoori/>.

clarify:hasType	rdf:type owl:ObjectProperty;	
				rdfs:label	"hasType";
				rdfs:domain	clarify:Concept;
				rdfs:range	clarify:Concept;
				rdfs:comment	"Indicates the type of the oncological treatment.";
				dcterms:modified "2021-02-25"^^xsd:date;
				dcterms:creator <https://www.tib.eu/en/research-development/scientific-data-management/staff/samaneh-jozashoori/>.

clarify:is_directed_OrNot	rdf:type owl:ObjectProperty;	
							rdfs:label	"is_directed_OrNot";
							rdfs:domain	clarify:ClinicalTrial;
							rdfs:range	clarify:TrialType;
							rdfs:comment	"Indicates if the trial is direct or not.";
							dcterms:modified "2021-02-25"^^xsd:date;
							dcterms:creator <https://www.tib.eu/en/research-development/scientific-data-management/staff/samaneh-jozashoori/>.

clarify:hasPhase	rdf:type owl:ObjectProperty;	
					rdfs:label	"hasPhase";
					rdfs:domain	clarify:ClinicalTrial;
					rdfs:range	clarify:TrialPhase;
					rdfs:comment	"Indicates the phase of a clinical trial.";
					dcterms:modified "2021-02-25"^^xsd:date;
					dcterms:creator <https://www.tib.eu/en/research-development/scientific-data-management/staff/samaneh-jozashoori/>.

clarify:has_mutation_T790M_positive_result	rdf:type owl:ObjectProperty;	
											rdfs:label	"has_mutation_T790M_positive_result";
											rdfs:domain	clarify:Biomarker;
											rdfs:range	clarify:BiomarkerTestResult;
											rdfs:comment	"Indicates a positive result of the mutation EGFR T790M.";
											dcterms:modified "2021-03-02"^^xsd:date;
											dcterms:creator <https://www.tib.eu/en/research-development/scientific-data-management/staff/samaneh-jozashoori/>.

clarify:has_mutation_T790M_negative_result	rdf:type owl:ObjectProperty;	
											rdfs:label	"has_mutation_T790M_negative_result";
											rdfs:domain	clarify:Biomarker;
											rdfs:range	clarify:BiomarkerTestResult;
											rdfs:comment	"Indicates a negative result of the mutation EGFR T790M.";
											dcterms:modified "2021-03-02"^^xsd:date;
											dcterms:creator <https://www.tib.eu/en/research-development/scientific-data-management/staff/samaneh-jozashoori/>.

clarify:has_mutation_exon19_result	rdf:type owl:ObjectProperty;	
									rdfs:label	"has_mutation_exon19_result";
									rdfs:domain	clarify:Biomarker;
									rdfs:range	clarify:BiomarkerTestResult;
									rdfs:comment	"Indicates a positive result of the mutation EGFR in exon19.";
									dcterms:modified "2021-03-02"^^xsd:date;
									dcterms:creator <https://www.tib.eu/en/research-development/scientific-data-management/staff/samaneh-jozashoori/>.

clarify:has_mutation_exon21_result	rdf:type owl:ObjectProperty;	
									rdfs:label	"has_mutation_exon21_result";
									rdfs:domain	clarify:Biomarker;
									rdfs:range	clarify:BiomarkerTestResult;
									rdfs:comment	"Indicates a positive result of the mutation EGFR in exon21.";
									dcterms:modified "2021-03-02"^^xsd:date;
									dcterms:creator <https://www.tib.eu/en/research-development/scientific-data-management/staff/samaneh-jozashoori/>.

clarify:has_performed_study	rdf:type owl:ObjectProperty;	
							rdfs:label	"has_performed_study";
							rdfs:domain	clarify:Biomarker;
							rdfs:range	clarify:PerformedStudyStatus;
							rdfs:comment	"Connect the biomarker to the indication of performed study.";
							dcterms:modified "2021-04-07"^^xsd:date;
							dcterms:creator <https://www.tib.eu/en/research-development/scientific-data-management/staff/samaneh-jozashoori/>.

clarify:hasNegativeTestResult	rdf:type owl:ObjectProperty;	
								rdfs:label	"hasNegativeTestResult";
								rdfs:domain	clarify:Biomarker;
								rdfs:range	clarify:BiomarkerTestResult;
								rdfs:comment	"Indicates a negative result.";
								dcterms:modified "2021-03-02"^^xsd:date;
								dcterms:creator <https://www.tib.eu/en/research-development/scientific-data-management/staff/samaneh-jozashoori/>.

clarify:has_familyWithCancer_OrNot	rdf:type owl:ObjectProperty;	
									rdfs:label	"has_familyWithCancer_OrNot";
									rdfs:domain	clarify:CancerPatient;
									rdfs:range	clarify:FamilyWithCancer;
									rdfs:comment "Indicates if the patient has a family with cancer or not.";
									dcterms:modified "2021-02-25"^^xsd:date;
									dcterms:creator <https://www.tib.eu/en/research-development/scientific-data-management/staff/samaneh-jozashoori/>.

clarify:hasFamilyCancerType	rdf:type owl:ObjectProperty;	
							rdfs:label	"hasFamilyCancerType";
							rdfs:domain	clarify:CancerPatient;
							rdfs:range	clarify:CancerType;
							rdfs:comment "Indicates the type of cancer of the relatives.";
							dcterms:modified "2021-02-25"^^xsd:date;
							dcterms:creator <https://www.tib.eu/en/research-development/scientific-data-management/staff/samaneh-jozashoori/>.

clarify:hasSymptom	rdf:type owl:ObjectProperty;	
					rdfs:label	"hasSymptom";
					rdfs:domain	clarify:Concept;
					rdfs:range	clarify:Phenotype;
					rdfs:comment	"Indicates the symptoms that a person had.";
					dcterms:modified "2021-02-25"^^xsd:date;
					dcterms:creator <https://www.tib.eu/en/research-development/scientific-data-management/staff/samaneh-jozashoori/>.

clarify:patient_is_asymptomatic	rdf:type owl:ObjectProperty;	
								rdfs:label	"patient_is_asymptomatic";
								rdfs:domain	clarify:Observation;
								rdfs:range	clarify:Phenotype;
								rdfs:comment	"Indicates if the patient had no symptom before the first consultation in Oncology.";
								dcterms:modified "2021-02-25"^^xsd:date;
								dcterms:creator <https://www.tib.eu/en/research-development/scientific-data-management/staff/samaneh-jozashoori/>.

clarify:has_cancer_metastasized_to	rdf:type owl:ObjectProperty;	
									rdfs:label	"has_cancer_metastasized_to";
									rdfs:domain	clarify:CancerPatient;
									rdfs:range	clarify:MetastasisLocation;
									rdfs:comment	"Associates the patient with the location to where the cancer is metastasized.";
									dcterms:modified "2021-02-25"^^xsd:date;
									dcterms:creator <https://www.tib.eu/en/research-development/scientific-data-management/staff/samaneh-jozashoori/>.

clarify:hasReasonOfDeath	rdf:type owl:ObjectProperty;	
							rdfs:label	"hasReasonOfDeath";
							rdfs:domain	clarify:StatusEvolution;
							rdfs:range	clarify:ReasonOfDeath;
							rdfs:comment  "Indicates the reason of the death.";
							dcterms:modified "2021-02-25"^^xsd:date;
							dcterms:creator <https://www.tib.eu/en/research-development/scientific-data-management/staff/samaneh-jozashoori/>.

clarify:hasCurrentStatus	rdf:type owl:ObjectProperty;	
							rdfs:label	"hasCurrentStatus";
							rdfs:domain	clarify:StatusEvolution;
							rdfs:range	clarify:CurrentStatus;
							rdfs:comment	"Indicates the current status of Lung Cancer patient.";
							dcterms:modified "2021-02-25"^^xsd:date;
							dcterms:creator <https://www.tib.eu/en/research-development/scientific-data-management/staff/samaneh-jozashoori/>.

clarify:hasCauseOfDeath	rdf:type owl:ObjectProperty;	
						rdfs:label	"hasCauseOfDeath";
						rdfs:domain	clarify:StatusEvolution;
						rdfs:range	clarify:CauseOfDeath;
						rdfs:comment	"Indicates the cause of death, lung cancer or others.";
						dcterms:modified "2021-02-25"^^xsd:date;
						dcterms:creator <https://www.tib.eu/en/research-development/scientific-data-management/staff/samaneh-jozashoori/>.

clarify:has_previousCancerHistory_OrNot	rdf:type owl:ObjectProperty;	
										rdfs:label	"has_previousCancerHistory_OrNot";
										rdfs:domain	clarify:CancerPatient;
										rdfs:range	clarify:PatientCancerHistory;
										rdfs:comment "Indicates if the patient has previous cancer history or not.";
										dcterms:modified "2021-02-25"^^xsd:date;
										dcterms:creator <https://www.tib.eu/en/research-development/scientific-data-management/staff/samaneh-jozashoori/>.

clarify:hasPreviousCancerType	rdf:type owl:ObjectProperty;	
								rdfs:label	"hasPreviousCancerType";
								rdfs:domain	clarify:CancerPatient;
								rdfs:range	clarify:CancerType;
								rdfs:comment "Indicates whicht type of previous cancer.";
								dcterms:modified "2021-02-25"^^xsd:date;
								dcterms:creator <https://www.tib.eu/en/research-development/scientific-data-management/staff/samaneh-jozashoori/>.

clarify:hasCurrentCancerType	rdf:type	owl:ObjectProperty;
								rdfs:label	"hasCurrentCancerType";
								rdfs:domain	clarify:CancerPatient;
								rdfs:range	clarify:CancerType;
								rdfs:comment	"Indicates the cancer type of the patient.";
								dcterms:modified "2021-02-25"^^xsd:date;								
								dcterms:creator <https://www.tib.eu/en/research-development/scientific-data-management/staff/samaneh-jozashoori/>.

clarify:locatedInHospital	rdf:type	owl:ObjectProperty;
							rdfs:label	"locatedInHospital";
							rdfs:domain	clarify:CancerPatient;
							rdfs:range	clarify:Hospital;
							rdfs:comment	"Represents the hospital where the patient is assigned.";
							dcterms:modified "2021-02-25"^^xsd:date;							
							dcterms:creator <https://www.tib.eu/en/research-development/scientific-data-management/staff/samaneh-jozashoori/>.

clarify:locatedInCity	rdf:type	owl:ObjectProperty;
						rdfs:label	"locatedInCity";
						rdfs:domain	clarify:CancerPatient;
						rdfs:range	clarify:City;
						rdfs:comment	"Represents the city where the patient is assigned.";
						dcterms:modified "2021-02-25"^^xsd:date;							
						dcterms:creator <https://www.tib.eu/en/research-development/scientific-data-management/staff/samaneh-jozashoori/>.

clarify:is_located_in	rdf:type	owl:ObjectProperty;
						rdfs:label	"is_located_in";
						rdfs:domain	clarify:RadiotherapyTreatmentLine;
						rdfs:range	clarify:RadiotherapyLocation;
						rdfs:comment	"indicates the irradiated area during radiotherapy.";
						dcterms:modified "2021-02-25"^^xsd:date;							
						dcterms:creator <https://www.tib.eu/en/research-development/scientific-data-management/staff/samaneh-jozashoori/>.

clarify:hasIntention	rdf:type	owl:ObjectProperty;
						rdfs:label	"hasIntention";
						rdfs:domain	clarify:RadiotherapyTreatmentLine;
						rdfs:range	clarify:RadiotherapyIntention;
						rdfs:comment	"Indicates the intention of the radiotherapy.";
						dcterms:modified "2021-02-25"^^xsd:date;							
						dcterms:creator <https://www.tib.eu/en/research-development/scientific-data-management/staff/samaneh-jozashoori/>.

clarify:hasProgressionRelapse	rdf:type	owl:ObjectProperty;
								rdfs:label	"hasProgressionRelapse";
								rdfs:domain	clarify:CancerPatient;
								rdfs:range	clarify:ProgressionRelapse;
								rdfs:comment	"Specifies which of progression or relapse occured.";
								dcterms:modified "2021-05-11"^^xsd:date;							
								dcterms:creator <https://www.tib.eu/en/research-development/scientific-data-management/staff/samaneh-jozashoori/>.

clarify:hasProgressionOrRelapse	rdf:type	owl:ObjectProperty;
								rdfs:label	"hasProgressionOrRelapse";
								rdfs:domain	clarify:CancerPatient;
								rdfs:range	clarify:ProgressionRelapse;
								rdfs:comment	"Specifies that either of progression or relapse exists.";
								dcterms:modified "2021-05-17"^^xsd:date;							
								dcterms:creator <https://www.tib.eu/en/research-development/scientific-data-management/staff/samaneh-jozashoori/>.

clarify:hasTherapyType	rdf:type	owl:ObjectProperty;
						rdfs:label	"hasTherapyType";
						rdfs:domain	clarify:CancerPatient;
						rdfs:range	clarify:TherapyType;
						rdfs:comment	"Type of therapy.";
						dcterms:modified "2021-02-25"^^xsd:date;							
						dcterms:creator <https://www.tib.eu/en/research-development/scientific-data-management/staff/samaneh-jozashoori/>.

clarify:hasProgressionType	rdf:type	owl:ObjectProperty;
							rdfs:label	"hasProgressionType";
							rdfs:domain	clarify:CancerPatient;
							rdfs:range	clarify:ProgressionType;
							rdfs:comment	"Indicates the type of therapy at progression .";
							dcterms:modified "2021-02-25"^^xsd:date;							
							dcterms:creator <https://www.tib.eu/en/research-development/scientific-data-management/staff/samaneh-jozashoori/>.

clarify:hasTreatmentLineNumber	rdf:type	owl:ObjectProperty;
							rdfs:label	"hasProgressionType";
							rdfs:domain	clarify:Concept;
							rdfs:range	clarify:TreatmentLineNumber;
							rdfs:comment	"Indicates the type of patient.";
							dcterms:modified "2021-02-25"^^xsd:date;							
							dcterms:creator <https://www.tib.eu/en/research-development/scientific-data-management/staff/samaneh-jozashoori/>.

clarify:livedWithSmoker_OrNot	rdf:type	owl:ObjectProperty;
								rdfs:label	"livedWithSmoker_OrNot";
								rdfs:domain	clarify:CancerPatient;
								rdfs:range	clarify:SmokerFamily;
								rdfs:comment	"Indicates if the person has lived with smokers (last 20 years).";
								dcterms:modified "2021-02-25"^^xsd:date;								
								dcterms:creator <https://www.tib.eu/en/research-development/scientific-data-management/staff/samaneh-jozashoori/>.

clarify:livingWithSmoker_OrNot	rdf:type	owl:ObjectProperty;
								rdfs:label	"livingWithSmoker_OrNot";
								rdfs:domain	clarify:CancerPatient;
								rdfs:range	clarify:SmokerFamily;
								rdfs:comment	"Indicates if the person live with smokers.";
								dcterms:modified "2021-02-25"^^xsd:date;								
								dcterms:creator <https://www.tib.eu/en/research-development/scientific-data-management/staff/samaneh-jozashoori/>.

clarify:hasSmokingHabit	rdf:type	owl:ObjectProperty;
						rdfs:label	"hasSmokingHabit";
						rdfs:domain	clarify:CancerPatient;
						rdfs:range	clarify:SmokingHabit;
						rdfs:comment	"Indicates the patient's smoking habit.";
						dcterms:modified "2021-06-05"^^xsd:date;								
						dcterms:creator <https://www.tib.eu/en/research-development/scientific-data-management/staff/samaneh-jozashoori/>.

clarify:performedMonitoring_OrNot	rdf:type	owl:ObjectProperty;
									rdfs:label	"performedMonitoring_OrNot";
									rdfs:domain	clarify:StatusEvolution;
									rdfs:range	clarify:PerformedMonitoring;
									rdfs:comment	"Indicates if the monitoring has been performed on the patient.";
									dcterms:modified "2021-04-29"^^xsd:date;								
									dcterms:creator <https://www.tib.eu/en/research-development/scientific-data-management/staff/samaneh-jozashoori/>.

clarify:hasPathologicalResponse	rdf:type	owl:ObjectProperty;
								rdfs:label	"hasPathologicalResponse";
								rdfs:domain	clarify:OncologicalSurgery;
								rdfs:range	clarify:SurgeryPathologicalResponse;
								rdfs:comment	"Indicates the pathologic response of the patient.";
								dcterms:modified "2021-02-25"^^xsd:date;							
								dcterms:creator <https://www.tib.eu/en/research-development/scientific-data-management/staff/samaneh-jozashoori/>.

clarify:hasClass	rdf:type	owl:ObjectProperty;
					rdfs:label	"hasClass";
					rdfs:domain	clarify:OncologicalSurgery;
					rdfs:range	clarify:SurgeryClass;
					rdfs:comment	"Indicates the class of the surgery.";
					dcterms:modified "2021-02-25"^^xsd:date;							
					dcterms:creator <https://www.tib.eu/en/research-development/scientific-data-management/staff/samaneh-jozashoori/>.

clarify:hasSubType	rdf:type	owl:ObjectProperty;
					rdfs:label	"hasSubType";
					rdfs:domain	clarify:OncologicalSurgery;
					rdfs:range	clarify:SurgerySubType;
					rdfs:comment	"Is the subtype of procedure follow in in a surgery.";
					dcterms:modified "2021-02-25"^^xsd:date;							
					dcterms:creator <https://www.tib.eu/en/research-development/scientific-data-management/staff/samaneh-jozashoori/>.

clarify:has_PerioperativeDeath_orNot	rdf:type	owl:ObjectProperty;
										rdfs:label	"has_PerioperativeDeath_orNot";
										rdfs:domain	clarify:OncologicalSurgery;
										rdfs:range	clarify:PerioperativeDeath;
										rdfs:comment "Indicates if the perioperative death was the cause of death (30 days after surgery).";
										dcterms:modified "2021-02-25"^^xsd:date;							
										dcterms:creator <https://www.tib.eu/en/research-development/scientific-data-management/staff/samaneh-jozashoori/>.

clarify:cancerStageTNM_TumorSize	rdf:type	owl:ObjectProperty;
									rdfs:label	"cancerStageTNM_TumorSize";
									rdfs:domain	clarify:CancerPatient;
									rdfs:range	clarify:TumorSize;
									rdfs:comment "Associates the cancer stage (based on on TNM system) of the patient with the size of the primary tumor, based on which the cancer stage is evaluated.";
									dcterms:modified "2021-05-11"^^xsd:date;							
									dcterms:creator <https://www.tib.eu/en/research-development/scientific-data-management/staff/samaneh-jozashoori/>.

clarify:cancerStageTNM_LymphNodesInvolvement	rdf:type	owl:ObjectProperty;
												rdfs:label	"cancerStageTNM_LymphNodesInvolvement";
												rdfs:domain	clarify:CancerPatient;
												rdfs:range	clarify:LymphNodesInvolvement;
												rdfs:comment "Associates the cancer stage (based on on TNM system) of the patient with the involvement of lymph nodes, based on which the cancer stage is evaluated.";
												dcterms:modified "2021-05-11"^^xsd:date;							
												dcterms:creator <https://www.tib.eu/en/research-development/scientific-data-management/staff/samaneh-jozashoori/>.

clarify:cancerStageTNM_MetastatisStage	rdf:type	owl:ObjectProperty;
										rdfs:label	"cancerStageTNM_MetastatisStage";
										rdfs:domain	clarify:CancerPatient;
										rdfs:range	clarify:MetastatisStage;
										rdfs:comment "Associates the cancer stage (based on on TNM system) of the patient with the metasta stage, based on which the cancer stage is evaluated.";
										dcterms:modified "2021-05-11"^^xsd:date;								
										dcterms:creator <https://www.tib.eu/en/research-development/scientific-data-management/staff/samaneh-jozashoori/>.

clarify:cancerStageTNM_Version	rdf:type	owl:ObjectProperty;
								rdfs:label	"cancerStageTNM_Version";
								rdfs:domain	clarify:Concept;
								rdfs:range	clarify:Version;
								rdfs:comment "Associates the concept with the version, based on which the concept value is provided.";
								dcterms:modified "2021-04-26"^^xsd:date;								
								dcterms:creator <https://www.tib.eu/en/research-development/scientific-data-management/staff/samaneh-jozashoori/>.

clarify:basedOn_Scale	rdf:type	owl:ObjectProperty;
						rdfs:label	"basedOn_Scale";
						rdfs:domain	clarify:PerformanceStatusObservation;
						rdfs:range	clarify:Scale;
						rdfs:comment "Associates the performance status observation with the scale that is considered for the assessment.";
						dcterms:modified "2021-03-03"^^xsd:date;								
						dcterms:creator <https://www.tib.eu/en/research-development/scientific-data-management/staff/samaneh-jozashoori/>.

clarify:has_SynchronousTumor_OrNot	rdf:type	owl:ObjectProperty;
									rdfs:label	"has_SynchronousTumor_OrNot";
									rdfs:domain	clarify:CancerPatient;
									rdfs:range	clarify:SynchronousTumor;
									rdfs:comment "indicates if a second primary cancer is diagnosed within 6 months of the primary cancer or not.";
									dcterms:modified "2021-02-25"^^xsd:date;								
									dcterms:creator <https://www.tib.eu/en/research-development/scientific-data-management/staff/samaneh-jozashoori/>.

clarify:hasMesotheliomaType	rdf:type	owl:ObjectProperty;
							rdfs:label	"hasMesotheliomaType";
							rdfs:domain	clarify:TumorType;
							rdfs:range	clarify:MesotheliomaType;
							rdfs:comment	"Associates the tumor type with the related subtype mesothelyoma.";
							dcterms:modified "2021-02-25"^^xsd:date;								
							dcterms:creator <https://www.tib.eu/en/research-development/scientific-data-management/staff/samaneh-jozashoori/>.

clarify:hasAdenocarcinomaHistology	rdf:type	owl:ObjectProperty;
									rdfs:label	"hasAdenocarcinomaHistology";
									rdfs:domain	clarify:TumorType;
									rdfs:range	clarify:AdenocarcinomaHistology;
									rdfs:comment	"Associates the tumor type with the related subtype adenocarcinoma.";
									dcterms:modified "2021-02-25"^^xsd:date;								
									dcterms:creator <https://www.tib.eu/en/research-development/scientific-data-management/staff/samaneh-jozashoori/>.

clarify:hasCarcinomaType	rdf:type	owl:ObjectProperty;
							rdfs:label	"hasCarcinomaType";
							rdfs:domain	clarify:TumorType;
							rdfs:range	clarify:CarcinomaType;
							rdfs:comment	"Associates the tumor type with the details of the type of carcinoma.";
							dcterms:modified "2021-02-25"^^xsd:date;							
							dcterms:creator <https://www.tib.eu/en/research-development/scientific-data-management/staff/samaneh-jozashoori/>.

clarify:hasHistologyDegree	rdf:type	owl:ObjectProperty;
							rdfs:label	"hasHistologyDegree";
							rdfs:domain	clarify:TumorType;
							rdfs:range	clarify:HistologyDegree;
							rdfs:comment	"Associates the tumor type with the related degree of the histology.";
							dcterms:modified "2021-02-25"^^xsd:date;							
							dcterms:creator <https://www.tib.eu/en/research-development/scientific-data-management/staff/samaneh-jozashoori/>.

clarify:hasSmallCellCarcinomaType	rdf:type	owl:ObjectProperty;
									rdfs:label	"hasSmallCellCarcinomaType";
									rdfs:domain	clarify:TumorType;
									rdfs:range	clarify:SmallCellCarcinomaType;
									rdfs:comment	"Associates the tumor type with the subtype small cell lung cancer (microcytic).";
									dcterms:modified "2021-02-25"^^xsd:date;							
									dcterms:creator <https://www.tib.eu/en/research-development/scientific-data-management/staff/samaneh-jozashoori/>.

clarify:hasSecondNeoplasm	rdf:type 	owl:ObjectProperty;	
							rdfs:label	"hasSecondNeoplasm";
							rdfs:domain	clarify:StatusEvolution;
							rdfs:range	clarify:SecondNeoplasm;
							rdfs:comment "Associates the status evolution with the information on secondary malignant neoplasm.";
							dcterms:modified "2021-03-18"^^xsd:date;
							dcterms:creator <https://www.tib.eu/en/research-development/scientific-data-management/staff/samaneh-jozashoori/>.

clarify:has_other_result	rdf:type owl:ObjectProperty;	
							rdfs:label	"has_other_result";
							rdfs:domain	clarify:Biomarker;
							rdfs:range	clarify:BiomarkerTestResult;
							rdfs:comment "Assocaites the Biomarker with the other test results.";
							dcterms:modified "2021-03-18"^^xsd:date;
							dcterms:creator <https://www.tib.eu/en/research-development/scientific-data-management/staff/samaneh-jozashoori/>.

clarify:has_NOS_result	rdf:type owl:ObjectProperty;	
						rdfs:label	"has_NOS_result";
						rdfs:domain	clarify:Biomarker;
						rdfs:range	clarify:BiomarkerTestResult;
						rdfs:comment "Associates the Biomarker with NOS(!) test results.";
						dcterms:modified "2021-03-18"^^xsd:date;
						dcterms:creator <https://www.tib.eu/en/research-development/scientific-data-management/staff/samaneh-jozashoori/>.

clarify:hasClinicalTrialTreatmentLine	rdf:type 	owl:ObjectProperty;	
							rdfs:label	"hasClinicalTrialTreatmentLine";
							rdfs:domain	clarify:CancerPatient;
							rdfs:range	clarify:ClinicalTrialTreatmentLine;
							rdfs:comment "Associates Patient with treatment line of the clinical trial .";
							dcterms:modified "2021-05-17"^^xsd:date;
							dcterms:creator <https://www.tib.eu/en/research-development/scientific-data-management/staff/samaneh-jozashoori/>.

clarify:hasComorbidityStatus	rdf:type 	owl:ObjectProperty;	
								rdfs:label	"hasComorbidityStatus";
								rdfs:domain	clarify:CancerPatient;
								rdfs:range	clarify:ComorbidityStatus;
								rdfs:comment "Associates Patient with the comorbidity status.";
								dcterms:modified "2021-05-17"^^xsd:date;
								dcterms:creator <https://www.tib.eu/en/research-development/scientific-data-management/staff/samaneh-jozashoori/>.

clarify:hasSecondNeoplasmType	rdf:type 	owl:ObjectProperty;	
								rdfs:label	"hasSecondNeoplasmType";
								rdfs:domain	clarify:StatusEvolution;
								rdfs:range	clarify:hasSecondNeoplasmType;
								rdfs:comment "Associates Patient with second neoplasm type.";
								dcterms:modified "2021-05-17"^^xsd:date;
								dcterms:creator <https://www.tib.eu/en/research-development/scientific-data-management/staff/samaneh-jozashoori/>.

clarify:hasPerformanceStatus	rdf:type 	owl:ObjectProperty;	
								rdfs:label	"hasPerformanceStatus";
								rdfs:domain	clarify:CancerPatient;
								rdfs:range	clarify:PerformanceStatus;
								rdfs:comment "Associates Patient with her/his performance status.";
								dcterms:modified "2021-05-17"^^xsd:date;
								dcterms:creator <https://www.tib.eu/en/research-development/scientific-data-management/staff/samaneh-jozashoori/>.

clarify:hasStudiedBiomarker	rdf:type 	owl:ObjectProperty;	
							rdfs:label	"hasStudiedBiomarker";
							rdfs:domain	clarify:CancerPatient;
							rdfs:range	clarify:Biomarker;
							rdfs:comment "Associates Patient with the studied biomarkers.";
							dcterms:modified "2021-05-17"^^xsd:date;
							dcterms:creator <https://www.tib.eu/en/research-development/scientific-data-management/staff/samaneh-jozashoori/>.

clarify:hasBiomarkerTestResult	rdf:type 	owl:ObjectProperty;	
								rdfs:label	"hasBiomarkerTestResult";
								rdfs:domain	clarify:CancerPatient;
								rdfs:range	clarify:BiomarkerTestResult;
								rdfs:comment "Associates Patient with the result of the studied biomarkers.";
								dcterms:modified "2021-05-17"^^xsd:date;
								dcterms:creator <https://www.tib.eu/en/research-development/scientific-data-management/staff/samaneh-jozashoori/>.

clarify:hasSurgeryIteration	rdf:type 	owl:ObjectProperty;	
							rdfs:label	"hasSurgeryIteration";
							rdfs:domain	clarify:SurgerySubType;
							rdfs:range	clarify:SurgeryIteration;
							rdfs:comment "Associates the surgery sub type with the surgery iteration.";
							dcterms:modified "2021-05-17"^^xsd:date;
							dcterms:creator <https://www.tib.eu/en/research-development/scientific-data-management/staff/samaneh-jozashoori/>.

clarify:hasResectionGrade	rdf:type 	owl:ObjectProperty;	
							rdfs:label	"hasResectionGrade";
							rdfs:domain	clarify:OncologicalSurgery;
							rdfs:range	clarify:SurgeryResectionDegree;
							rdfs:comment "Associates the oncological surgery with the surgery resection degree.";
							dcterms:modified "2021-05-17"^^xsd:date;
							dcterms:creator <https://www.tib.eu/en/research-development/scientific-data-management/staff/samaneh-jozashoori/>.

######################################################################################################################################
#####################################################    Publication    ##############################################################
######################################################################################################################################

clarify:hasAnnotation	rdf:type owl:ObjectProperty;
						rdfs:label	"hasAnnotation";
						rdfs:domain clarify:Relation;
		  				rdfs:range clarify:Annotation;
						rdfs:comment	"Connection between the annotation and the relation between annotation and publication";
						dcterms:modified "2020-12-15"^^xsd:date;
						dcterms:creator <https://www.tib.eu/en/research-development/scientific-data-management/staff/samaneh-jozashoori/>.

clarify:annotates	rdf:type	owl:ObjectProperty;
					rdfs:label	"annotates";
					rdfs:domain	clarify:Relation;
					rdfs:range	clarify:Publication;
					rdfs:comment	"Connection between mentionedIn or HasTopic relation with CUI.";
					dcterms:modified "2020-12-15"^^xsd:date;
					dcterms:creator <https://www.tib.eu/en/research-development/scientific-data-management/staff/samaneh-jozashoori/>.

clarify:relation_isRelatedTo_annotation	rdf:type        owl:ObjectProperty;	
										rdfs:label	"relation_isRelatedTo_annotation";
										rdfs:domain	clarify:Relation;
										rdfs:range	clarify:Annotation;
										rdfs:comment "The relationship between the relation and the annotation.";
										dcterms:modified "2020-12-15"^^xsd:date;
										dcterms:creator <https://www.tib.eu/en/research-development/scientific-data-management/staff/samaneh-jozashoori/>.

clarify:relation_isRelatedTo_publication	rdf:type        owl:ObjectProperty;	
											rdfs:label	"relation_isRelatedTo_publication";
											rdfs:domain	clarify:Relation;
											rdfs:range	clarify:Publication;
											rdfs:comment "The relationship between the relation and the publication.";
											dcterms:modified "2020-12-15"^^xsd:date;
											dcterms:creator <https://www.tib.eu/en/research-development/scientific-data-management/staff/samaneh-jozashoori/>.				

clarify:hasAuthor	rdf:type owl:ObjectProperty;
					rdfs:label "hasAuthor";
					rdfs:domain clarify:Publication;
				  	rdfs:range clarify:Author;
					rdfs:comment "Author of Publication.";
					dcterms:modified "2021-05-17"^^xsd:date;
					dcterms:creator <https://www.tib.eu/en/research-development/scientific-data-management/staff/samaneh-jozashoori/>.

clarify:hasPublicationType	rdf:type owl:ObjectProperty;
					rdfs:label "hasPublicationType";
					rdfs:domain clarify:Publication;
				  	rdfs:range clarify:PublicationType;
					rdfs:comment "The publication type.";
					dcterms:modified "2021-06-08"^^xsd:date;
					dcterms:creator <https://www.tib.eu/en/research-development/scientific-data-management/staff/samaneh-jozashoori/>.

######################################################################################################################################
#########################################################    Drug    #################################################################
######################################################################################################################################

clarify:semanticTypeID	rdf:type	owl:ObjectProperty;
						rdfs:label	"semanticTypeID";
						rdfs:domain	clarify:Annotation;
						rdfs:range	clarify:SemanticType;
		                rdfs:comment "The semantic type id provided by UMLS.";
						dcterms:modified "2019-12-15"^^xsd:date;				
						dcterms:creator <https://www.tib.eu/en/research-development/scientific-data-management/staff/samaneh-jozashoori/>.

clarify:semanticTypeGroupID	rdf:type	owl:ObjectProperty;
							rdfs:label	"semanticTypeGroupID";
							rdfs:domain	clarify:SemanticType;
							rdfs:range	clarify:SemanticTypeGroup;
			                rdfs:comment "The semantic type group id provided by UMLS.";
							dcterms:modified "2021-07-21"^^xsd:date;
							dcterms:creator <https://www.tib.eu/en/research-development/scientific-data-management/staff/samaneh-jozashoori/>.

clarify:biomarker_has_indication	rdf:type	owl:ObjectProperty;
								rdfs:label	"biomarker_has_indication";
								rdfs:domain	clarify:Biomarker;
								rdfs:range	clarify:Drug;
								rdfs:comment	"A biomarker has indication Drug";
								dcterms:modified "2020-12-15"^^xsd:date;
								dcterms:creator <https://www.tib.eu/en/research-development/scientific-data-management/staff/samaneh-jozashoori/>.

clarify:interactor1	rdf:type owl:ObjectProperty;
					rdfs:label "interactor1";
					rdfs:domain clarify:Interaction;
				  	rdfs:range clarify:Drug;
					rdfs:comment "Interactor 1";
					dcterms:modified "2020-12-15"^^xsd:date;
					dcterms:creator <https://www.tib.eu/en/research-development/scientific-data-management/staff/samaneh-jozashoori/>.

clarify:interactor2	rdf:type owl:ObjectProperty;
					rdfs:label "interactor2";
					rdfs:domain clarify:Interaction;
				  	rdfs:range clarify:Concept;
					rdfs:comment "Interactor 2";
					dcterms:modified "2020-12-15"^^xsd:date;
					dcterms:creator <https://www.tib.eu/en/research-development/scientific-data-management/staff/samaneh-jozashoori/>.

clarify:drug_isRelatedTo_dse	rdf:type	owl:ObjectProperty;
							rdfs:label	"drug_isRelatedTo_dse";
							rdfs:domain	clarify:Drug;
							rdfs:range	clarify:DrugSideEffect;
							rdfs:comment	"relationship between drug and drug-sideEffect relation.";
							dcterms:modified "2020-12-15"^^xsd:date;
							dcterms:creator <https://www.tib.eu/en/research-development/scientific-data-management/staff/samaneh-jozashoori/>.

clarify:sideEffect_isRelatedTo_dse	rdf:type	owl:ObjectProperty;
									rdfs:label	"sideEffect_isRelatedTo_dse";
									rdfs:domain	clarify:Phenotype;
									rdfs:range	clarify:DrugSideEffect;
									rdfs:comment	"relationship between sideEffect and drug-sideEffect relation.";
									dcterms:modified "2020-12-15"^^xsd:date;
									dcterms:creator <https://www.tib.eu/en/research-development/scientific-data-management/staff/samaneh-jozashoori/>.

clarify:enzyme_isRelatedTo_gene	rdf:type	owl:ObjectProperty;
									rdfs:label	"enzyme_isRelatedTo_gene";
									rdfs:domain	clarify:Enzyme;
									rdfs:range	clarify:Gene;
									rdfs:comment	"The relationship between the enzyme and the gene from which it is produced.";
									dcterms:modified "2020-09-14"^^xsd:date;
									dcterms:creator <https://www.tib.eu/en/research-development/scientific-data-management/staff/samaneh-jozashoori/>.

clarify:affects	rdf:type	owl:ObjectProperty;
								rdfs:label	"affects";
								rdfs:domain	clarify:DrugDrugInteraction;
								rdfs:range	clarify:Drug;
								rdfs:comment	"The conncetion between drug that affects by the other one through their interaction and the interaction node.";
								dcterms:modified "2020-12-15"^^xsd:date;
								dcterms:creator <https://www.tib.eu/en/research-development/scientific-data-management/staff/samaneh-jozashoori/>.

clarify:isAffected	rdf:type	owl:ObjectProperty;
								rdfs:label	"isAffected";
								rdfs:domain	clarify:DrugDrugInteraction;
								rdfs:range	clarify:Drug;
								rdfs:comment	"The conncetion between drug that is affected by the other one through their interaction and the interaction node.";
								dcterms:modified "2020-12-15"^^xsd:date;
								dcterms:creator <https://www.tib.eu/en/research-development/scientific-data-management/staff/samaneh-jozashoori/>.

clarify:precipitant_drug	rdf:type	owl:ObjectProperty;
								rdfs:label	"precipitant_drug";
								rdfs:domain	clarify:DrugDrugInteraction;
								rdfs:range	clarify:Drug;
								rdfs:comment	"The relationship between the drug drug interaction and corresponding precipitant drug.";
								dcterms:modified "2020-12-15"^^xsd:date;
								dcterms:creator <https://www.tib.eu/en/research-development/scientific-data-management/staff/samaneh-jozashoori/>.

clarify:precipitant_drug_cui	rdf:type	owl:ObjectProperty;
								rdfs:label	"precipitant_drug_cui";
								rdfs:domain	clarify:DrugDrugInteraction;
								rdfs:range	clarify:Annotation;
								rdfs:comment	"The relationship between the drug drug interaction and corresponding precipitant drug annotated by CUI IDs.";
								dcterms:modified "2021-06-30"^^xsd:date;
								dcterms:creator <https://www.tib.eu/en/research-development/scientific-data-management/staff/samaneh-jozashoori/>.

clarify:object_drug	rdf:type	owl:ObjectProperty;
								rdfs:label	"object_drug";
								rdfs:domain	clarify:DrugDrugInteraction;
								rdfs:range	clarify:Drug;
								rdfs:comment	"The relationship between the drug drug interaction and corresponding object drug .";
								dcterms:modified "2020-12-15"^^xsd:date;
								dcterms:creator <https://www.tib.eu/en/research-development/scientific-data-management/staff/samaneh-jozashoori/>.

clarify:object_drug_cui	rdf:type	owl:ObjectProperty;
								rdfs:label	"object_drug_cui";
								rdfs:domain	clarify:DrugDrugInteraction;
								rdfs:range	clarify:Annotation;
								rdfs:comment	"The relationship between the drug drug interaction and corresponding object drug annotated by CUI IDs.";
								dcterms:modified "2021-06-30"^^xsd:date;
								dcterms:creator <https://www.tib.eu/en/research-development/scientific-data-management/staff/samaneh-jozashoori/>.

clarify:effect	rdf:type	owl:ObjectProperty;
				rdfs:label	"effect";
				rdfs:domain	clarify:DrugDrugInteraction;
				rdfs:range	clarify:AdverseEvent;
				rdfs:comment	"The relationship between the drug drug interaction and corresponding adverse event.";
				dcterms:modified "2020-12-15"^^xsd:date;
				dcterms:creator <https://www.tib.eu/en/research-development/scientific-data-management/staff/samaneh-jozashoori/>.

clarify:impact	rdf:type	owl:ObjectProperty;
				rdfs:label	"impact";
				rdfs:domain	clarify:DrugDrugInteraction;
				rdfs:range	clarify:Impact;
				rdfs:comment	"The relationship between the drug drug interaction and corresponding impact.";
				dcterms:modified "2021-06-30"^^xsd:date;
				dcterms:creator <https://www.tib.eu/en/research-development/scientific-data-management/staff/samaneh-jozashoori/>.

clarify:effect_cui	rdf:type	owl:ObjectProperty;
					rdfs:label	"effect_cui";
					rdfs:domain	clarify:DrugDrugInteraction;
					rdfs:range	clarify:Annotation;
					rdfs:comment	"The relationship between the drug drug interaction and corresponding adverse event annotated by CUI IDs.";
					dcterms:modified "2021-06-30"^^xsd:date;
					dcterms:creator <https://www.tib.eu/en/research-development/scientific-data-management/staff/samaneh-jozashoori/>.

clarify:target_isRelatedTo_gene	rdf:type	owl:ObjectProperty;
									rdfs:label	"target_isRelatedTo_gene";
									rdfs:domain	clarify:Target;
									rdfs:range	clarify:Gene;
									rdfs:comment	"The relationship between the target and the gene from which it is produced.";
									dcterms:modified "2020-12-15"^^xsd:date;
									dcterms:creator <https://www.tib.eu/en/research-development/scientific-data-management/staff/samaneh-jozashoori/>.

clarify:CancerStage_has_indication	rdf:type	owl:ObjectProperty;
									rdfs:label	"CancerStage_has_indication";
									rdfs:domain	clarify:CancerStage;
									rdfs:range	clarify:Drug;
									rdfs:comment	"Tumor stage has indication drug";
									dcterms:modified "2020-09-14"^^xsd:date;
									dcterms:creator <https://www.tib.eu/en/research-development/scientific-data-management/staff/samaneh-jozashoori/>.

clarify:hasHPOAnnotation	rdf:type owl:ObjectProperty;
							rdfs:label	"hasHPOAnnotation";
							rdfs:domain clarify:Phenotype;
			  				rdfs:range clarify:Annotation;
							rdfs:comment	"HPO annotation of the phenotype.";
							dcterms:modified "2020-12-15"^^xsd:date;
							dcterms:creator <https://www.tib.eu/en/research-development/scientific-data-management/staff/samaneh-jozashoori/>.