@prefix clarify: <http://clarify2020.eu/vocab/> .
@prefix owl: <http://www.w3.org/2002/07/owl#> .
@prefix rdf: <http://www.w3.org/1999/02/22-rdf-syntax-ns#> .
@prefix rdfs: <http://www.w3.org/2000/01/rdf-schema#> .
@prefix xsd: <http://www.w3.org/2001/XMLSchema#> .
@prefix dcterms: <http://purl.org/dc/terms/> .
@prefix prv: <http://purl.org/net/provenance/ns#> .

#################################################################################################################################################
#################################################################################################################################################
#################################################################################################################################################
###############################################################   Classes   #####################################################################
#################################################################################################################################################
#################################################################################################################################################
#################################################################################################################################################

clarify:Concept	rdf:type	owl:Class;
				rdfs:label	"Concept";
				rdfs:comment "Constituents of thoughts or real world entities.";
				dcterms:modified "2020-10-19"^^xsd:date;
				dcterms:creator <https://www.tib.eu/en/research-development/scientific-data-management/staff/samaneh-jozashoori/>.

clarify:Annotation	rdf:type	owl:Class;
					rdfs:label	"Annotation";
					rdfs:comment "Annotation of a concept including label, id and source of concept.";
					dcterms:modified "2020-10-19"^^xsd:date;
					dcterms:creator <https://www.tib.eu/en/research-development/scientific-data-management/staff/samaneh-jozashoori/>.

clarify:CancerPatient	rdf:type	owl:Class;
					rdfs:label	"CancerPatient";
					rdfs:comment "Cancer Patient independent of type of their cancer.";
					dcterms:modified "2020-10-19"^^xsd:date;
					dcterms:creator <https://www.tib.eu/en/research-development/scientific-data-management/staff/samaneh-jozashoori/>.

clarify:LCPatient	rdf:type	owl:Class;
				rdfs:label	"LungCancerPatient";
				rdfs:subClassOf	clarify:CancerPatient;
				rdfs:comment "A patient who is diagnosed with Lung Cancer.";
				dcterms:modified "2020-10-19"^^xsd:date;
				prv:File "patient.ttl";				
				dcterms:creator <https://www.tib.eu/en/research-development/scientific-data-management/staff/samaneh-jozashoori/>.

clarify:Diagnosis  	rdf:type owl:Class;
					rdfs:label	"Diagnosis";
					rdfs:subClassOf	clarify:Observation;
					rdfs:comment "The identification of the nature of an illness or other problem by examination of the symptoms.";
					dcterms:modified "2020-09-15"^^xsd:date;
					prv:File "diagnostic.ttl";
					dcterms:creator <https://www.tib.eu/en/research-development/scientific-data-management/staff/samaneh-jozashoori/>.	

clarify:Gender	rdf:type	owl:Class;
						rdfs:label	"Gender";
						rdfs:comment "The gender of patients.";
						dcterms:modified "2020-10-19"^^xsd:date;
						prv:File "patient.ttl";
						dcterms:creator <https://www.tib.eu/en/research-development/scientific-data-management/staff/samaneh-jozashoori/>.

clarify:Race	rdf:type	owl:Class;
						rdfs:label	"Race";
						rdfs:comment "The race of patients.";
						dcterms:modified "2020-10-19"^^xsd:date;
						prv:File "patient.ttl";
						dcterms:creator <https://www.tib.eu/en/research-development/scientific-data-management/staff/samaneh-jozashoori/>.						

clarify:Biomarker	 rdf:type	owl:Class;
					rdfs:label	"Biomarker";
					rdfs:subClassOf	clarify:Concept;
					rdfs:comment "A biomarker, or biological marker is a measurable indicator of some biological state or condition.";
					dcterms:modified "2020-10-19"^^xsd:date;
					dcterms:creator <https://www.tib.eu/en/research-development/scientific-data-management/staff/samaneh-jozashoori/>.

clarify:BiomarkerObservation	 rdf:type	owl:Class;
					rdfs:label	"BiomarkerObservation";
					rdfs:subClassOf	clarify:Observation;
					rdfs:comment "A biomarker, or biological marker is a measurable indicator of some biological state or condition.";
					dcterms:modified "2020-10-19"^^xsd:date;
					dcterms:creator <https://www.tib.eu/en/research-development/scientific-data-management/staff/samaneh-jozashoori/>.

clarify:Carcinogen	 rdf:type	owl:Class;
					rdfs:label	"Carcinogen";
					rdfs:subClassOf	clarify:Concept;
					rdfs:comment "Represents any substance, radionuclide, or radiation that promotes carcinogenesis, the formation of cancer.";
					dcterms:modified "2020-10-20"^^xsd:date;
					dcterms:creator <https://www.tib.eu/en/research-development/scientific-data-management/staff/samaneh-jozashoori/>.					

clarify:ProgressionRelapseObservation	rdf:type	owl:Class;
										rdfs:label	"ProgressionRelapseObservation";
										rdfs:subClassOf	clarify:Observation;
										rdfs:comment "Indicates if the disease is relapsed or progressed.";
										dcterms:modified "2020-10-20"^^xsd:date;
										dcterms:creator <https://www.tib.eu/en/research-development/scientific-data-management/staff/samaneh-jozashoori/>.	

clarify:PatientHistory	rdf:type	owl:Class;
						rdfs:label	"PatientHistory";
						rdfs:subClassOf	clarify:Concept;
						rdfs:comment "Represents the cancers from which the patient have suffered before.";
						dcterms:modified "2020-10-20"^^xsd:date;
						dcterms:creator <https://www.tib.eu/en/research-development/scientific-data-management/staff/samaneh-jozashoori/>.

clarify:FamilyHistory	rdf:type	owl:Class;
						rdfs:label	"FamilyHistory";
						rdfs:subClassOf	clarify:Concept;
						rdfs:comment "Represents the cancers from which the direct blood relatives of the patient have suffered.";
						dcterms:modified "2020-10-20"^^xsd:date;
						dcterms:creator <https://www.tib.eu/en/research-development/scientific-data-management/staff/samaneh-jozashoori/>.	

clarify:ClinicalTrial	 rdf:type	owl:Class;
					rdfs:label	"ClinicalTrial";
					rdfs:subClassOf	clarify:Observation;
					rdfs:comment "Represents the clinical trial that the patient is involved in.";
					dcterms:modified "2020-10-20"^^xsd:date;
					dcterms:creator <https://www.tib.eu/en/research-development/scientific-data-management/staff/samaneh-jozashoori/>.

clarify:CancerStageTNM	 rdf:type	owl:Class;
					rdfs:label	"CancerStageTNM";
					rdfs:subClassOf	clarify:Observation;
					rdfs:comment "Determines a patient's prognosis and the course of treatement to be used for a certain patient based on TNM staging system.";
					dcterms:modified "2020-10-20"^^xsd:date;
					dcterms:creator <https://www.tib.eu/en/research-development/scientific-data-management/staff/samaneh-jozashoori/>.

clarify:CancerStage	 rdf:type	owl:Class;
					rdfs:label	"CancerStage";
					rdfs:subClassOf	clarify:Observation;
					rdfs:comment "Determines a patient's prognosis and the course of treatement to be used for a certain patient, based on a scale of 0 to IV.";
					dcterms:modified "2020-10-20"^^xsd:date;
					dcterms:creator <https://www.tib.eu/en/research-development/scientific-data-management/staff/samaneh-jozashoori/>.

clarify:MetastasisLocation	 rdf:type	owl:Class;
					rdfs:label	"MetastasisLocation";
					rdfs:subClassOf	clarify:Observation;
					rdfs:comment "Determines the area to which the cancer is metastasized.";
					dcterms:modified "2020-10-20"^^xsd:date;
					dcterms:creator <https://www.tib.eu/en/research-development/scientific-data-management/staff/samaneh-jozashoori/>.

clarify:Diagnosis  	rdf:type owl:Class;
					rdfs:label	"Diagnosis";
					rdfs:subClassOf	clarify:Observation;
					rdfs:comment "The identification of the nature of an illness or other problem by examination of the symptoms.";
					dcterms:modified "2020-10-20"^^xsd:date;
					prv:File "diagnostic.ttl";
					dcterms:creator <https://www.tib.eu/en/research-development/scientific-data-management/staff/samaneh-jozashoori/>.		

clarify:OncologicalTreatmentLine	rdf:type	owl:Class;
								rdfs:label	"OncologicalTreatmentLine";
								rdfs:subClassOf clarify:Concept;
								rdfs:comment "Records of patients in clinical notes that are related to oncological treatment lines";
								dcterms:modified "2020-10-20"^^xsd:date;
								dcterms:creator <https://www.tib.eu/en/research-development/scientific-data-management/staff/samaneh-jozashoori/>.

clarify:ChemotherapyTreatmentLine	rdf:type	owl:Class;
								rdfs:label	"ChemotherapyTreatmentLine";
								rdfs:subClassOf clarify:OncologicalTreatmentLine;
								rdfs:comment "Records of patients in clinical notes that are related to chemotherapy treatment lines";
								dcterms:modified "2020-10-20"^^xsd:date;
								prv:File "chemotherapy_treatment_line.ttl";
								dcterms:creator <https://www.tib.eu/en/research-development/scientific-data-management/staff/samaneh-jozashoori/>.

clarify:RadiotherapyTreatmentLine	rdf:type	owl:Class;
								rdfs:label	"RadiotherapyTreatmentLine";
								rdfs:subClassOf clarify:OncologicalTreatmentLine;
								rdfs:comment "Records of patients in clinical notes that are related to radiotherapy treatment lines";
								dcterms:modified "2020-09-15"^^xsd:date;
								prv:File "radiotherapy_treatment_line.ttl";
								dcterms:creator <https://www.tib.eu/en/research-development/scientific-data-management/staff/samaneh-jozashoori/>.	

clarify:OncologicalSurgery	rdf:type	owl:Class;
							rdfs:label	"OncologicalSurgery";
							rdfs:subClassOf clarify:Concept;
							rdfs:comment " Is the branch of surgery applied to oncology; it focuses on the surgical management of tumors, especially cancerous tumors.";
							dcterms:modified "2020-10-20"^^xsd:date;
							prv:File "surgery.ttl";
							dcterms:creator <https://www.tib.eu/en/research-development/scientific-data-management/staff/samaneh-jozashoori/>.																																	

clarify:Drug	rdf:type	owl:Class;
				rdfs:label	"Drug";
				rdfs:subClassOf	clarify:Concept;
				rdfs:comment "A substance used as a medication or in the preparation of medication.";
				dcterms:modified "2020-10-20"^^xsd:date;
				dcterms:creator <https://www.tib.eu/en/research-development/scientific-data-management/staff/samaneh-jozashoori/>.

clarify:StageClassification	rdf:type	owl:Class;
									rdfs:label	"StageClassification";
									rdfs:subClassOf	clarify:Concept;
									rdfs:comment "The clinical technique that is applied to indicate the TNM stage.";
									dcterms:modified "2020-10-21"^^xsd:date;
									dcterms:creator <https://www.tib.eu/en/research-development/scientific-data-management/staff/samaneh-jozashoori/>.

clarify:ClinicalStageClassification	rdf:type	owl:Class;
									rdfs:label	"ClinicalStageClassification";
									rdfs:subClassOf	clarify:StageClassification;
									rdfs:comment "The clinical technique that is applied to indicate the TNM stage.";
									dcterms:modified "2020-10-21"^^xsd:date;
									dcterms:creator <https://www.tib.eu/en/research-development/scientific-data-management/staff/samaneh-jozashoori/>.

clarify:PathologicalStageClassification	rdf:type	owl:Class;
										rdfs:label	"PathologicalStageClassification";
										rdfs:subClassOf	clarify:StageClassification;
										rdfs:comment "The pathological technique that is applied to indicate the TNM stage.";
										dcterms:modified "2020-10-21"^^xsd:date;
										dcterms:creator <https://www.tib.eu/en/research-development/scientific-data-management/staff/samaneh-jozashoori/>.

clarify:Disorder	rdf:type	owl:Class;
					rdfs:label	"Disorder";
					rdfs:subClassOf	clarify:Concept;
					rdfs:comment "A particular abnormal condition that negatively affects the structure or function of all or part of an organism, and that is not due to any immediate external injury.";
					dcterms:modified "2020-10-21"^^xsd:date;
					dcterms:creator <https://www.tib.eu/en/research-development/scientific-data-management/staff/samaneh-jozashoori/>.

clarify:StatusEvolution	rdf:type	owl:Class;
							rdfs:label	"StatusEvolution";
							rdfs:subClassOf	clarify:Observation;
							rdfs:comment "Patient survival status through monitoring.";
							dcterms:modified "2020-10-21"^^xsd:date;
							dcterms:creator <https://www.tib.eu/en/research-development/scientific-data-management/staff/samaneh-jozashoori/>.

clarify:TumorType	rdf:type	owl:Class;
						rdfs:subClassOf clarify:Concept;
						rdfs:label	"TumorType";
						rdfs:comment "The histology kind of the lung cancer. The type of tumor.";
						dcterms:modified "2020-09-15"^^xsd:date;
						prv:File "tumor_histology.ttl";
						dcterms:creator <https://www.tib.eu/en/research-development/scientific-data-management/staff/samaneh-jozashoori/>.	

clarify:PerformanceStatus	rdf:type	owl:Class;
						rdfs:subClassOf clarify:Observation;
						rdfs:label	"PerformanceStatus";
						rdfs:comment "Represents the Performance Status of the patient.";
						dcterms:modified "2020-10-21"^^xsd:date;
						prv:File "performance_status.ttl";
						dcterms:creator <https://www.tib.eu/en/research-development/scientific-data-management/staff/samaneh-jozashoori/>.	

clarify:SmokingHistory	rdf:type	owl:Class;
				rdfs:subClassOf clarify:Concept;
				rdfs:label	"Smoking";
				rdfs:comment "Represents the smoking habits of the patient and people with whom they live.";
				dcterms:modified "2020-10-21"^^xsd:date;
				prv:File "smoker_information.ttl";
				dcterms:creator <https://www.tib.eu/en/research-development/scientific-data-management/staff/samaneh-jozashoori/>.

clarify:ReproductionHistory	rdf:type	owl:Class;
							rdfs:subClassOf clarify:Concept;
							rdfs:label	"ReproductionHistory";
							rdfs:comment "Represents the reproduction history of the patient.";
							dcterms:modified "2020-10-21"^^xsd:date;
							prv:File "reproductive_information.ttl";
							dcterms:creator <https://www.tib.eu/en/research-development/scientific-data-management/staff/samaneh-jozashoori/>.

clarify:Prediagnosis  	rdf:type owl:Class;
					rdfs:label	"Prediagnosis";
					rdfs:subClassOf	clarify:Observation;
					rdfs:comment "Represents the symptoms of patients prior to diagnosis.";
					dcterms:modified "2020-10-23"^^xsd:date;
					prv:File "Prediagnosis_symptoms.ttl";
					dcterms:creator <https://www.tib.eu/en/research-development/scientific-data-management/staff/samaneh-jozashoori/>.	

clarify:Hemogram  	rdf:type owl:Class;
					rdfs:label	"Hemogram";
					rdfs:subClassOf	clarify:Observation;
					rdfs:comment "Represents a group of tests on blood sample to provide informaiton about general health. The tests include white blood cell count (WBC), red blood cell count (RBC), hemoglobin (HGB), hematocrit (HCT), mean cell volume (MCV), mean cell hemoglobin (MCH), mean cell hemoglobin concentration (MCHC) and platelet count.";
					dcterms:modified "2020-10-23"^^xsd:date;
					prv:File "Hemogram.ttl";
					dcterms:creator <https://www.tib.eu/en/research-development/scientific-data-management/staff/samaneh-jozashoori/>.	

clarify:NonOncologicalConsultation  	rdf:type owl:Class;
										rdfs:label	"NonOncologicalConsultation";
										rdfs:subClassOf	clarify:Observation;
										rdfs:comment "Represents the first consulation with a non-oncology specialist prior to be diagnosed wih cancer.";
										dcterms:modified "2020-10-23"^^xsd:date;
										prv:File "First_consultation_pre_oncology.ttl";
										dcterms:creator <https://www.tib.eu/en/research-development/scientific-data-management/staff/samaneh-jozashoori/>.	

#################################################################################################################################################
#################################################################################################################################################
#################################################################################################################################################
######################################################## Properties - attributes ################################################################
#################################################################################################################################################
#################################################################################################################################################
#################################################################################################################################################

clarify:annID	rdf:type	owl:DatatypeProperty;
				rdfs:label	"annID";
				rdfs:domain clarify:Annotation;
				rdfs:range	rdfs:Literal;
				rdfs:comment	"Identification of instances of Annotation class";	
				dcterms:modified "2020-11-19"^^xsd:date;
				dcterms:creator <https://www.tib.eu/en/research-development/scientific-data-management/staff/samaneh-jozashoori/>.

clarify:date	rdf:type	owl:DatatypeProperty;
								rdfs:label	"date";
								rdfs:domain	clarify:Concept;
								rdfs:range	rdfs:Literal;
								rdfs:comment "Represents the date of occurrence.";
								dcterms:modified "2020-10-20"^^xsd:date;							
								dcterms:creator <https://www.tib.eu/en/research-development/scientific-data-management/staff/samaneh-jozashoori/>.

clarify:description	rdf:type	owl:DatatypeProperty;
								rdfs:label	"description";
								rdfs:domain	clarify:Concept;
								rdfs:range	rdfs:Literal;
								rdfs:comment "Represents extra description of the concept.";
								dcterms:modified "2020-10-21"^^xsd:date;							
								dcterms:creator <https://www.tib.eu/en/research-development/scientific-data-management/staff/samaneh-jozashoori/>.

clarify:city	rdf:type	owl:DatatypeProperty;
						rdfs:label	"city ";
						rdfs:domain	clarify:LCPatient;
						rdfs:range	rdfs:Literal;
						rdfs:comment "Represents the city of residence of the patient (structured information provided by HUPHM)";
						dcterms:modified "2020-10-19"^^xsd:date;
						prv:File "patient.ttl";
						dcterms:creator <https://www.tib.eu/en/research-development/scientific-data-management/staff/samaneh-jozashoori/>.

clarify:birthDate	rdf:type	owl:DatatypeProperty;
						rdfs:label	"birthDate";
						rdfs:domain	clarify:LCPatient;
						rdfs:range	rdfs:Literal;
						rdfs:comment "Represents the birth date of the patient.";
						dcterms:modified "2020-10-19"^^xsd:date;
						prv:File "patient.ttl";
						dcterms:creator <https://www.tib.eu/en/research-development/scientific-data-management/staff/samaneh-jozashoori/>.		

clarify:hospitalID	rdf:type	owl:DatatypeProperty;
						rdfs:label	"hospitalID";
						rdfs:domain	clarify:LCPatient;
						rdfs:range	rdfs:Literal;
						rdfs:comment "Represents the ID of the hospital in which the patient is hopitaized.";
						dcterms:modified "2020-10-19"^^xsd:date;
						prv:File "patient.ttl";
						dcterms:creator <https://www.tib.eu/en/research-development/scientific-data-management/staff/samaneh-jozashoori/>.											

clarify:ehrID	rdf:type	owl:DatatypeProperty;
						rdfs:label	"ehrID";
						rdfs:domain	clarify:Concept;
						rdfs:range	rdfs:Literal;
						rdfs:comment "Represents the ID of the Electronic Health Record (EHR) to which the information is associated.";
						dcterms:modified "2020-10-19"^^xsd:date;
						dcterms:creator <https://www.tib.eu/en/research-development/scientific-data-management/staff/samaneh-jozashoori/>.

clarify:recordID	rdf:type	owl:DatatypeProperty;
						rdfs:label	"recordID";
						rdfs:domain	clarify:Concept;
						rdfs:range	rdfs:Literal;
						rdfs:comment "Represents the UPM auto-generated numeric ID.";
						dcterms:modified "2020-10-19"^^xsd:date;
						dcterms:creator <https://www.tib.eu/en/research-development/scientific-data-management/staff/samaneh-jozashoori/>.						

clarify:biomarkerObservationDate	rdf:type	owl:DatatypeProperty;
						rdfs:label	"biomarkerObservationDate";
						rdfs:domain	clarify:BiomarkerObservation;
						rdfs:range	rdfs:Literal;
						rdfs:comment "Represents the date on which the mutation is discovered.";
						dcterms:modified "2020-10-19"^^xsd:date;
						prv:File "mutation.ttl";
						dcterms:creator <https://www.tib.eu/en/research-development/scientific-data-management/staff/samaneh-jozashoori/>.						

clarify:biomarkerResult	rdf:type	owl:DatatypeProperty;
							rdfs:label	"biomarkerResult";
							rdfs:domain	clarify:Biomarker;
							rdfs:range	rdfs:Literal;
							rdfs:comment "Result of the reactive expression of the gene.";
							dcterms:modified "2020-10-19"^^xsd:date;
							prv:File "biomarker_mutation.ttl";
							prv:File "pdl1_expression.ttl";
							prv:File "ros1_mutation.ttl";
							dcterms:creator <https://www.tib.eu/en/research-development/scientific-data-management/staff/samaneh-jozashoori/>.	

clarify:biomarkerResult_FISH	rdf:type	owl:DatatypeProperty;
								rdfs:label	"biomarkerResult_FISH";
								rdfs:domain	clarify:Biomarker;
								rdfs:range	rdfs:Literal;
								rdfs:comment "Result of the FISH (Sanger sequencing plus Fluorescence In Situ Hybridization) test on targeted gene.";
								dcterms:modified "2020-11-19"^^xsd:date;
								prv:File "ALK_mutation.ttl";
								prv:File "HER2_mutation.ttl";
								dcterms:creator <https://www.tib.eu/en/research-development/scientific-data-management/staff/samaneh-jozashoori/>.

clarify:biomarkerResult_IHQ	rdf:type	owl:DatatypeProperty;
							rdfs:label	"biomarkerResult_IHQ";
							rdfs:domain	clarify:Biomarker;
							rdfs:range	rdfs:Literal;
							rdfs:comment "Result of the IHQ test on targeted gene.";
							dcterms:modified "2020-11-19"^^xsd:date;
							prv:File "ALK_mutation.ttl";
							prv:File "HER2_mutation.ttl";
							dcterms:creator <https://www.tib.eu/en/research-development/scientific-data-management/staff/samaneh-jozashoori/>.

clarify:biomarkerResult_RNA	rdf:type	owl:DatatypeProperty;
							rdfs:label	"biomarkerResult_RNA";
							rdfs:domain	clarify:Biomarker;
							rdfs:range	rdfs:Literal;
							rdfs:comment "Result of the RNA-based test on targeted gene.";
							dcterms:modified "2020-11-19"^^xsd:date;
							prv:File "ALK_mutation.ttl";
							prv:File "HER2_mutation.ttl";
							dcterms:creator <https://www.tib.eu/en/research-development/scientific-data-management/staff/samaneh-jozashoori/>.

clarify:biomarkerSpecification	rdf:type	owl:DatatypeProperty;
								rdfs:label	"biomarkerSpecification";
								rdfs:domain	clarify:Biomarker;
								rdfs:range	rdfs:Literal;
								rdfs:comment "";
								dcterms:modified "2020-10-19"^^xsd:date;
								prv:File "egfr_mutation.ttl";
								prv:File "pdl1_expression.ttl";
								prv:File "ros1_mutation.ttl";
								dcterms:creator <https://www.tib.eu/en/research-development/scientific-data-management/staff/samaneh-jozashoori/>.

clarify:biomarkerNegativeResult	rdf:type	owl:DatatypeProperty;
							rdfs:label	"biomarkerNegativeResult";
							rdfs:domain	clarify:Biomarker;
							rdfs:range	rdfs:Literal;
							rdfs:comment "Negativity of the mutation.";
							dcterms:modified "2020-10-19"^^xsd:date;
							dcterms:creator <https://www.tib.eu/en/research-development/scientific-data-management/staff/samaneh-jozashoori/>.

clarify:biomarkerResultPositivity	rdf:type	owl:DatatypeProperty;
							rdfs:label	"biomarkerResultPositivity";
							rdfs:domain	clarify:Biomarker;
							rdfs:range	rdfs:Literal;
							rdfs:comment "Positivity of the result.";
							dcterms:modified "2020-10-19"^^xsd:date;
							prv:File "pdl1_expression.ttl";
							dcterms:creator <https://www.tib.eu/en/research-development/scientific-data-management/staff/samaneh-jozashoori/>.

clarify:biomarkerResultReason	rdf:type	owl:DatatypeProperty;
								rdfs:label	"biomarkerResultReason";
								rdfs:domain	clarify:Biomarker;
								rdfs:range	rdfs:Literal;
								rdfs:comment "Provided reason to the result.";
								dcterms:modified "2020-10-19"^^xsd:date;
								prv:File "pdl1_expression.ttl";
								dcterms:creator <https://www.tib.eu/en/research-development/scientific-data-management/staff/samaneh-jozashoori/>.

clarify:mutation_T790M_positive_result	rdf:type	owl:DatatypeProperty;
								rdfs:label	"mutation_T790M_positive_result";
								rdfs:domain	clarify:Biomarker;
								rdfs:range	rdfs:Literal;
								rdfs:comment "Represents the mutation associated with positive T790M.";
								dcterms:modified "2020-10-19"^^xsd:date;
								prv:File "egfr_mutation.ttl";
								dcterms:creator <https://www.tib.eu/en/research-development/scientific-data-management/staff/samaneh-jozashoori/>.

clarify:mutation_T790M_negative_result	rdf:type	owl:DatatypeProperty;
								rdfs:label	"mutation_T790M_negative_result";
								rdfs:domain	clarify:Biomarker;
								rdfs:range	rdfs:Literal;
								rdfs:comment "Represents the mutation associated with negative T790M.";
								dcterms:modified "2020-10-19"^^xsd:date;
								prv:File "egfr_mutation.ttl";								
								dcterms:creator <https://www.tib.eu/en/research-development/scientific-data-management/staff/samaneh-jozashoori/>.

clarify:mutation_exon19_result	rdf:type	owl:DatatypeProperty;
								rdfs:label	"mutation_exon19_result";
								rdfs:domain	clarify:Biomarker;
								rdfs:range	rdfs:Literal;
								rdfs:comment "Represents the mutation associated with exon19.";
								dcterms:modified "2020-10-19"^^xsd:date;
								prv:File "egfr_mutation.ttl";								
								dcterms:creator <https://www.tib.eu/en/research-development/scientific-data-management/staff/samaneh-jozashoori/>.

clarify:mutation_exon21_result	rdf:type	owl:DatatypeProperty;
								rdfs:label	"mutation_exon21_result";
								rdfs:domain	clarify:Biomarker;
								rdfs:range	rdfs:Literal;
								rdfs:comment "Represents the mutation associated with exon21.";
								dcterms:modified "2020-10-19"^^xsd:date;
								prv:File "egfr_mutation.ttl";								
								dcterms:creator <https://www.tib.eu/en/research-development/scientific-data-management/staff/samaneh-jozashoori/>.

clarify:mutation_NOS_result	rdf:type	owl:DatatypeProperty;
								rdfs:label	"mutation_NOS_result";
								rdfs:domain	clarify:Biomarker;
								rdfs:range	rdfs:Literal;
								rdfs:comment "Represents the mutation assoc\iated with NOS.";
								dcterms:modified "2020-10-19"^^xsd:date;
								prv:File "egfr_mutation.ttl";								
								dcterms:creator <https://www.tib.eu/en/research-development/scientific-data-management/staff/samaneh-jozashoori/>.

clarify:mutation_other_result	rdf:type	owl:DatatypeProperty;
								rdfs:label	"mutation_other_result";
								rdfs:domain	clarify:Biomarker;
								rdfs:range	rdfs:Literal;
								rdfs:comment "Represents the specification of other observed mutations.";
								dcterms:modified "2020-10-19"^^xsd:date;
								prv:File "egfr_mutation.ttl";								
								dcterms:creator <https://www.tib.eu/en/research-development/scientific-data-management/staff/samaneh-jozashoori/>.	

clarify:occupation	rdf:type	owl:DatatypeProperty;
								rdfs:label	"occupation";
								rdfs:domain	clarify:LCPatient;
								rdfs:range	rdfs:Literal;
								rdfs:comment "Represents the occupation of the patient.";
								dcterms:modified "2020-10-20"^^xsd:date;
								prv:File "environmental_risk.ttl";								
								dcterms:creator <https://www.tib.eu/en/research-development/scientific-data-management/staff/samaneh-jozashoori/>.																

clarify:occupationDuration	rdf:type	owl:DatatypeProperty;
								rdfs:label	"occupationDuration";
								rdfs:domain	clarify:LCPatient;
								rdfs:range	rdfs:Literal;
								rdfs:comment "Represents the years spent in this occupation by patient.";
								dcterms:modified "2020-10-20"^^xsd:date;
								prv:File "environmental_risk.ttl";								
								dcterms:creator <https://www.tib.eu/en/research-development/scientific-data-management/staff/samaneh-jozashoori/>.	

clarify:mostProbable	rdf:type	owl:DatatypeProperty;
								rdfs:label	"mostProbable";
								rdfs:domain	clarify:Carcinogen;
								rdfs:range	rdfs:Literal;
								rdfs:comment "Represents the the most probable carcinogen that the patient has been exposed to.";
								dcterms:modified "2020-10-20"^^xsd:date;
								prv:File "environmental_risk.ttl";								
								dcterms:creator <https://www.tib.eu/en/research-development/scientific-data-management/staff/samaneh-jozashoori/>.

clarify:asbestos	rdf:type	owl:DatatypeProperty;
								rdfs:label	"asbestos";
								rdfs:domain	clarify:Carcinogen;
								rdfs:range	rdfs:Literal;
								rdfs:comment "Represents if the patient has been exposed to asbestos (a group of six naturally occurring minerals composed of soft, flexible fibers that are heat-resistant. Its use is allowed as long as it accounts for less than 1% of the product).";
								dcterms:modified "2020-10-20"^^xsd:date;
								prv:File "environmental_risk.ttl";								
								dcterms:creator <https://www.tib.eu/en/research-development/scientific-data-management/staff/samaneh-jozashoori/>.

clarify:arsenic	rdf:type	owl:DatatypeProperty;
								rdfs:label	"arsenic";
								rdfs:domain	clarify:Carcinogen;
								rdfs:range	rdfs:Literal;
								rdfs:comment "Represents if the patient has been exposed to arsenic.";
								dcterms:modified "2020-10-20"^^xsd:date;
								prv:File "environmental_risk.ttl";								
								dcterms:creator <https://www.tib.eu/en/research-development/scientific-data-management/staff/samaneh-jozashoori/>.

clarify:radon	rdf:type	owl:DatatypeProperty;
								rdfs:label	"radon";
								rdfs:domain	clarify:Carcinogen;
								rdfs:range	rdfs:Literal;
								rdfs:comment "Represents if the patient has been exposed to radon.";
								dcterms:modified "2020-10-20"^^xsd:date;
								prv:File "environmental_risk.ttl";								
								dcterms:creator <https://www.tib.eu/en/research-development/scientific-data-management/staff/samaneh-jozashoori/>.

clarify:silica	rdf:type	owl:DatatypeProperty;
								rdfs:label	"silica";
								rdfs:domain	clarify:Carcinogen;
								rdfs:range	rdfs:Literal;
								rdfs:comment "Represents if the patient has been exposed to silica.";
								dcterms:modified "2020-10-20"^^xsd:date;
								prv:File "environmental_risk.ttl";								
								dcterms:creator <https://www.tib.eu/en/research-development/scientific-data-management/staff/samaneh-jozashoori/>.

clarify:dieselSmoke	rdf:type	owl:DatatypeProperty;
								rdfs:label	"dieselSmoke";
								rdfs:domain	clarify:Carcinogen;
								rdfs:range	rdfs:Literal;
								rdfs:comment "Represents if the patient has been exposed to diesel smoke.";
								dcterms:modified "2020-10-20"^^xsd:date;
								prv:File "environmental_risk.ttl";								
								dcterms:creator <https://www.tib.eu/en/research-development/scientific-data-management/staff/samaneh-jozashoori/>.																								

clarify:asbestosExposure	rdf:type	owl:DatatypeProperty;
							rdfs:label	"asbestosExposure";
							rdfs:domain	clarify:Carcinogen;
							rdfs:range	rdfs:Literal;
							rdfs:comment "Represents if the patient has been exposed to asbestos.";
							dcterms:modified "2020-11-17"^^xsd:date;
							prv:File "environmental_risk.ttl";								
							dcterms:creator <https://www.tib.eu/en/research-development/scientific-data-management/staff/samaneh-jozashoori/>.

clarify:asbestosExposureType	rdf:type	owl:DatatypeProperty;
								rdfs:label	"asbestosExposureType";
								rdfs:domain	clarify:Carcinogen;
								rdfs:range	rdfs:Literal;
								rdfs:comment "Represents type of exposition to asbestos.";
								dcterms:modified "2020-10-20"^^xsd:date;
								prv:File "environmental_risk.ttl";								
								dcterms:creator <https://www.tib.eu/en/research-development/scientific-data-management/staff/samaneh-jozashoori/>.								

clarify:progressionOrRelapse	rdf:type	owl:DatatypeProperty;
								rdfs:label	"progressionOrRelapse";
								rdfs:domain	clarify:ProgressionRelapseObservation;
								rdfs:range	rdfs:Literal;
								rdfs:comment "Represents the value indicating if the progression or relapse is occurred.";
								dcterms:modified "2020-10-20"^^xsd:date;
								prv:File "relapse_progression.ttl";								
								dcterms:creator <https://www.tib.eu/en/research-development/scientific-data-management/staff/samaneh-jozashoori/>.

clarify:progressionType	rdf:type	owl:DatatypeProperty;
								rdfs:label	"progressionType";
								rdfs:domain	clarify:ProgressionRelapseObservation;
								rdfs:range	rdfs:Literal;
								rdfs:comment "Represents type of progression that patient has experienced.";
								dcterms:modified "2020-10-20"^^xsd:date;
								prv:File "relapse_progression.ttl";								
								dcterms:creator <https://www.tib.eu/en/research-development/scientific-data-management/staff/samaneh-jozashoori/>.

clarify:therapyType	rdf:type	owl:DatatypeProperty;
								rdfs:label	"therapyType";
								rdfs:domain	clarify:ProgressionRelapseObservation;
								rdfs:range	rdfs:Literal;
								rdfs:comment "Represents the type of therapy that is prescribed to the patient (active or palliative care -pain relieving-).";
								dcterms:modified "2020-10-20"^^xsd:date;
								prv:File "relapse_progression.ttl";								
								dcterms:creator <https://www.tib.eu/en/research-development/scientific-data-management/staff/samaneh-jozashoori/>.

clarify:progressionLocation	rdf:type	owl:DatatypeProperty;
								rdfs:label	"progressionLocation";
								rdfs:domain	clarify:CancerPatient;
								rdfs:range	rdfs:Literal;
								rdfs:comment "Represents the location of occurrence of the progression/ relapse.";
								dcterms:modified "2020-11-16"^^xsd:date;
								prv:File "progression_location.ttl";								
								dcterms:creator <https://www.tib.eu/en/research-development/scientific-data-management/staff/samaneh-jozashoori/>.

clarify:previousCancer	rdf:type	owl:DatatypeProperty;
								rdfs:label	"previousCancer";
								rdfs:domain	clarify:PatientHistory;
								rdfs:range	rdfs:Literal;
								rdfs:comment "Represents the previous cancer from which the patient has suffered before.";
								dcterms:modified "2020-10-20"^^xsd:date;
								prv:File "oncological_history.ttl";								
								dcterms:creator <https://www.tib.eu/en/research-development/scientific-data-management/staff/samaneh-jozashoori/>.

clarify:previousCancerType	rdf:type	owl:DatatypeProperty;
								rdfs:label	"previousCancerType";
								rdfs:domain	clarify:PatientHistory;
								rdfs:range	rdfs:Literal;
								rdfs:comment "Represents the type of previous cancer from which the patient has suffered before.";
								dcterms:modified "2020-10-20"^^xsd:date;
								prv:File "oncological_history.ttl";								
								dcterms:creator <https://www.tib.eu/en/research-development/scientific-data-management/staff/samaneh-jozashoori/>.

clarify:numberOfFamilyWithLC	rdf:type	owl:DatatypeProperty;
									rdfs:label	"numberOfFamilyWithLC";
									rdfs:domain	clarify:FamilyHistory;
									rdfs:range	rdfs:Literal;
									rdfs:comment "Represents the number of family members with lung cancer.";
									dcterms:modified "2020-10-20"^^xsd:date;
									prv:File "oncological_history.ttl";								
									dcterms:creator <https://www.tib.eu/en/research-development/scientific-data-management/staff/samaneh-jozashoori/>.

clarify:numberOfFamilyWithOtherCancers	rdf:type	owl:DatatypeProperty;
										rdfs:label	"numberOfFamilyWithOtherCancers";
										rdfs:domain	clarify:FamilyHistory;
										rdfs:range	rdfs:Literal;
										rdfs:comment "Represents the number of family members with cancers other than lung.";
										dcterms:modified "2020-10-20"^^xsd:date;
										prv:File "oncological_history.ttl";								
										dcterms:creator <https://www.tib.eu/en/research-development/scientific-data-management/staff/samaneh-jozashoori/>.

clarify:familyType	rdf:type	owl:DatatypeProperty;
									rdfs:label	"familyType";
									rdfs:domain	clarify:FamilyHistory;
									rdfs:range	rdfs:Literal;
									rdfs:comment "Represents the type of family kinship with the patient.";
									dcterms:modified "2020-10-20"^^xsd:date;
									prv:File "oncological_history.ttl";								
									dcterms:creator <https://www.tib.eu/en/research-development/scientific-data-management/staff/samaneh-jozashoori/>.

clarify:familyCancerType	rdf:type	owl:DatatypeProperty;
									rdfs:label	"familyCancerType";
									rdfs:domain	clarify:FamilyHistory;
									rdfs:range	rdfs:Literal;
									rdfs:comment "Represents the type of the cancer that the family member had/ has (1=Breast, 2=Head and neck, 3=Germinal tumors, 4=Sarcoma, 5=Central nervous system, 6=Unknown origin carcinoma, 7=Colorrectal, 8=Esophagogastric, 9=Pancreatic, 10=Gall bladder, 11=Liver, 2=Melanoma, 13=Skin no melanoma, 14=Bladder/urinary tract, 15=Renal, 16=Prostate, 17=Uterus/cervical, 18=Lymphoma, 19=Leukemia, 20=Lung, 22=Ovarian, 888=Others, -1=- ).";
									dcterms:modified "2020-10-20"^^xsd:date;
									prv:File "oncological_history.ttl";								
									dcterms:creator <https://www.tib.eu/en/research-development/scientific-data-management/staff/samaneh-jozashoori/>.

clarify:trialLabel	rdf:type	owl:DatatypeProperty;
					rdfs:label	"trialLabel";
					rdfs:domain	clarify:ClinicalTrial;
					rdfs:range	rdfs:Literal;
					rdfs:comment "Represents the name of the clinical trial.";
					dcterms:modified "2020-10-20"^^xsd:date;
					prv:File "clinical_trial.ttl";								
					dcterms:creator <https://www.tib.eu/en/research-development/scientific-data-management/staff/samaneh-jozashoori/>.

clarify:trialIsObservational	rdf:type	owl:DatatypeProperty;
								rdfs:label	"trialIsObservational";
								rdfs:domain	clarify:ClinicalTrial;
								rdfs:range	rdfs:Literal;
								rdfs:comment "Indicates if the clinical trial is observational.";
								dcterms:modified "2020-10-20"^^xsd:date;
								prv:File "clinical_trial.ttl";								
								dcterms:creator <https://www.tib.eu/en/research-development/scientific-data-management/staff/samaneh-jozashoori/>.

clarify:drugBasedTrial	rdf:type	owl:DatatypeProperty;
						rdfs:label	"drugBasedTrial";
						rdfs:domain	clarify:ClinicalTrial;
						rdfs:range	rdfs:Literal;
						rdfs:comment "Indicates if the clinical trial is based on drugs.";
						dcterms:modified "2020-10-20"^^xsd:date;
						prv:File "clinical_trial.ttl";								
						dcterms:creator <https://www.tib.eu/en/research-development/scientific-data-management/staff/samaneh-jozashoori/>.

clarify:directedTrial	rdf:type	owl:DatatypeProperty;
						rdfs:label	"directedTrial";
						rdfs:domain	clarify:ClinicalTrial;
						rdfs:range	rdfs:Literal;
						rdfs:comment "Indicates if the clinical trial is directed.";
						dcterms:modified "2020-10-20"^^xsd:date;
						prv:File "clinical_trial.ttl";								
						dcterms:creator <https://www.tib.eu/en/research-development/scientific-data-management/staff/samaneh-jozashoori/>.

clarify:trialPhase	rdf:type	owl:DatatypeProperty;
						rdfs:label	"trialPhase";
						rdfs:domain	clarify:ClinicalTrial;
						rdfs:range	rdfs:Literal;
						rdfs:comment "Indicates the phase of the clinical trial.";
						dcterms:modified "2020-10-20"^^xsd:date;
						prv:File "clinical_trial.ttl";								
						dcterms:creator <https://www.tib.eu/en/research-development/scientific-data-management/staff/samaneh-jozashoori/>.

clarify:trialTargetLabel	rdf:type	owl:DatatypeProperty;
							rdfs:label	"trialTargetLabel";
							rdfs:domain	clarify:ClinicalTrial;
							rdfs:range	rdfs:Literal;
							rdfs:comment "Indicates the name of the target of the clinical trial.";
							dcterms:modified "2020-10-20"^^xsd:date;
							prv:File "targets_clinical_trial.ttl";								
							dcterms:creator <https://www.tib.eu/en/research-development/scientific-data-management/staff/samaneh-jozashoori/>.

clarify:diagnosticTumorSize	rdf:type	owl:DatatypeProperty;
							rdfs:label	"diagnosticTumorSize";
							rdfs:domain	clarify:Diagnosis;
							rdfs:range	rdfs:Literal;
							rdfs:comment "Indicates the size of the patient's tumor (T) at the diagnosis time.";
							dcterms:modified "2020-11-16"^^xsd:date;
							prv:File "diagnostic.ttl";								
							dcterms:creator <https://www.tib.eu/en/research-development/scientific-data-management/staff/samaneh-jozashoori/>.

clarify:tumorSize	rdf:type	owl:DatatypeProperty;
							rdfs:label	"tumorSize";
							rdfs:domain	clarify:CancerStageTNM;
							rdfs:range	rdfs:Literal;
							rdfs:comment "Indicates the size of the patient's tumor (T).";
							dcterms:modified "2020-10-20"^^xsd:date;
							prv:File "tnm_stadification.ttl";
							prv:File "surgery.ttl";							
							dcterms:creator <https://www.tib.eu/en/research-development/scientific-data-management/staff/samaneh-jozashoori/>.

clarify:lymphNodesInvolvement	rdf:type	owl:DatatypeProperty;
							rdfs:label	"lymphNodesInvolvement";
							rdfs:domain	clarify:CancerStageTNM;
							rdfs:range	rdfs:Literal;
							rdfs:comment "Indicates if the lymph nodes are involved (N).";
							dcterms:modified "2020-10-20"^^xsd:date;
							prv:File "tnm_stadification.ttl";
							prv:File "surgery.ttl";								
							dcterms:creator <https://www.tib.eu/en/research-development/scientific-data-management/staff/samaneh-jozashoori/>.

clarify:metastatisStage	rdf:type	owl:DatatypeProperty;
							rdfs:label	"metastatisStage";
							rdfs:domain	clarify:CancerStageTNM;
							rdfs:range	rdfs:Literal;
							rdfs:comment "Indicates that to what extend the cancer is metastasized (M).";
							dcterms:modified "2020-10-20"^^xsd:date;
							prv:File "tnm_stadification.ttl";
							prv:File "surgery.ttl";								
							dcterms:creator <https://www.tib.eu/en/research-development/scientific-data-management/staff/samaneh-jozashoori/>.

clarify:existenceOf_extrathoracicLymphadenopathies	rdf:type	owl:DatatypeProperty;
													rdfs:label	"existenceOf_extrathoracicLymphadenopathies";
													rdfs:domain	clarify:MetastasisLocation;
													rdfs:range	rdfs:Literal;
													rdfs:comment ".";
													dcterms:modified "2020-10-20"^^xsd:date;
													prv:File "metastasis_location.ttl";								
													dcterms:creator <https://www.tib.eu/en/research-development/scientific-data-management/staff/samaneh-jozashoori/>.

clarify:existenceOf_thoracicLymphadenopathy	rdf:type	owl:DatatypeProperty;
											rdfs:label	"existenceOf_thoracicLymphadenopathy";
											rdfs:domain	clarify:MetastasisLocation;
											rdfs:range	rdfs:Literal;
											rdfs:comment ".";
											dcterms:modified "2020-10-20"^^xsd:date;
											prv:File "metastasis_location.ttl";								
											dcterms:creator <https://www.tib.eu/en/research-development/scientific-data-management/staff/samaneh-jozashoori/>.

clarify:existenceOf_meningealCarcinomatosis	rdf:type	owl:DatatypeProperty;
											rdfs:label	"existenceOf_meningealCarcinomatosis";
											rdfs:domain	clarify:MetastasisLocation;
											rdfs:range	rdfs:Literal;
											rdfs:comment ".";
											dcterms:modified "2020-10-20"^^xsd:date;
											prv:File "metastasis_location.ttl";								
											dcterms:creator <https://www.tib.eu/en/research-development/scientific-data-management/staff/samaneh-jozashoori/>.

clarify:existenceOf_pericardialEffusion	rdf:type	owl:DatatypeProperty;
										rdfs:label	"existenceOf_pericardialEffusion";
										rdfs:domain	clarify:MetastasisLocation;
										rdfs:range	rdfs:Literal;
										rdfs:comment ".";
										dcterms:modified "2020-10-20"^^xsd:date;
										prv:File "metastasis_location.ttl";								
										dcterms:creator <https://www.tib.eu/en/research-development/scientific-data-management/staff/samaneh-jozashoori/>.

clarify:existenceOf_pleuralEffusion	rdf:type	owl:DatatypeProperty;
									rdfs:label	"existenceOf_pleuralEffusion";
									rdfs:domain	clarify:MetastasisLocation;
									rdfs:range	rdfs:Literal;
									rdfs:comment ".";
									dcterms:modified "2020-10-20"^^xsd:date;
									prv:File "metastasis_location.ttl";								
									dcterms:creator <https://www.tib.eu/en/research-development/scientific-data-management/staff/samaneh-jozashoori/>.

clarify:existenceOf_liverMetastasis	rdf:type	owl:DatatypeProperty;
									rdfs:label	"existenceOf_liverMetastasis";
									rdfs:domain	clarify:MetastasisLocation;
									rdfs:range	rdfs:Literal;
									rdfs:comment ".";
									dcterms:modified "2020-10-20"^^xsd:date;
									prv:File "metastasis_location.ttl";								
									dcterms:creator <https://www.tib.eu/en/research-development/scientific-data-management/staff/samaneh-jozashoori/>.

clarify:existenceOf_boneMetastasis	rdf:type	owl:DatatypeProperty;
									rdfs:label	"existenceOf_boneMetastasis";
									rdfs:domain	clarify:MetastasisLocation;
									rdfs:range	rdfs:Literal;
									rdfs:comment ".";
									dcterms:modified "2020-10-20"^^xsd:date;
									prv:File "metastasis_location.ttl";								
									dcterms:creator <https://www.tib.eu/en/research-development/scientific-data-management/staff/samaneh-jozashoori/>.

clarify:existenceOf_bilateralLymphangitis	rdf:type	owl:DatatypeProperty;
											rdfs:label	"existenceOf_bilateralLymphangitis";
											rdfs:domain	clarify:MetastasisLocation;
											rdfs:range	rdfs:Literal;
											rdfs:comment ".";
											dcterms:modified "2020-10-20"^^xsd:date;
											prv:File "metastasis_location.ttl";								
											dcterms:creator <https://www.tib.eu/en/research-development/scientific-data-management/staff/samaneh-jozashoori/>.													

clarify:existenceOf_pleuralNodules	rdf:type	owl:DatatypeProperty;
									rdfs:label	"existenceOf_pleuralNodules";
									rdfs:domain	clarify:MetastasisLocation;
									rdfs:range	rdfs:Literal;
									rdfs:comment ".";
									dcterms:modified "2020-10-20"^^xsd:date;
									prv:File "metastasis_location.ttl";								
									dcterms:creator <https://www.tib.eu/en/research-development/scientific-data-management/staff/samaneh-jozashoori/>.

clarify:existenceOf_pancreasMetastasis	rdf:type	owl:DatatypeProperty;
										rdfs:label	"existenceOf_pancreasMetastasis";
										rdfs:domain	clarify:MetastasisLocation;
										rdfs:range	rdfs:Literal;
										rdfs:comment ".";
										dcterms:modified "2020-10-20"^^xsd:date;
										prv:File "metastasis_location.ttl";								
										dcterms:creator <https://www.tib.eu/en/research-development/scientific-data-management/staff/samaneh-jozashoori/>.

clarify:existenceOf_peritoneumMetastasis	rdf:type	owl:DatatypeProperty;
											rdfs:label	"existenceOf_peritoneumMetastasis";
											rdfs:domain	clarify:MetastasisLocation;
											rdfs:range	rdfs:Literal;
											rdfs:comment "The peritoneum is the serous membrane forming the lining of the abdominal cavity or coelom in amniotes and some invertebrates, such as annelids. It covers most of the intra-abdominal (or coelomic) organs, and is composed of a layer of mesothelium supported by a thin layer of connective tissue.";
											dcterms:modified "2020-10-20"^^xsd:date;
											prv:File "metastasis_location.ttl";								
											dcterms:creator <https://www.tib.eu/en/research-development/scientific-data-management/staff/samaneh-jozashoori/>.

clarify:existenceOf_lungMetastasis	rdf:type	owl:DatatypeProperty;
									rdfs:label	"existenceOf_lungMetastasis";
									rdfs:domain	clarify:MetastasisLocation;
									rdfs:range	rdfs:Literal;
									rdfs:comment ".";
									dcterms:modified "2020-10-20"^^xsd:date;
									prv:File "metastasis_location.ttl";								
									dcterms:creator <https://www.tib.eu/en/research-development/scientific-data-management/staff/samaneh-jozashoori/>.

clarify:existenceOf_centralNervousSystemMetastasis	rdf:type	owl:DatatypeProperty;
													rdfs:label	"existenceOf_centralNervousSystemMetastasis";
													rdfs:domain	clarify:MetastasisLocation;
													rdfs:range	rdfs:Literal;
													rdfs:comment ".";
													dcterms:modified "2020-10-20"^^xsd:date;
													prv:File "metastasis_location.ttl";								
													dcterms:creator <https://www.tib.eu/en/research-development/scientific-data-management/staff/samaneh-jozashoori/>.

clarify:existenceOf_subcutaneousMetastasis	rdf:type	owl:DatatypeProperty;
											rdfs:label	"existenceOf_subcutaneousMetastasis";
											rdfs:domain	clarify:MetastasisLocation;
											rdfs:range	rdfs:Literal;
											rdfs:comment "Subcutaneous refers to what is situated or applied under the skin.";
											dcterms:modified "2020-10-20"^^xsd:date;
											prv:File "metastasis_location.ttl";								
											dcterms:creator <https://www.tib.eu/en/research-development/scientific-data-management/staff/samaneh-jozashoori/>.																																							

clarify:existenceOf_adrenalMetastasis	rdf:type	owl:DatatypeProperty;
											rdfs:label	"existenceOf_adrenalMetastasis";
											rdfs:domain	clarify:MetastasisLocation;
											rdfs:range	rdfs:Literal;
											rdfs:comment ".";
											dcterms:modified "2020-10-20"^^xsd:date;
											prv:File "metastasis_location.ttl";								
											dcterms:creator <https://www.tib.eu/en/research-development/scientific-data-management/staff/samaneh-jozashoori/>.	

clarify:existenceOf_softTissuesMetastasis	rdf:type	owl:DatatypeProperty;
											rdfs:label	"existenceOf_softTissuesMetastasis";
											rdfs:domain	clarify:MetastasisLocation;
											rdfs:range	rdfs:Literal;
											rdfs:comment ".";
											dcterms:modified "2020-10-20"^^xsd:date;
											prv:File "metastasis_location.ttl";								
											dcterms:creator <https://www.tib.eu/en/research-development/scientific-data-management/staff/samaneh-jozashoori/>.												

clarify:existenceOf_otherMetastasis	rdf:type	owl:DatatypeProperty;
											rdfs:label	"existenceOf_otherMetastasis";
											rdfs:domain	clarify:MetastasisLocation;
											rdfs:range	rdfs:Literal;
											rdfs:comment ".";
											dcterms:modified "2020-10-20"^^xsd:date;
											prv:File "metastasis_location.ttl";								
											dcterms:creator <https://www.tib.eu/en/research-development/scientific-data-management/staff/samaneh-jozashoori/>.		

clarify:diagnosisTechnique	rdf:type	owl:DatatypeProperty;
							rdfs:label	"diagnosisTechnique";
							rdfs:domain	clarify:Diagnosis;
							rdfs:range	rdfs:Literal;
							rdfs:comment "Indicates the diagnosis technique that is used.";
							dcterms:modified "2020-10-20"^^xsd:date;
							prv:File "diagnostic.ttl";								
							dcterms:creator <https://www.tib.eu/en/research-development/scientific-data-management/staff/samaneh-jozashoori/>.

clarify:stagingSystemTechnique	rdf:type	owl:DatatypeProperty;
								rdfs:label	"stagingSystemTechnique";
								rdfs:domain	clarify:Diagnosis;
								rdfs:range	rdfs:Literal;
								rdfs:comment "Indicates the technique that is applied for staging diagnosis.";
								dcterms:modified "2020-10-20"^^xsd:date;
								prv:File "diagnostic.ttl";								
								dcterms:creator <https://www.tib.eu/en/research-development/scientific-data-management/staff/samaneh-jozashoori/>.

clarify:treatementLineBestResponse	rdf:type	owl:DatatypeProperty;
									rdfs:label	"treatementLineBestResponse";
									rdfs:domain	clarify:OncologicalTreatmentLine;
									rdfs:range	rdfs:Literal;
									rdfs:comment "Represents the best response of the patient to the treatement line.";
									dcterms:modified "2020-11-19"^^xsd:date;
									prv:File "chemotherapy_treatment_line.ttl";								
									dcterms:creator <https://www.tib.eu/en/research-development/scientific-data-management/staff/samaneh-jozashoori/>.

clarify:treatementLineStartDate	rdf:type	owl:DatatypeProperty;
							rdfs:label	"treatementLineStartDate";
							rdfs:domain	clarify:OncologicalTreatmentLine;
							rdfs:range	rdfs:Literal;
							rdfs:comment "Represents the starting date of the chemotherapy treatment line.";
							dcterms:modified "2020-11-17"^^xsd:date;
							prv:File "chemotherapy_treatment_line.ttl";
							prv:File "radiotherapy_treatment_line.ttl";								
							dcterms:creator <https://www.tib.eu/en/research-development/scientific-data-management/staff/samaneh-jozashoori/>.

clarify:treatementLineEndingDate	rdf:type	owl:DatatypeProperty;
								rdfs:label	"treatementLineEndingDate";
								rdfs:domain	clarify:OncologicalTreatmentLine;
								rdfs:range	rdfs:Literal;
								rdfs:comment "Represents the ending date of the chemotherapy treatment line.";
								dcterms:modified "2020-11-17"^^xsd:date;
								prv:File "chemotherapy_treatment_line.ttl";	
								prv:File "radiotherapy_treatment_line.ttl";							
								dcterms:creator <https://www.tib.eu/en/research-development/scientific-data-management/staff/samaneh-jozashoori/>.

clarify:treatmentLineNumber	rdf:type     owl:DatatypeProperty;
							rdfs:label	"treatmentLineNumber";
							rdfs:domain	clarify:OncologicalTreatmentLine;
							rdfs:range	rdfs:Literal;
							rdfs:comment "The number representing the oncological line of treatment.";
							dcterms:modified "2020-10-20"^^xsd:date;
							prv:File "chemotherapy_treatment_line.ttl";								
							prv:File "radiotherapy_treatment_line.ttl";								
							dcterms:creator <https://www.tib.eu/en/research-development/scientific-data-management/staff/samaneh-jozashoori/>.

clarify:treatmentLineType	rdf:type     owl:DatatypeProperty;
							rdfs:label	"treatmentLineType";
							rdfs:domain	clarify:OncologicalTreatmentLine;
							rdfs:range	rdfs:Literal;
							rdfs:comment "Represents type of the treatment line (1=QT intravenous, 2=Oral targeted therapy, 3=Neoadjuvant chemotherapy, 4=Adjuvant chemotherapy, 6=Concomitant QT-RT, 7=Sequential QT-RT, 8=Adjuvant QT-RT, 9=Neoadjuvant QT-RT, 10=Immunotherapy, 12=Hormonal, 13=Oral and intravenous chemotherapy, 14=Oral chemotherapy, 15=Intravenous chemotherapy + immunotherapy, 11=Others, -1=- ).";
							dcterms:modified "2020-10-20"^^xsd:date;
							prv:File "chemotherapy_treatment_line.ttl";								
							prv:File "radiotherapy_treatment_line.ttl";								
							dcterms:creator <https://www.tib.eu/en/research-development/scientific-data-management/staff/samaneh-jozashoori/>.

clarify:treatmentLineCycle	rdf:type	owl:DatatypeProperty;
							rdfs:label	"treatmentLineCycle";
							rdfs:domain	clarify:OncologicalTreatmentLine;
							rdfs:range	rdfs:Literal;
							rdfs:comment "Represents the number of cycles through which the corresponding drugs have been applied.";
							dcterms:modified "2020-10-20"^^xsd:date;
							prv:File "chemotherapy_drugs.ttl";	
							prv:File "radiotherapy_drugs.ttl";															
							dcterms:creator <https://www.tib.eu/en/research-development/scientific-data-management/staff/samaneh-jozashoori/>.

clarify:treatmentLineDosage	rdf:type	owl:DatatypeProperty;
							rdfs:label	"treatmentLineDosage";
							rdfs:domain	clarify:OncologicalTreatmentLine;
							rdfs:range	rdfs:Literal;
							rdfs:comment "Represents the dosage that is prescribed to the patient.";
							dcterms:modified "2020-10-20"^^xsd:date;
							prv:File "radiotherapy_drugs.ttl";															
							dcterms:creator <https://www.tib.eu/en/research-development/scientific-data-management/staff/samaneh-jozashoori/>.

clarify:treatmentLineFractioning	rdf:type	owl:DatatypeProperty;
									rdfs:label	"treatmentLineFractioning";
									rdfs:domain	clarify:OncologicalTreatmentLine;
									rdfs:range	rdfs:Literal;
									rdfs:comment "Represents the fractioning that is prescribed to the patient.";
									dcterms:modified "2020-11-19"^^xsd:date;
									prv:File "radiotherapy_drugs.ttl";															
									dcterms:creator <https://www.tib.eu/en/research-development/scientific-data-management/staff/samaneh-jozashoori/>.

clarify:treatmentLineMaintenance	rdf:type	owl:DatatypeProperty;
									rdfs:label	"treatmentLineMaintenance";
									rdfs:domain	clarify:OncologicalTreatmentLine;
									rdfs:range	rdfs:Literal;
									rdfs:comment "Represents the type of drugs that are prescribed for the maintenance!";
									dcterms:modified "2020-11-19"^^xsd:date;
									prv:File "chemotherapy_drugs.ttl";															
									dcterms:creator <https://www.tib.eu/en/research-development/scientific-data-management/staff/samaneh-jozashoori/>.

clarify:radiotherapyArea	rdf:type	owl:DatatypeProperty;
							rdfs:label	"radiotherapyArea";
							rdfs:domain	clarify:RadiotherapyTreatmentLine;
							rdfs:range	rdfs:Literal;
							rdfs:comment "Represents the area that is radiated during the radiotherapy.";
							dcterms:modified "2020-10-20"^^xsd:date;
							prv:File "radiotherapy_treatment_line.ttl";								
							dcterms:creator <https://www.tib.eu/en/research-development/scientific-data-management/staff/samaneh-jozashoori/>.

clarify:radiotherapyType	rdf:type	owl:DatatypeProperty;
							rdfs:label	"radiotherapyType";
							rdfs:domain	clarify:RadiotherapyTreatmentLine;
							rdfs:range	rdfs:Literal;
							rdfs:comment "Represents the type of radiotherapy.";
							dcterms:modified "2020-11-19"^^xsd:date;
							prv:File "radiotherapy_treatment_line.ttl";								
							dcterms:creator <https://www.tib.eu/en/research-development/scientific-data-management/staff/samaneh-jozashoori/>.

clarify:radiotherapyIntention	rdf:type	owl:DatatypeProperty;
								rdfs:label	"radiotherapyIntention";
								rdfs:domain	clarify:RadiotherapyTreatmentLine;
								rdfs:range	rdfs:Literal;
								rdfs:comment "Represents the purpose(!) of performing radiotherapy.";
								dcterms:modified "2020-10-20"^^xsd:date;
								prv:File "radiotherapy_treatment_line.ttl";								
								dcterms:creator <https://www.tib.eu/en/research-development/scientific-data-management/staff/samaneh-jozashoori/>.							

clarify:surgeryLabel	rdf:type	owl:DatatypeProperty;
							rdfs:label	"surgeryLabel";
							rdfs:domain	clarify:OncologicalSurgery;
							rdfs:range	rdfs:Literal;
							rdfs:comment "Represents the name of the surgery.";
							dcterms:modified "2020-10-20"^^xsd:date;
							prv:File "surgery.ttl";								
							dcterms:creator <https://www.tib.eu/en/research-development/scientific-data-management/staff/samaneh-jozashoori/>.

clarify:surgeryClass	rdf:type	owl:DatatypeProperty;
							rdfs:label	"surgeryClass";
							rdfs:domain	clarify:OncologicalSurgery;
							rdfs:range	rdfs:Literal;
							rdfs:comment "Represents the type of the surgery.";
							dcterms:modified "2020-10-20"^^xsd:date;
							prv:File "surgery.ttl";								
							dcterms:creator <https://www.tib.eu/en/research-development/scientific-data-management/staff/samaneh-jozashoori/>.

clarify:surgerySubType	rdf:type	owl:DatatypeProperty;
							rdfs:label	"surgerySubType";
							rdfs:domain	clarify:OncologicalSurgery;
							rdfs:range	rdfs:Literal;
							rdfs:comment "Represents the subtype of the surgery.";
							dcterms:modified "2020-10-20"^^xsd:date;
							prv:File "surgery.ttl";								
							dcterms:creator <https://www.tib.eu/en/research-development/scientific-data-management/staff/samaneh-jozashoori/>.

clarify:surgeryPathologicalResponse	rdf:type	owl:DatatypeProperty;
									rdfs:label	"surgeryPathologicalResponse";
									rdfs:domain	clarify:OncologicalSurgery;
									rdfs:range	rdfs:Literal;
									rdfs:comment "Represents the type of pathological response to the surgery that the patient experienced.";
									dcterms:modified "2020-11-19"^^xsd:date;
									prv:File "surgery.ttl";								
									dcterms:creator <https://www.tib.eu/en/research-development/scientific-data-management/staff/samaneh-jozashoori/>.

clarify:surgeryResectionGrade	rdf:type	owl:DatatypeProperty;
								rdfs:label	"surgeryResectionGrade";
								rdfs:domain	clarify:OncologicalSurgery;
								rdfs:range	rdfs:Literal;
								rdfs:comment "Indicates the degree of the resection that is applied during the surgery.";
								dcterms:modified "2020-11-19"^^xsd:date;
								prv:File "surgery.ttl";								
								dcterms:creator <https://www.tib.eu/en/research-development/scientific-data-management/staff/samaneh-jozashoori/>.

clarify:surgeryPerioperativeDeath	rdf:type	owl:DatatypeProperty;
									rdfs:label	"surgeryPerioperativeDeath";
									rdfs:domain	clarify:OncologicalSurgery;
									rdfs:range	rdfs:Literal;
									rdfs:comment "Represents if the perioperative death has took place during or after the surgery.";
									dcterms:modified "2020-11-19"^^xsd:date;
									prv:File "surgery.ttl";								
									dcterms:creator <https://www.tib.eu/en/research-development/scientific-data-management/staff/samaneh-jozashoori/>.

clarify:fullBloodCount	rdf:type	owl:DatatypeProperty;
						rdfs:label	"fullBloodCount";
						rdfs:domain	clarify:ClinicalStageClassification;
						rdfs:range	rdfs:Literal;
						rdfs:comment "Indicates if the stage classification technique (pTNM) used is FBC (The full blood count, a blood test that may play a role in early detection of the disease).";
						dcterms:modified "2020-10-21"^^xsd:date;
						prv:File "clinical_stadification_techniques.ttl";								
						dcterms:creator <https://www.tib.eu/en/research-development/scientific-data-management/staff/samaneh-jozashoori/>.

clarify:gammaScan	rdf:type	owl:DatatypeProperty;
					rdfs:label	"gammaScan";
					rdfs:domain	clarify:ClinicalStageClassification;
					rdfs:range	rdfs:Literal;
					rdfs:comment "Indicates if the stage classification technique (pTNM) used is gamma scan.";
					dcterms:modified "2020-10-21"^^xsd:date;
					prv:File "clinical_stadification_techniques.ttl";								
					dcterms:creator <https://www.tib.eu/en/research-development/scientific-data-management/staff/samaneh-jozashoori/>.

clarify:mediastinoscopy	rdf:type	owl:DatatypeProperty;
						rdfs:label	"mediastinoscopy";
						rdfs:domain	clarify:StageClassification;
						rdfs:range	rdfs:Literal;
						rdfs:comment "Indicates if the stage classification technique (pTNM) used is mediastinoscopy (a procedure used to examine the mediastinum. This is the space behind the breastbone (sternum) in the middle of the chest, between the 2 lungs. It contains: Lymph nodes. The heart and its great vessels).";
						dcterms:modified "2020-10-21"^^xsd:date;
						prv:File "clinical_stadification_techniques.ttl";
						prv:File "pathological_stadification_techniques.ttl";								
						dcterms:creator <https://www.tib.eu/en/research-development/scientific-data-management/staff/samaneh-jozashoori/>.

clarify:mediastinotomy	rdf:type	owl:DatatypeProperty;
						rdfs:label	"mediastinotomy";
						rdfs:domain	clarify:ClinicalStageClassification;
						rdfs:range	rdfs:Literal;
						rdfs:comment "Indicates if the stage classification technique (pTNM) used is mediastinotomy (a surgical procedure opening of the mediastinum).";
						dcterms:modified "2020-10-21"^^xsd:date;
						prv:File "clinical_stadification_techniques.ttl";								
						dcterms:creator <https://www.tib.eu/en/research-development/scientific-data-management/staff/samaneh-jozashoori/>.

clarify:thoracicRX	rdf:type	owl:DatatypeProperty;
						rdfs:label	"thoracicRX";
						rdfs:domain	clarify:ClinicalStageClassification;
						rdfs:range	rdfs:Literal;
						rdfs:comment "Indicates if the stage classification technique (pTNM) used is thoracicRX.";
						dcterms:modified "2020-10-21"^^xsd:date;
						prv:File "clinical_stadification_techniques.ttl";								
						dcterms:creator <https://www.tib.eu/en/research-development/scientific-data-management/staff/samaneh-jozashoori/>.

clarify:brainMRI	rdf:type	owl:DatatypeProperty;
						rdfs:label	"brainMRI";
						rdfs:domain	clarify:ClinicalStageClassification;
						rdfs:range	rdfs:Literal;
						rdfs:comment "Indicates if the stage classification technique (pTNM) used is brain MRI.";
						dcterms:modified "2020-10-21"^^xsd:date;
						prv:File "clinical_stadification_techniques.ttl";								
						dcterms:creator <https://www.tib.eu/en/research-development/scientific-data-management/staff/samaneh-jozashoori/>.

clarify:mri	rdf:type	owl:DatatypeProperty;
						rdfs:label	"mri";
						rdfs:domain	clarify:ClinicalStageClassification;
						rdfs:range	rdfs:Literal;
						rdfs:comment "Indicates if the stage classification technique (pTNM) used is MRI.";
						dcterms:modified "2020-10-21"^^xsd:date;
						prv:File "clinical_stadification_techniques.ttl";								
						dcterms:creator <https://www.tib.eu/en/research-development/scientific-data-management/staff/samaneh-jozashoori/>.

clarify:thoracoscopy	rdf:type	owl:DatatypeProperty;
						rdfs:label	"thoracoscopy";
						rdfs:domain	clarify:StageClassification;
						rdfs:range	rdfs:Literal;
						rdfs:comment "Indicates if the stage classification technique (pTNM) used is thoracoscopy (a visual examination of the lung surfaces and pleural space through a viewing tube (a thoracoscope)).";
						dcterms:modified "2020-10-21"^^xsd:date;
						prv:File "clinical_stadification_techniques.ttl";								
						dcterms:creator <https://www.tib.eu/en/research-development/scientific-data-management/staff/samaneh-jozashoori/>.

clarify:thoracotomy	rdf:type	owl:DatatypeProperty;
					rdfs:label	"thoracotomy";
					rdfs:domain	clarify:StageClassification;
					rdfs:range	rdfs:Literal;
					rdfs:comment ".";
					dcterms:modified "2020-11-17"^^xsd:date;
					prv:File "clinical_stadification_techniques.ttl";								
					dcterms:creator <https://www.tib.eu/en/research-development/scientific-data-management/staff/samaneh-jozashoori/>.

clarify:brainCT	rdf:type	owl:DatatypeProperty;
						rdfs:label	"brainCT";
						rdfs:domain	clarify:ClinicalStageClassification;
						rdfs:range	rdfs:Literal;
						rdfs:comment "Indicates if the stage classification technique (pTNM) used is brain CT.";
						dcterms:modified "2020-10-21"^^xsd:date;
						prv:File "clinical_stadification_techniques.ttl";								
						dcterms:creator <https://www.tib.eu/en/research-development/scientific-data-management/staff/samaneh-jozashoori/>.

clarify:petTAC	rdf:type	owl:DatatypeProperty;
						rdfs:label	"petTAC";
						rdfs:domain	clarify:ClinicalStageClassification;
						rdfs:range	rdfs:Literal;
						rdfs:comment "Indicates if the stage classification technique (pTNM) used is pet TAC.";
						dcterms:modified "2020-10-21"^^xsd:date;
						prv:File "clinical_stadification_techniques.ttl";								
						dcterms:creator <https://www.tib.eu/en/research-development/scientific-data-management/staff/samaneh-jozashoori/>.

clarify:biopsy	rdf:type	owl:DatatypeProperty;
				rdfs:label	"biopsy";
				rdfs:domain	clarify:PathologicalStageClassification;
				rdfs:range	rdfs:Literal;
				rdfs:comment "Indicates if the stage classification detection technique (pTNM) used is biopsy.";
				dcterms:modified "2020-10-21"^^xsd:date;
				prv:File "pathological_stadification_techniques.ttl";								
				dcterms:creator <https://www.tib.eu/en/research-development/scientific-data-management/staff/samaneh-jozashoori/>.

clarify:broncoscopy	rdf:type	owl:DatatypeProperty;
					rdfs:label	"broncoscopy";
					rdfs:domain	clarify:PathologicalStageClassification;
					rdfs:range	rdfs:Literal;
					rdfs:comment "Indicates if the stage classification detection technique (pTNM) used is broncoscopy.";
					dcterms:modified "2020-10-21"^^xsd:date;
					prv:File "pathological_stadification_techniques.ttl";								
					dcterms:creator <https://www.tib.eu/en/research-development/scientific-data-management/staff/samaneh-jozashoori/>.

clarify:ebus	rdf:type	owl:DatatypeProperty;
					rdfs:label	"ebus";
					rdfs:domain	clarify:PathologicalStageClassification;
					rdfs:range	rdfs:Literal;
					rdfs:comment "Indicates if the stage classification detection technique (pTNM) used is EBUS (endoluminal ultrasound).";
					dcterms:modified "2020-10-21"^^xsd:date;
					prv:File "pathological_stadification_techniques.ttl";								
					dcterms:creator <https://www.tib.eu/en/research-development/scientific-data-management/staff/samaneh-jozashoori/>.
clarify:laparoscopy	rdf:type	owl:DatatypeProperty;
					rdfs:label	"laparoscopy";
					rdfs:domain	clarify:PathologicalStageClassification;
					rdfs:range	rdfs:Literal;
					rdfs:comment "Indicates if the stage classification detection technique (pTNM) used is laparoscopy.";
					dcterms:modified "2020-10-21"^^xsd:date;
					prv:File "pathological_stadification_techniques.ttl";								
					dcterms:creator <https://www.tib.eu/en/research-development/scientific-data-management/staff/samaneh-jozashoori/>.

clarify:fineNeedleAspiration	rdf:type	owl:DatatypeProperty;
					rdfs:label	"fineNeedleAspiration";
					rdfs:domain	clarify:PathologicalStageClassification;
					rdfs:range	rdfs:Literal;
					rdfs:comment ".";
					dcterms:modified "2020-11-17"^^xsd:date;
					prv:File "pathological_stadification_techniques.ttl";								
					dcterms:creator <https://www.tib.eu/en/research-development/scientific-data-management/staff/samaneh-jozashoori/>.

clarify:transthoracicPuncture	rdf:type	owl:DatatypeProperty;
					rdfs:label	"transthoracicPuncture";
					rdfs:domain	clarify:PathologicalStageClassification;
					rdfs:range	rdfs:Literal;
					rdfs:comment "Indicates if the stage classification detection technique (pTNM) used is transthoracic puncture.";
					dcterms:modified "2020-10-21"^^xsd:date;
					prv:File "pathological_stadification_techniques.ttl";								
					dcterms:creator <https://www.tib.eu/en/research-development/scientific-data-management/staff/samaneh-jozashoori/>.

clarify:transthoracicVats	rdf:type	owl:DatatypeProperty;
					rdfs:label	"transthoracicVats";
					rdfs:domain	clarify:PathologicalStageClassification;
					rdfs:range	rdfs:Literal;
					rdfs:comment ".";
					dcterms:modified "2020-11-17"^^xsd:date;
					prv:File "pathological_stadification_techniques.ttl";								
					dcterms:creator <https://www.tib.eu/en/research-development/scientific-data-management/staff/samaneh-jozashoori/>.

clarify:bloodSample	rdf:type	owl:DatatypeProperty;
					rdfs:label	"bloodSample";
					rdfs:domain	clarify:PathologicalStageClassification;
					rdfs:range	rdfs:Literal;
					rdfs:comment "Indicates if the stage classification detection technique (pTNM) used is blood sample.";
					dcterms:modified "2020-10-21"^^xsd:date;
					prv:File "pathological_stadification_techniques.ttl";								
					dcterms:creator <https://www.tib.eu/en/research-development/scientific-data-management/staff/samaneh-jozashoori/>.

clarify:disorderLabel	rdf:type owl:DatatypeProperty;
							rdfs:label "disorderLabel";
							rdfs:domain clarify:Disorder;
						  	rdfs:range rdfs:Literal;
							rdfs:comment "Disorder label.";
							dcterms:modified "2020-10-21"^^xsd:date;
							prv:File "comorbidity.ttl";
							dcterms:creator <https://www.tib.eu/en/research-development/scientific-data-management/staff/samaneh-jozashoori/>.

clarify:patientCurrentStatus	rdf:type	owl:DatatypeProperty;
								rdfs:label	"patientCurrentStatus";
								rdfs:domain	clarify:StatusEvolution;
								rdfs:range	rdfs:Literal;
								rdfs:comment "Current status of Lung Cancer patient";
								dcterms:modified "2020-10-21"^^xsd:date;
								prv:File "monitoring.ttl";
								dcterms:creator <https://www.tib.eu/en/research-development/scientific-data-management/staff/samaneh-jozashoori/>.	

clarify:lastMonitoringDate	rdf:type owl:DatatypeProperty;
							rdfs:label "lastMonitoringDate";
							rdfs:domain clarify:StatusEvolution;
						  	rdfs:range rdfs:Literal;
							rdfs:comment "Represents the date on which the patient was monitored for the last time.";
							dcterms:modified "2020-10-21"^^xsd:date;
							prv:File "monitoring.ttl";
							dcterms:creator <https://www.tib.eu/en/research-development/scientific-data-management/staff/samaneh-jozashoori/>.

clarify:deathDate	rdf:type	owl:DatatypeProperty;
					rdfs:label	"deathDate";
					rdfs:domain	clarify:StatusEvolution;
					rdfs:range	rdfs:Literal;
					rdfs:comment "Represents the lung cancer patient's date of death (structured information provided by HUPHM).";
					dcterms:modified "2020-10-21"^^xsd:date;
					prv:File "monitoring.ttl";
					dcterms:creator <https://www.tib.eu/en/research-development/scientific-data-management/staff/samaneh-jozashoori/>.

clarify:causeOfDeath	rdf:type	owl:DatatypeProperty;
							rdfs:label	"causeOfDeath";
							rdfs:domain	clarify:StatusEvolution;
							rdfs:range	rdfs:Literal;
							rdfs:comment "Indicates the lung cancer patient's cause of death.";
							dcterms:modified "2020-10-21"^^xsd:date;
							prv:File "monitoring.ttl";
							dcterms:creator <https://www.tib.eu/en/research-development/scientific-data-management/staff/samaneh-jozashoori/>.

clarify:placeOfDeath	rdf:type        owl:DatatypeProperty;	
									rdfs:label	"placeOfDeath";
									rdfs:domain	clarify:StatusEvolution;
									rdfs:range	rdfs:Literal;
									rdfs:comment "The place where the patient died.";
									dcterms:modified "2020-10-21"^^xsd:date;
									prv:File "monitoring.ttl";
									dcterms:creator <https://www.tib.eu/en/research-development/scientific-data-management/staff/samaneh-jozashoori/>.

clarify:secondNeoplasm	rdf:type        owl:DatatypeProperty;	
						rdfs:label	"placeOfDeath";
						rdfs:domain	clarify:StatusEvolution;
						rdfs:range	rdfs:Literal;
						rdfs:comment "Secondary malignant neoplasm is a malignant tumor whose cause is the treatment (usually radiation or chemotherapy) which was used for a prior tumor.";
						dcterms:modified "2020-10-21"^^xsd:date;
						prv:File "monitoring.ttl";
						dcterms:creator <https://www.tib.eu/en/research-development/scientific-data-management/staff/samaneh-jozashoori/>.

clarify:adenocarcinomaHistology	rdf:type        owl:DatatypeProperty;	
								rdfs:label	"adenocarcinomaHistology";
								rdfs:domain	clarify:TumorType;
								rdfs:range	rdfs:Literal;
								rdfs:comment "Represents type of adenocarcinoma (originally developement of the cancer in an organ or gland) experienced by the patient (if any).";
								dcterms:modified "2020-10-21"^^xsd:date;
								prv:File "tumor_histology.ttl";
								dcterms:creator <https://www.tib.eu/en/research-development/scientific-data-management/staff/samaneh-jozashoori/>.

clarify:smallCellCarcinomaType	rdf:type        owl:DatatypeProperty;	
								rdfs:label	"smallCellCarcinomaType";
								rdfs:domain	clarify:TumorType;
								rdfs:range	rdfs:Literal;
								rdfs:comment "Represents the type of small cell carcinoma that patient is experienced (if any).";
								dcterms:modified "2020-10-21"^^xsd:date;
								prv:File "tumor_histology.ttl";
								dcterms:creator <https://www.tib.eu/en/research-development/scientific-data-management/staff/samaneh-jozashoori/>.

clarify:carcinomaType	rdf:type        owl:DatatypeProperty;	
						rdfs:label	"carcinomaType";
						rdfs:domain	clarify:TumorType;
						rdfs:range	rdfs:Literal;
						rdfs:comment "Represents the type of carcinoma that the patient is experienced.";
						dcterms:modified "2020-11-17"^^xsd:date;
						prv:File "tumor_histology.ttl";
						dcterms:creator <https://www.tib.eu/en/research-development/scientific-data-management/staff/samaneh-jozashoori/>.

clarify:mesotheliomaType	rdf:type        owl:DatatypeProperty;	
							rdfs:label	"mesotheliomaType";
							rdfs:domain	clarify:TumorType;
							rdfs:range	rdfs:Literal;
							rdfs:comment "Represents the type of small cell mesothelioma (a malignant tumor that is caused by inhaled asbestos fibers and forms in the lining of the lungs, abdomen or heart) that patient is experienced (if any).";
							dcterms:modified "2020-10-21"^^xsd:date;
							prv:File "tumor_histology.ttl";
							dcterms:creator <https://www.tib.eu/en/research-development/scientific-data-management/staff/samaneh-jozashoori/>.

clarify:histologyDegree	rdf:type        owl:DatatypeProperty;	
							rdfs:label	"histologyDegree";
							rdfs:domain	clarify:TumorType;
							rdfs:range	rdfs:Literal;
							rdfs:comment "Represents the histology degree.";
							dcterms:modified "2020-10-21"^^xsd:date;
							prv:File "tumor_histology.ttl";
							dcterms:creator <https://www.tib.eu/en/research-development/scientific-data-management/staff/samaneh-jozashoori/>.

clarify:performanceStatusValue	rdf:type        owl:DatatypeProperty;	
								rdfs:label	"performanceStatusValue";
								rdfs:domain	clarify:PerformanceStatus;
								rdfs:range	rdfs:Literal;
								rdfs:comment "Represents the evaluated value of the performance status of the patient in certain date.";
								dcterms:modified "2020-10-21"^^xsd:date;
								prv:File "performance_status.ttl";
								dcterms:creator <https://www.tib.eu/en/research-development/scientific-data-management/staff/samaneh-jozashoori/>.

clarify:performanceStatusScale	rdf:type        owl:DatatypeProperty;	
							rdfs:label	"performanceStatusScale";
							rdfs:domain	clarify:PerformanceStatus;
							rdfs:range	rdfs:Literal;
							rdfs:comment "Represents the scale that is applied in patient performance status evaluation.";
							dcterms:modified "2020-10-21"^^xsd:date;
							prv:File "performance_status.ttl";
							dcterms:creator <https://www.tib.eu/en/research-development/scientific-data-management/staff/samaneh-jozashoori/>.

clarify:numberOfCigarettesPerDay	rdf:type	owl:DatatypeProperty;	
									rdfs:label	"numberOfCigarettesPerDay";
									rdfs:domain	clarify:SmokingHistory;
									rdfs:range	rdfs:Literal;
									rdfs:comment	"The number of cigarettes per day that the patient smokes.";
									dcterms:modified "2020-10-21"^^xsd:date;
									prv:File "smoker_information.ttl";
									dcterms:creator <https://www.tib.eu/en/research-development/scientific-data-management/staff/samaneh-jozashoori/>.

clarify:numberOfCigarettesPerYear	rdf:type	owl:DatatypeProperty;	
									rdfs:label	"numberOfCigarettesPerYear";
									rdfs:domain	clarify:SmokingHistory;
									rdfs:range	rdfs:Literal;
									rdfs:comment	"The number of cigarettes per year that the patient smokes.";
									dcterms:modified "2020-11-19"^^xsd:date;
									prv:File "smoker_information.ttl";
									dcterms:creator <https://www.tib.eu/en/research-development/scientific-data-management/staff/samaneh-jozashoori/>.

clarify:smokingStartingDate	rdf:type        owl:DatatypeProperty;	
							rdfs:label	"smokingStartingDate";
							rdfs:domain	clarify:SmokingHistory;
							rdfs:range	rdfs:Literal;
							rdfs:comment "Represents the date on which the patient started smoking (if it was the case).";
							dcterms:modified "2020-10-21"^^xsd:date;
							prv:File "smoker_information.ttl";
							dcterms:creator <https://www.tib.eu/en/research-development/scientific-data-management/staff/samaneh-jozashoori/>.

clarify:smokingStopingDate	rdf:type        owl:DatatypeProperty;	
							rdfs:label	"smokingStartingDate";
							rdfs:domain	clarify:SmokingHistory;
							rdfs:range	rdfs:Literal;
							rdfs:comment "Represents the date on which the patient stoped smoking (if it was the case).";
							dcterms:modified "2020-10-21"^^xsd:date;
							prv:File "smoker_information.ttl";
							dcterms:creator <https://www.tib.eu/en/research-development/scientific-data-management/staff/samaneh-jozashoori/>.

clarify:numberOfYearsOfSmoking	rdf:type        owl:DatatypeProperty;	
								rdfs:label	"numberOfYearsOfSmoking";
								rdfs:domain	clarify:SmokingHistory;
								rdfs:range	rdfs:Literal;
								rdfs:comment "Represents for how many years the patient used to be an active smoker.";
								dcterms:modified "2020-10-21"^^xsd:date;
								prv:File "smoker_information.ttl";
								dcterms:creator <https://www.tib.eu/en/research-development/scientific-data-management/staff/samaneh-jozashoori/>.

clarify:electronicCigarettes	rdf:type        owl:DatatypeProperty;	
								rdfs:label	"electronicCigarettes";
								rdfs:domain	clarify:SmokingHistory;
								rdfs:range	rdfs:Literal;
								rdfs:comment "Represents if the patient smokes electronic cigarettes.";
								dcterms:modified "2020-10-21"^^xsd:date;
								prv:File "smoker_information.ttl";
								dcterms:creator <https://www.tib.eu/en/research-development/scientific-data-management/staff/samaneh-jozashoori/>.

clarify:numberOfElectronicCigarettesPerDay	rdf:type        owl:DatatypeProperty;	
											rdfs:label	"numberOfElectronicCigarettesPerDay";
											rdfs:domain	clarify:SmokingHistory;
											rdfs:range	rdfs:Literal;
											rdfs:comment "Represents the number of electronic cigarettes per day that the patient smokes.";
											dcterms:modified "2020-10-21"^^xsd:date;
											prv:File "smoker_information.ttl";
											dcterms:creator <https://www.tib.eu/en/research-development/scientific-data-management/staff/samaneh-jozashoori/>.

clarify:electronicSmokingStartingDate	rdf:type        owl:DatatypeProperty;	
										rdfs:label	"electronicSmokingStartingDate";
										rdfs:domain	clarify:SmokingHistory;
										rdfs:range	rdfs:Literal;
										rdfs:comment "Represents the date on which the patient started smoking electronic cigarettes (if it was the case).";
										dcterms:modified "2020-10-21"^^xsd:date;
										prv:File "smoker_information.ttl";
										dcterms:creator <https://www.tib.eu/en/research-development/scientific-data-management/staff/samaneh-jozashoori/>.

clarify:electronicSmokingStopingDate	rdf:type        owl:DatatypeProperty;	
										rdfs:label	"electronicSmokingStopingDate";
										rdfs:domain	clarify:SmokingHistory;
										rdfs:range	rdfs:Literal;
										rdfs:comment "Represents the date on which the patient stoped smoking electronic cigarettes (if it was the case).";
										dcterms:modified "2020-10-21"^^xsd:date;
										prv:File "smoker_information.ttl";
										dcterms:creator <https://www.tib.eu/en/research-development/scientific-data-management/staff/samaneh-jozashoori/>.

clarify:rollingTobacco	rdf:type        owl:DatatypeProperty;	
						rdfs:label	"rollingTobacco";
						rdfs:domain	clarify:SmokingHistory;
						rdfs:range	rdfs:Literal;
						rdfs:comment "Represents if the patient smokes rolling(!) tobacco.";
						dcterms:modified "2020-10-21"^^xsd:date;
						prv:File "smoker_information.ttl";
						dcterms:creator <https://www.tib.eu/en/research-development/scientific-data-management/staff/samaneh-jozashoori/>.

clarify:rollingTobaccoSmokingStartingDate	rdf:type        owl:DatatypeProperty;	
											rdfs:label	"rollingTobaccoSmokingStartingDate";
											rdfs:domain	clarify:SmokingHistory;
											rdfs:range	rdfs:Literal;
											rdfs:comment "Represents the date on which the patient started smoking rolling(!) tobacco (if it was the case).";
											dcterms:modified "2020-10-21"^^xsd:date;
											prv:File "smoker_information.ttl";
											dcterms:creator <https://www.tib.eu/en/research-development/scientific-data-management/staff/samaneh-jozashoori/>.

clarify:rollingTobaccoSmokingStopingDate	rdf:type        owl:DatatypeProperty;	
											rdfs:label	"rollingTobaccoSmokingStopingDate";
											rdfs:domain	clarify:SmokingHistory;
											rdfs:range	rdfs:Literal;
											rdfs:comment "Represents the date on which the patient stoped smoking rolling(!) tobacco (if it was the case).";
											dcterms:modified "2020-10-21"^^xsd:date;
											prv:File "smoker_information.ttl";
											dcterms:creator <https://www.tib.eu/en/research-development/scientific-data-management/staff/samaneh-jozashoori/>.

clarify:livingWithSmoker	rdf:type        owl:DatatypeProperty;	
										rdfs:label	"livingWithSmoker";
										rdfs:domain	clarify:SmokingHistory;
										rdfs:range	rdfs:Literal;
										rdfs:comment "Represents if the patient lives with smokers.";
										dcterms:modified "2020-10-21"^^xsd:date;
										prv:File "smoker_information.ttl";
										dcterms:creator <https://www.tib.eu/en/research-development/scientific-data-management/staff/samaneh-jozashoori/>.

clarify:livedWithSmoker	rdf:type        owl:DatatypeProperty;	
										rdfs:label	"livedWithSmoker";
										rdfs:domain	clarify:SmokingHistory;
										rdfs:range	rdfs:Literal;
										rdfs:comment "Represents if the patient used to live with smokers.";
										dcterms:modified "2020-10-21"^^xsd:date;
										prv:File "smoker_information.ttl";
										dcterms:creator <https://www.tib.eu/en/research-development/scientific-data-management/staff/samaneh-jozashoori/>.

clarify:numberOfPregnencies	rdf:type owl:DatatypeProperty;	
							rdfs:label	"numberOfPregnencies";
							rdfs:domain	clarify:ReproductionHistory;
							rdfs:range	rdfs:Literal;
							rdfs:comment "Represents the number of pregnencies that the patient has had.";
							dcterms:modified "2020-10-21"^^xsd:date;
							prv:File "reproductie_information.ttl";
							dcterms:creator <https://www.tib.eu/en/research-development/scientific-data-management/staff/samaneh-jozashoori/>.

clarify:numberOfSuccessfulPregnencies	rdf:type owl:DatatypeProperty;	
										rdfs:label	"numberOfSuccessfulPregnencies";
										rdfs:domain	clarify:ReproductionHistory;
										rdfs:range	rdfs:Literal;
										rdfs:comment "Represents the number of pregnencies that the patient has had.";
										dcterms:modified "2020-10-21"^^xsd:date;
										prv:File "reproductie_information.ttl";
										dcterms:creator <https://www.tib.eu/en/research-development/scientific-data-management/staff/samaneh-jozashoori/>.

clarify:ageOfMenstruation 	rdf:type owl:DatatypeProperty;	
							rdfs:label	"ageOfMenstruation";
							rdfs:domain	clarify:ReproductionHistory;
							rdfs:range	rdfs:Literal;
							rdfs:comment "Represents the age at which the patient began to menstruate.";
							dcterms:modified "2020-10-21"^^xsd:date;
							prv:File "reproductie_information.ttl";
							dcterms:creator <https://www.tib.eu/en/research-development/scientific-data-management/staff/samaneh-jozashoori/>.

clarify:menopause 	rdf:type owl:DatatypeProperty;	
						rdfs:label	"menopause";
						rdfs:domain	clarify:ReproductionHistory;
						rdfs:range	rdfs:Literal;
						rdfs:comment "Represents if the patient has experienced menopause.";
						dcterms:modified "2020-10-21"^^xsd:date;
						prv:File "reproductie_information.ttl";
						dcterms:creator <https://www.tib.eu/en/research-development/scientific-data-management/staff/samaneh-jozashoori/>.

clarify:ageOfMenopause 	rdf:type owl:DatatypeProperty;	
						rdfs:label	"ageOfMenopause";
						rdfs:domain	clarify:ReproductionHistory;
						rdfs:range	rdfs:Literal;
						rdfs:comment "Represents the age at which the menstruate happend.";
						dcterms:modified "2020-10-21"^^xsd:date;
						prv:File "reproductie_information.ttl";
						dcterms:creator <https://www.tib.eu/en/research-development/scientific-data-management/staff/samaneh-jozashoori/>.

clarify:contraceptivePill 	rdf:type owl:DatatypeProperty;	
							rdfs:label	"contraceptivePill";
							rdfs:domain	clarify:ReproductionHistory;
							rdfs:range	rdfs:Literal;
							rdfs:comment "Indicates if the patient takes a contraceptive pill.";
							dcterms:modified "2020-10-21"^^xsd:date;
							prv:File "reproductie_information.ttl";
							dcterms:creator <https://www.tib.eu/en/research-development/scientific-data-management/staff/samaneh-jozashoori/>.

clarify:contraceptivePillStoppingDate 	rdf:type owl:DatatypeProperty;	
										rdfs:label	"contraceptivePillStoppingDate";
										rdfs:domain	clarify:ReproductionHistory;
										rdfs:range	rdfs:Literal;
										rdfs:comment "Represents the date on which the patient stopped taking contraceptive pills (if it was the case).";
										dcterms:modified "2020-10-21"^^xsd:date;
										prv:File "reproductie_information.ttl";
										dcterms:creator <https://www.tib.eu/en/research-development/scientific-data-management/staff/samaneh-jozashoori/>.

clarify:fever 	rdf:type owl:DatatypeProperty;	
				rdfs:label	"fever";
				rdfs:domain	clarify:Prediagnosis;
				rdfs:range	rdfs:Literal;
				rdfs:comment "Represents if the patient experienced fever prior to the diagnosis.";
				dcterms:modified "2020-10-23"^^xsd:date;
				prv:File "Prediagnosis_symptoms.ttl";
				dcterms:creator <https://www.tib.eu/en/research-development/scientific-data-management/staff/samaneh-jozashoori/>.

clarify:weightLoss 	rdf:type owl:DatatypeProperty;	
					rdfs:label	"weightLoss";
					rdfs:domain	clarify:Observation;
					rdfs:range	rdfs:Literal;
					rdfs:comment "Represents if the patient experienced weight loss prior to the diagnosis (1=yes, 0=no, -1=unknown).";
					dcterms:modified "2020-10-23"^^xsd:date;
					prv:File "Prediagnosis_symptoms.ttl";
					prv:File "First_consultation_pre_oncology.ttl";
					dcterms:creator <https://www.tib.eu/en/research-development/scientific-data-management/staff/samaneh-jozashoori/>.

clarify:sleepingDifficulty 	rdf:type owl:DatatypeProperty;	
							rdfs:label	"sleepingDifficulty";
							rdfs:domain	clarify:Prediagnosis;
							rdfs:range	rdfs:Literal;
							rdfs:comment "Represents if the patient experienced sleeping difficulty prior to the diagnosis.";
							dcterms:modified "2020-10-23"^^xsd:date;
							prv:File "Prediagnosis_symptoms.ttl";
							dcterms:creator <https://www.tib.eu/en/research-development/scientific-data-management/staff/samaneh-jozashoori/>.

clarify:leucocytesCount 	rdf:type owl:DatatypeProperty;	
							rdfs:label	"leucocytesCount";
							rdfs:domain	clarify:Hemogram;
							rdfs:range	rdfs:Literal;
							rdfs:comment "Represents a type of White Blood Cell count (WBC).";
							dcterms:modified "2020-10-23"^^xsd:date;
							prv:File "Hemogram.ttl";
							dcterms:creator <https://www.tib.eu/en/research-development/scientific-data-management/staff/samaneh-jozashoori/>.

clarify:lymphocytesCount 	rdf:type owl:DatatypeProperty;	
							rdfs:label	"lymphocytesCount";
							rdfs:domain	clarify:Hemogram;
							rdfs:range	rdfs:Literal;
							rdfs:comment "Represents a type of White Blood Cell count (WBC).";
							dcterms:modified "2020-10-23"^^xsd:date;
							prv:File "Hemogram.ttl";
							dcterms:creator <https://www.tib.eu/en/research-development/scientific-data-management/staff/samaneh-jozashoori/>.

clarify:redBloodCellCount 	rdf:type owl:DatatypeProperty;	
							rdfs:label	"redBloodCellCount";
							rdfs:domain	clarify:Hemogram;
							rdfs:range	rdfs:Literal;
							rdfs:comment "Represents Red Blood Cell count (RBC).";
							dcterms:modified "2020-10-23"^^xsd:date;
							prv:File "Hemogram.ttl";
							dcterms:creator <https://www.tib.eu/en/research-development/scientific-data-management/staff/samaneh-jozashoori/>.

clarify:synchronousTumor 	rdf:type owl:DatatypeProperty;	
							rdfs:label	"synchronousTumor";
							rdfs:domain	clarify:CancerPatient;
							rdfs:range	rdfs:Literal;
							rdfs:comment "Represents if a synchronous tumor is also discovered.";
							dcterms:modified "2020-10-23"^^xsd:date;
							prv:File "Synchronous_tumor.ttl";
							dcterms:creator <https://www.tib.eu/en/research-development/scientific-data-management/staff/samaneh-jozashoori/>.

clarify:asymptomatic 	rdf:type owl:DatatypeProperty;	
						rdfs:label	"asymptomatic";
						rdfs:domain	clarify:NonOncologicalConsultation;
						rdfs:range	rdfs:Literal;
						rdfs:comment "Represents if the patient was asymptomatic.";
						dcterms:modified "2020-10-23"^^xsd:date;
						prv:File "First_consultation_pre_oncology.ttl";
						dcterms:creator <https://www.tib.eu/en/research-development/scientific-data-management/staff/samaneh-jozashoori/>.

clarify:cough 	rdf:type owl:DatatypeProperty;	
				rdfs:label	"cough";
				rdfs:domain	clarify:NonOncologicalConsultation;
				rdfs:range	rdfs:Literal;
				rdfs:comment "Represents if the patient had cough.";
				dcterms:modified "2020-10-23"^^xsd:date;
				prv:File "First_consultation_pre_oncology.ttl";
				dcterms:creator <https://www.tib.eu/en/research-development/scientific-data-management/staff/samaneh-jozashoori/>.

clarify:pain 	rdf:type owl:DatatypeProperty;	
				rdfs:label	"pain";
				rdfs:domain	clarify:NonOncologicalConsultation;
				rdfs:range	rdfs:Literal;
				rdfs:comment "Represents if the patient had any pain.";
				dcterms:modified "2020-10-23"^^xsd:date;
				prv:File "First_consultation_pre_oncology.ttl";
				dcterms:creator <https://www.tib.eu/en/research-development/scientific-data-management/staff/samaneh-jozashoori/>.

clarify:dyspnoea 	rdf:type owl:DatatypeProperty;	
					rdfs:label	"dyspnoea";
					rdfs:domain	clarify:NonOncologicalConsultation;
					rdfs:range	rdfs:Literal;
					rdfs:comment "Represents if the patient experienced dyspnoea (difficulty in breathing.).";
					dcterms:modified "2020-10-23"^^xsd:date;
					prv:File "First_consultation_pre_oncology.ttl";
					dcterms:creator <https://www.tib.eu/en/research-development/scientific-data-management/staff/samaneh-jozashoori/>.														

clarify:hemoptysis 	rdf:type owl:DatatypeProperty;	
					rdfs:label	"hemoptysis";
					rdfs:domain	clarify:NonOncologicalConsultation;
					rdfs:range	rdfs:Literal;
					rdfs:comment "Represents if the patient experienced hemoptysis (coughing up of blood or blood-stained mucus from the bronchi, larynx, trachea, or lungs).";
					dcterms:modified "2020-10-23"^^xsd:date;
					prv:File "First_consultation_pre_oncology.ttl";
					dcterms:creator <https://www.tib.eu/en/research-development/scientific-data-management/staff/samaneh-jozashoori/>.

clarify:asthenia 	rdf:type owl:DatatypeProperty;	
					rdfs:label	"asthenia";
					rdfs:domain	clarify:NonOncologicalConsultation;
					rdfs:range	rdfs:Literal;
					rdfs:comment "Represents if the patient experienced asthenia (abnormal physical weakness or lack of energy).";
					dcterms:modified "2020-10-23"^^xsd:date;
					prv:File "First_consultation_pre_oncology.ttl";
					dcterms:creator <https://www.tib.eu/en/research-development/scientific-data-management/staff/samaneh-jozashoori/>.

clarify:anorexia 	rdf:type owl:DatatypeProperty;	
					rdfs:label	"anorexia";
					rdfs:domain	clarify:NonOncologicalConsultation;
					rdfs:range	rdfs:Literal;
					rdfs:comment "Represents if the patient experienced anorexia (eating disorder).";
					dcterms:modified "2020-10-23"^^xsd:date;
					prv:File "First_consultation_pre_oncology.ttl";
					dcterms:creator <https://www.tib.eu/en/research-development/scientific-data-management/staff/samaneh-jozashoori/>.														

clarify:comment 	rdf:type owl:DatatypeProperty;	
					rdfs:label	"comment";
					rdfs:domain	clarify:CancerPatient;
					rdfs:range	rdfs:Literal;
					rdfs:comment "Represents further clinical comments provided in the clinical notes.";
					dcterms:modified "2020-10-23"^^xsd:date;
					prv:File "Comments.ttl";
					dcterms:creator <https://www.tib.eu/en/research-development/scientific-data-management/staff/samaneh-jozashoori/>.		

#################################################################################################################################################																																			
#################################################################################################################################################
#################################################################################################################################################
#################################################### Properties - relationships #################################################################
#################################################################################################################################################
#################################################################################################################################################
#################################################################################################################################################

clarify:provenance	rdf:type	owl:ObjectProperty;
					rdfs:label	"provenance";
					rdfs:domain	clarify:Concept;
					rdfs:range	clarify:SourceName;
					rdfs:comment	"The name of the source from which the concept is extracted or derived";
					dcterms:modified "2020-10-19"^^xsd:date;
					dcterms:creator <https://www.tib.eu/en/research-development/scientific-data-management/staff/samaneh-jozashoori/>.

clarify:hasCUIAnnotation	rdf:type owl:ObjectProperty;
							rdfs:label	"hasCUIAnnotation";
							rdfs:domain clarify:Concept;
			  				rdfs:range clarify:Annotation;
							rdfs:comment	"CUI annotation of the concept.";
							dcterms:modified "2020-10-19"^^xsd:date;
							dcterms:creator <https://www.tib.eu/en/research-development/scientific-data-management/staff/samaneh-jozashoori/>.

clarify:gender	rdf:type	owl:ObjectProperty;
				rdfs:label	"gender";
				rdfs:domain	clarify:CancerPatient;
				rdfs:range	clarify:Gender;
				rdfs:comment	"Gender value of the patient.";
				dcterms:modified "2020-10-19"^^xsd:date;
				prv:File "patient.ttl";
				dcterms:creator <https://www.tib.eu/en/research-development/scientific-data-management/staff/samaneh-jozashoori/>.	

clarify:hasRace	rdf:type	owl:ObjectProperty;
				rdfs:label	"hasRace";
				rdfs:domain	clarify:CancerPatient;
				rdfs:range	clarify:Race;
				rdfs:comment	"Race value of the patient.";
				dcterms:modified "2020-11-16"^^xsd:date;
				prv:File "patient.ttl";
				dcterms:creator <https://www.tib.eu/en/research-development/scientific-data-management/staff/samaneh-jozashoori/>.		

clarify:hasBiomarkerObservation	rdf:type	owl:ObjectProperty;
								rdfs:label	"hasBiomarkerObservation";
								rdfs:domain	clarify:CancerPatient;
								rdfs:range	clarify:BiomarkerObservation;
								rdfs:comment ".";
								dcterms:modified "2020-10-19"^^xsd:date;
								prv:File "mutation.ttl";
								prv:File "biomarker_mutation.ttl";								
								dcterms:creator <https://www.tib.eu/en/research-development/scientific-data-management/staff/samaneh-jozashoori/>.								

clarify:hasBiomarker	rdf:type	owl:ObjectProperty;
						rdfs:label	"hasBiomarker";
						rdfs:domain	clarify:Concept;
						rdfs:range	clarify:Biomarker;
						rdfs:comment ".";
						dcterms:modified "2020-10-19"^^xsd:date;
						prv:File "mutation.ttl";
						prv:File "biomarker_mutation.ttl";						
						dcterms:creator <https://www.tib.eu/en/research-development/scientific-data-management/staff/samaneh-jozashoori/>.						

clarify:exposed_to	rdf:type	owl:ObjectProperty;
								rdfs:label	"exposed_to";
								rdfs:domain	clarify:CancerPatient;
								rdfs:range	clarify:Carcinogen;
								rdfs:comment "Relation between the cancer patient and exposed carcinogen.";
								dcterms:modified "2020-10-20"^^xsd:date;
								prv:File "environmental_risk.ttl";								
								dcterms:creator <https://www.tib.eu/en/research-development/scientific-data-management/staff/samaneh-jozashoori/>.		

clarify:involved_in	rdf:type	owl:ObjectProperty;
								rdfs:label	"involved_in";
								rdfs:domain	clarify:CancerPatient;
								rdfs:range	clarify:ClinicalTrial;
								rdfs:comment "Relation between the cancer patient and the clinical trial.";
								dcterms:modified "2020-10-20"^^xsd:date;
								prv:File "clinical_trial.ttl";								
								dcterms:creator <https://www.tib.eu/en/research-development/scientific-data-management/staff/samaneh-jozashoori/>.	

clarify:hasStage	rdf:type	owl:ObjectProperty;
								rdfs:label	"hasStage";
								rdfs:domain	clarify:CancerPatient;
								rdfs:range	clarify:CancerStageTNM;
								rdfs:comment "Relation between the cancer patient and the cancer stage.";
								dcterms:modified "2020-10-20"^^xsd:date;
								prv:File "tnm_stadification.ttl";								
								dcterms:creator <https://www.tib.eu/en/research-development/scientific-data-management/staff/samaneh-jozashoori/>.

clarify:metastasized_to	rdf:type	owl:ObjectProperty;
								rdfs:label	"metastasized_to";
								rdfs:domain	clarify:CancerStageTNM;
								rdfs:range	clarify:MetastasisLocation;
								rdfs:comment "Relation between the cancer patient and the metastasis location.";
								dcterms:modified "2020-10-20"^^xsd:date;
								prv:File "metastasis_location.ttl";								
								dcterms:creator <https://www.tib.eu/en/research-development/scientific-data-management/staff/samaneh-jozashoori/>.		

clarify:hasDiagnosis	rdf:type     owl:ObjectProperty;
						rdfs:label	"hasDiagnosis";
						rdfs:domain	clarify:CancerPatient;
						rdfs:range	clarify:Diagnosis;
						rdfs:comment "Patient's initial diagnosis.";
						dcterms:modified "2020-10-20"^^xsd:date;
						prv:File "diagnostic.ttl";
						dcterms:creator <https://www.tib.eu/en/research-development/scientific-data-management/staff/samaneh-jozashoori/>.			

clarify:hasOncologicalTreatmentLine       rdf:type     owl:ObjectProperty;
										rdfs:label	"hasOncologicalTreatmentLine";
										rdfs:domain	clarify:LCPatient;
										rdfs:range	clarify:OncologicalTreatmentLine;
										rdfs:comment "Oncological treatment line  received by the patient.";
										dcterms:modified "2020-10-20"^^xsd:date;
										dcterms:creator <https://www.tib.eu/en/research-development/scientific-data-management/staff/samaneh-jozashoori/>.

clarify:hasChemotherapyTreatmentLine       rdf:type     owl:ObjectProperty;
										rdfs:label	"hasChemotherapyTreatmentLine";
										rdfs:domain	clarify:LCPatient;
										rdfs:range	clarify:ChemotherapyTreatmentLine;
										rdfs:subPropertyOf clarify:hasOncologicalTreatmentLine;
										rdfs:comment "Relation between the patient and the chemotherapy treatment line that is received by the patient.";
										dcterms:modified "2020-10-20"^^xsd:date;
										prv:File "chemotherapy_treatment_line.ttl";
										dcterms:creator <https://www.tib.eu/en/research-development/scientific-data-management/staff/samaneh-jozashoori/>.

clarify:hasRadiotherapyTreatmentLine    rdf:type     owl:ObjectProperty;
										rdfs:label	"hasRadiotherapyTreatmentLine";
										rdfs:domain	clarify:LCPatient;
										rdfs:range	clarify:RadiotherapyTreatmentLine;
										rdfs:subPropertyOf clarify:hasOncologicalTreatmentLine;
										rdfs:comment "Relation between the patient and the radiotherapy treatment line that is received by the patient.";
										dcterms:modified "2020-10-20"^^xsd:date;
										prv:File "radiotherapy_treatment_line.ttl";
										dcterms:creator <https://www.tib.eu/en/research-development/scientific-data-management/staff/samaneh-jozashoori/>.

clarify:hasProgressionRelapseObservation    rdf:type     owl:ObjectProperty;
										rdfs:label	"hasProgressionRelapseObservation";
										rdfs:domain	clarify:LCPatient;
										rdfs:range	clarify:ProgressionRelapseObservation;
										rdfs:comment "Relation between the patient and the radiotherapy treatment line that is received by the patient.";
										dcterms:modified "2020-11-16"^^xsd:date;
										prv:File "relapse_progression.ttl";
										dcterms:creator <https://www.tib.eu/en/research-development/scientific-data-management/staff/samaneh-jozashoori/>.

clarify:hasOncologicalSurgery	rdf:type        owl:ObjectProperty;	
											rdfs:label	"hasOncologicalSurgery";
											rdfs:domain	clarify:LCPatient;
											rdfs:range	clarify:OncologicalSurgery;
											rdfs:comment "A relation between each oncological surgery observation and related data.";
											dcterms:modified "2020-10-20"^^xsd:date;
											prv:File "surgery.ttl";
											dcterms:creator <https://www.tib.eu/en/research-development/scientific-data-management/staff/samaneh-jozashoori/>.	

clarify:hasPatientHistory	rdf:type        owl:ObjectProperty;	
							rdfs:label	"hasPatientHistory";
							rdfs:domain	clarify:CancerPatient;
							rdfs:range	clarify:PatientHistory;
							rdfs:comment "Connection between patient and her/his cancer history.";
							dcterms:modified "2020-11-16"^^xsd:date;
							prv:File "oncological_history.ttl";
							dcterms:creator <https://www.tib.eu/en/research-development/scientific-data-management/staff/samaneh-jozashoori/>.

clarify:hasFamilyHistory	rdf:type        owl:ObjectProperty;	
							rdfs:label	"hasFamilyHistory";
							rdfs:domain	clarify:CancerPatient;
							rdfs:range	clarify:FamilyHistory;
							rdfs:comment "Connection between patient and her/his family history.";
							dcterms:modified "2020-11-16"^^xsd:date;
							prv:File "oncological_history.ttl";
							dcterms:creator <https://www.tib.eu/en/research-development/scientific-data-management/staff/samaneh-jozashoori/>.

clarify:hasDrug	rdf:type        owl:ObjectProperty;	
				rdfs:label	"hasDrug";
				rdfs:domain	clarify:ChemotherapyTreatmentLine;
				rdfs:range	clarify:Drug;
				rdfs:comment "A relation between the chemotherapy treatment line and the prescribed drug.";
				dcterms:modified "2020-10-20"^^xsd:date;
				prv:File "chemotherapy_drugs.ttl";
				dcterms:creator <https://www.tib.eu/en/research-development/scientific-data-management/staff/samaneh-jozashoori/>.													

clarify:hasClinicalStageClassification	rdf:type        owl:ObjectProperty;	
										rdfs:label	"hasDrug";
										rdfs:domain	clarify:CancerPatient;
										rdfs:range	clarify:ClinicalStageClassification;
										rdfs:comment "A relation between the patient and the clinical stage technique.";
										dcterms:modified "2020-10-21"^^xsd:date;
										prv:File "clinical_stadification_techniques.ttl";
										dcterms:creator <https://www.tib.eu/en/research-development/scientific-data-management/staff/samaneh-jozashoori/>.	

clarify:hasPathologicalStageClassification	rdf:type        owl:ObjectProperty;
											rdfs:label	"hasDrug";
											rdfs:domain	clarify:CancerPatient;
											rdfs:range	clarify:PathologicalStageClassification;
											rdfs:comment "A relation between the patient and the pathological stage technique.";
											dcterms:modified "2020-10-21"^^xsd:date;
											prv:File "PathologicalStageClassification.ttl";
											dcterms:creator <https://www.tib.eu/en/research-development/scientific-data-management/staff/samaneh-jozashoori/>.					

clarify:hasComorbidity	rdf:type        owl:ObjectProperty;	
						rdfs:label	"hasComorbidity";
						rdfs:domain	clarify:CancerPatient;
						rdfs:range	clarify:Disorder;
						rdfs:comment	"Connection between patient and her/his Comorbidities.";
						dcterms:modified "2020-10-21"^^xsd:date;
						prv:File "comorbidity.ttl";
						dcterms:creator <https://www.tib.eu/en/research-development/scientific-data-management/staff/samaneh-jozashoori/>.

clarify:hasNonOncologicalConsultation	rdf:type        owl:ObjectProperty;	
						rdfs:label	"hasNonOncologicalConsultation";
						rdfs:domain	clarify:CancerPatient;
						rdfs:range	clarify:NonOncologicalConsultation;
						rdfs:comment	"Connection between patient and her/his non-oncological consultation that have had.";
						dcterms:modified "2020-11-17"^^xsd:date;
						prv:File "First_consultation_pre_oncology.ttl";
						dcterms:creator <https://www.tib.eu/en/research-development/scientific-data-management/staff/samaneh-jozashoori/>.

clarify:hasPrediagnosis	rdf:type        owl:ObjectProperty;	
						rdfs:label	"hasPrediagnosis";
						rdfs:domain	clarify:CancerPatient;
						rdfs:range	clarify:Prediagnosis;
						rdfs:comment	"Connection between patient and her/his prediagnosis observation.";
						dcterms:modified "2020-11-17"^^xsd:date;
						prv:File "Prediagnosis_symptoms.ttl";
						dcterms:creator <https://www.tib.eu/en/research-development/scientific-data-management/staff/samaneh-jozashoori/>.

clarify:hasMontoring	rdf:type        owl:ObjectProperty;	
						rdfs:label	"hasMontoring";
						rdfs:domain	clarify:CancerPatient;
						rdfs:range	clarify:StatusEvolution;
						rdfs:comment	"Connection between patient and srvival observation.";
						dcterms:modified "2020-10-21"^^xsd:date;
						prv:File "monitoring.ttl";
						dcterms:creator <https://www.tib.eu/en/research-development/scientific-data-management/staff/samaneh-jozashoori/>.		

clarify:hasTumorHistology	rdf:type        owl:ObjectProperty;	
						rdfs:label	"hasTumorHistology";
						rdfs:domain	clarify:CancerPatient;
						rdfs:range	clarify:TumorType;
						rdfs:comment	"Connection between patient and the tumor histology (type).";
						dcterms:modified "2020-10-21"^^xsd:date;
						prv:File "tumor_histology.ttl";
						dcterms:creator <https://www.tib.eu/en/research-development/scientific-data-management/staff/samaneh-jozashoori/>.										

clarify:hasPerformanceStatus   rdf:type     owl:ObjectProperty;
							rdfs:label	"hasPerformanceStatus";
							rdfs:domain	clarify:CancerPatient;
							rdfs:range	clarify:PerformanceStatus;
							rdfs:comment "Relation between the patient and their performance status.";
							dcterms:modified "2020-10-21"^^xsd:date;
							prv:File "performance_status.ttl";
							dcterms:creator <https://www.tib.eu/en/research-development/scientific-data-management/staff/samaneh-jozashoori/>.	

clarify:hasSmokingHistory   rdf:type     owl:ObjectProperty;
							rdfs:label	"hasSmokingHistory";
							rdfs:domain	clarify:CancerPatient;
							rdfs:range	clarify:SmokingHistory;
							rdfs:comment "Relation between the patient and their smoking history.";
							dcterms:modified "2020-10-21"^^xsd:date;
							prv:File "smoker_information.ttl";
							dcterms:creator <https://www.tib.eu/en/research-development/scientific-data-management/staff/samaneh-jozashoori/>.	

clarify:hasReproductionHistory  rdf:type     owl:ObjectProperty;
								rdfs:label	"hasReproductionHistory";
								rdfs:domain	clarify:CancerPatient;
								rdfs:range	clarify:ReproductionHistory;
								rdfs:comment "Relation between the patient and their reproduction history.";
								dcterms:modified "2020-10-21"^^xsd:date;
								prv:File "reproductive_information.ttl";
								dcterms:creator <https://www.tib.eu/en/research-development/scientific-data-management/staff/samaneh-jozashoori/>.	
